<?xml version="1.0"?>
<!DOCTYPE rdf:RDF [
    <!ENTITY dcterms "http://purl.org/dc/terms/" >
    <!ENTITY vann "http://purl.org/vocab/vann/" >
    <!ENTITY owl "http://www.w3.org/2002/07/owl#" >
    <!ENTITY qu "http://purl.oclc.org/NET/ssnx/qu/qu#" >
    <!ENTITY dc "http://purl.org/dc/elements/1.1/" >
    <!ENTITY xsd "http://www.w3.org/2001/XMLSchema#" >
    <!ENTITY iottaxolite "http://purl.org/iot/vocab/iot-taxonomy-lite#" >
    <!ENTITY xml "http://www.w3.org/XML/1998/namespace" >
    <!ENTITY rdfs "http://www.w3.org/2000/01/rdf-schema#" >
    <!ENTITY geo "http://www.w3.org/2003/01/geo/wgs84_pos#" >
    <!ENTITY rdf "http://www.w3.org/1999/02/22-rdf-syntax-ns#" >
    <!ENTITY qudt "http://data.qudt.org/qudt/owl/1.0.0/unit.owl#" >
    <!ENTITY vs "http://www.w3.org/2003/06/sw-vocab-status/ns#" >
    <!ENTITY sosa "http://www.w3.org/ns/sosa/" >
    <!ENTITY skos "http://www.w3.org/2004/02/skos/core#">
    <!ENTITY ssn "http://www.w3.org/ns/ssn/">
    <!ENTITY consent "http://purl.org/adaptcentre/openscience/ontologies/consent#">
    <!ENTITY iot-lite "http://purl.oclc.org/NET/UNIS/fiware/iot-lite#" >
]>
<rdf:RDF xmlns="http://purl.org/iot/vocab/iot-taxonomy-lite#"
     xml:base="http://purl.org/iot/vocab/iot-taxonomy-lite#"
     xmlns:vann="http://purl.org/vocab/vann/"
     xmlns:vs="http://www.w3.org/2003/06/sw-vocab-status/ns#"
     xmlns:qudt="http://data.qudt.org/qudt/owl/1.0.0/unit.owl#"
     xmlns:dcterms="http://purl.org/dc/terms/"
     xmlns:rdfs="http://www.w3.org/2000/01/rdf-schema#"
     xmlns:iottaxolite="http://purl.org/iot/vocab/iot-taxonomy-lite#"
     xmlns:rdf="http://www.w3.org/1999/02/22-rdf-syntax-ns#"
     xmlns:qu="http://purl.oclc.org/NET/ssnx/qu/qu#"
     xmlns:dc="http://purl.org/dc/elements/1.1/"
     xmlns:geo="http://www.w3.org/2003/01/geo/wgs84_pos#"
     xmlns:iot-lite="http://purl.oclc.org/NET/UNIS/fiware/iot-lite#"
     xmlns:xml="http://www.w3.org/XML/1998/namespace"
     xmlns:xsd="http://www.w3.org/2001/XMLSchema#"
     xmlns:skos="http://www.w3.org/2004/02/skos/core#"
     xmlns:sosa="http://www.w3.org/ns/sosa/"
     xmlns:ssn="http://www.w3.org/ns/ssn/"
     xmlns:consent="http://purl.org/adaptcentre/openscience/ontologies/consent#"
     xmlns:owl="http://www.w3.org/2002/07/owl#">

    <owl:Ontology rdf:about="http://purl.org/iot/vocab/iot-taxonomy-lite#">
        <owl:versionInfo rdf:datatype="&xsd;decimal">1</owl:versionInfo>
        <dcterms:issued rdf:datatype="&xsd;date">2019-09-07</dcterms:issued>
        <rdfs:comment xml:lang="en">The IoT-Taxonomy-lite is adapted from M3-lite taxonomy. This taxonomy is refactored and defines many other concepts such as subclasses of Feature-of-Interest and Quality-of-Observation. </rdfs:comment>
        <vann:preferredNamespacePrefix>iot-taxonomy-lite</vann:preferredNamespacePrefix>
        <vann:preferredNamespaceUri>http://purl.org/iot/vocab/iot-taxonomy-lite#</vann:preferredNamespaceUri>
        <dc:title xml:lang="en">The IoTTaxonomy-lite Taxonomy</dc:title>
        <dcterms:modified rdf:datatype="&xsd;date">2019-09-07</dcterms:modified>
        <dc:contributor xml:lang="en">Elias Tragos, UCD, Dublin</dc:contributor>
        <dc:contributor xml:lang="en">Rachit Agarwal, Inria, Paris</dc:contributor>
        <dc:contributor xml:lang="en">Tarek Elsaleh, UNIS, Surrey</dc:contributor>
        <dc:description xml:lang="en">The IoT-Taxonomy-lite is adapted from M3-lite taxonomy. This taxonomy is refactored and defines many other concepts such as subclasses of Feature-of-Interest and Quality-of-Observation. 

        We further acknowledge authors of M3-lite for the initial work.

        Please report any errors to rachit.agarwal@inria.fr

        </dc:description>
        <dc:rights>Creative Commons Attribution 4.0 International</dc:rights>
    </owl:Ontology>



    

    <!--
    ///////////////////////////////////////////////////////////////////////////////////////
    //
    // Annotation properties
    //
    ///////////////////////////////////////////////////////////////////////////////////////
     -->



    <!-- http://purl.org/dc/elements/1.1/description -->

    <owl:AnnotationProperty rdf:about="&dc;description"/>



    <!-- http://purl.org/dc/elements/1.1/title -->

    <owl:AnnotationProperty rdf:about="&dc;title"/>



    <!-- http://purl.org/dc/terms/issued -->

    <owl:AnnotationProperty rdf:about="&dcterms;issued"/>



    <!-- http://purl.org/dc/terms/modified -->

    <owl:AnnotationProperty rdf:about="&dcterms;modified"/>



    <!-- http://purl.org/vocab/vann/preferredNamespacePrefix -->

    <owl:AnnotationProperty rdf:about="&vann;preferredNamespacePrefix"/>



    <!-- http://purl.org/vocab/vann/preferredNamespaceUri -->

    <owl:AnnotationProperty rdf:about="&vann;preferredNamespaceUri"/>



    <!-- http://www.w3.org/2000/01/rdf-schema#comment -->

    <owl:AnnotationProperty rdf:about="&rdfs;comment"/>



    <!-- http://www.w3.org/2002/07/owl#equivalentClass -->

    <owl:AnnotationProperty rdf:about="&owl;equivalentClass"/>


    <!-- http://purl.org/dc/elements/1.1/creator -->

    <owl:AnnotationProperty rdf:about="&dc;creator"/>
    

    <!-- http://purl.org/dc/elements/1.1/contributor -->

    <owl:AnnotationProperty rdf:about="&dc;contributor"/>



    <!-- http://purl.org/dc/elements/1.1/rights -->

    <owl:AnnotationProperty rdf:about="&dc;rights"/>

    <!-- http://www.w3.org/2002/07/owl#versionInfo -->

    <owl:AnnotationProperty rdf:about="&owl;versionInfo"/>


        <!-- http://www.w3.org/2000/01/rdf-schema#isDefinedBy -->

    <owl:AnnotationProperty rdf:about="&rdfs;isDefinedBy"/>
    


    <!-- http://www.w3.org/2000/01/rdf-schema#label -->

    <owl:AnnotationProperty rdf:about="&rdfs;label"/>
    


    <!-- http://www.w3.org/2000/01/rdf-schema#seeAlso -->

    <owl:AnnotationProperty rdf:about="&rdfs;seeAlso"/>

    <!--
    ///////////////////////////////////////////////////////////////////////////////////////
    //
    // Object Properties
    //
    ///////////////////////////////////////////////////////////////////////////////////////
     -->




    



    <!--
    ///////////////////////////////////////////////////////////////////////////////////////
    //
    // Classes
    //
    ///////////////////////////////////////////////////////////////////////////////////////
     -->

<!-- http://purl.oclc.org/NET/UNIS/fiware/iot-lite#Tag -->

    <owl:Class rdf:about="&iot-lite;Tag">
        <rdfs:subClassOf rdf:resource="&ssn;System"/>
        <rdfs:comment xml:lang="en">
        Device that can redirect to a resource with information (i.e. RFID, NFC, QR-codes, bar-codes).
        </rdfs:comment>
        <rdfs:label xml:lang="en">Tagging Device</rdfs:label>
    </owl:Class>

<!-- http://www.w3.org/ns/sosa/Actuator -->

    <owl:Class rdf:about="&sosa;Actuator">
        <rdfs:subClassOf rdf:resource="&ssn;System"/>
        <rdfs:comment xml:lang="en">A device that is used by, or implements, an (Actuation) Procedure that changes the state of the world.</rdfs:comment>
        <rdfs:isDefinedBy rdf:resource="http://www.w3.org/ns/sosa/"/>
        <rdfs:label xml:lang="en">Actuator</rdfs:label>
        <skos:example xml:lang="en">A window actuator for automatic window control, i.e., opening or closing the window.</skos:example>
    </owl:Class>

    <!-- http://www.w3.org/ns/sosa/Sensor -->

    <owl:Class rdf:about="&sosa;Sensor">
        <rdfs:subClassOf rdf:resource="http://www.w3.org/ns/ssn/System"/>
        <rdfs:comment xml:lang="en">Device, agent (including humans), or software (simulation) involved in, or implementing, a Procedure. Sensors respond to a stimulus, e.g., a change in the environment, or input data composed from the results of prior Observations, and generate a Result. Sensors can be hosted by Platforms.</rdfs:comment>
        <rdfs:isDefinedBy rdf:resource="http://www.w3.org/ns/sosa/"/>
        <rdfs:label xml:lang="en">Sensor</rdfs:label>
        <skos:example xml:lang="en">Accelerometers, gyroscopes, barometers, magnetometers, and so forth are Sensors that are typically mounted on a modern smart phone (which acts as Platform). Other examples of sensors include the human eyes.</skos:example>
    </owl:Class>

    <!-- http://www.w3.org/ns/sosa/FeatureOfInterest -->

    <owl:Class rdf:about="&sosa;FeatureOfInterest">
        <rdfs:comment xml:lang="en">The thing whose property is being estimated or calculated in the course of an Observation to arrive at a Result or whose property is being manipulated by an Actuator, or which is being sampled or transformed in an act of Sampling.</rdfs:comment>
        <rdfs:isDefinedBy rdf:resource="http://www.w3.org/ns/sosa/"/>
        <rdfs:label xml:lang="en">Feature Of Interest</rdfs:label>
        <skos:example xml:lang="en">When measuring the height of a tree, the height is the observed ObservableProperty, 20m may be the Result of the Observation, and the tree is the FeatureOfInterest. A window is a FeatureOfInterest for an automatic window control Actuator.</skos:example>
    </owl:Class>

    <!-- http://www.w3.org/ns/sosa/Platform -->

    <owl:Class rdf:about="&sosa;Platform">
        <rdfs:comment xml:lang="en">A Platform is an entity that hosts other entities, particularly Sensors, Actuators, Samplers, and other Platforms.</rdfs:comment>
        <rdfs:isDefinedBy rdf:resource="http://www.w3.org/ns/sosa/"/>
        <rdfs:label xml:lang="en">Platform</rdfs:label>
        <skos:example xml:lang="en">A post, buoy, vehicle, ship, aircraft, satellite, cell-phone, human or animal may act as platforms for (technical or biological) sensors or actuators.</skos:example>
    </owl:Class>

    <!-- http://www.w3.org/ns/sosa/ObservableProperty -->

    <owl:Class rdf:about="&sosa;ObservableProperty">
        <rdfs:subClassOf rdf:resource="http://www.w3.org/ns/ssn/Property"/>
        <rdfs:comment xml:lang="en">An observable quality (property, characteristic) of a FeatureOfInterest.</rdfs:comment>
        <rdfs:isDefinedBy rdf:resource="http://www.w3.org/ns/sosa/"/>
        <rdfs:label xml:lang="en">Observable Property</rdfs:label>
        <skos:example xml:lang="en">The height of a tree, the depth of a water body, or the temperature of a surface are examples of observable properties, while the value of a classic car is not (directly) observable but asserted.</skos:example>
    </owl:Class>

    <!-- http://www.w3.org/ns/ssn/System -->

    <owl:Class rdf:about="http://www.w3.org/ns/ssn/System">
        <rdfs:comment xml:lang="en">System is a unit of abstraction for pieces of infrastructure that implement Procedures. A System may have components, its subsystems, which are other systems.</rdfs:comment>
        <rdfs:isDefinedBy rdf:resource="http://www.w3.org/ns/ssn/"/>
        <rdfs:label xml:lang="en">System</rdfs:label>
    </owl:Class>

    <!-- http://purl.oclc.org/NET/ssnx/qu/qu#Unit -->

    <owl:Class rdf:about="http://purl.oclc.org/NET/ssnx/qu/qu#Unit">
        <rdfs:comment>A Unit is an abstract classifier that represents the [VIM] concept of &quot;measurement unit&quot; that is defined as &quot;real scalar quantity, defined and adopted by convention, with which any other quantity of the same kind can be compared to express the ratio of the two quantities as a number.&quot;</rdfs:comment>
        <rdfs:isDefinedBy>http://purl.oclc.org/NET/ssnx/qu</rdfs:isDefinedBy>
        <rdfs:label>Unit</rdfs:label>
        <rdfs:seeAlso>http://www.omgsysml.org/qudv#Unit</rdfs:seeAlso>
    </owl:Class>


    <!-- http://www.w3.org/ns/ssn/Property -->

    <owl:Class rdf:about="http://www.w3.org/ns/ssn/Property">
        <rdfs:comment xml:lang="en">A quality of an entity. An aspect of an entity that is intrinsic to and cannot exist without the entity.</rdfs:comment>
        <rdfs:isDefinedBy rdf:resource="http://www.w3.org/ns/ssn/"/>
        <rdfs:label xml:lang="en">Property</rdfs:label>
    </owl:Class>


    <!-- http://purl.org/iot/vocab/iot-taxonomy-lite#Bar -->

    <owl:Class rdf:about="&iottaxolite;Bar">
        <rdfs:subClassOf rdf:resource="&qu;Unit"/>
        <rdfs:comment xml:lang="en">Metric unit of atmospheric pressure equal to 14.50 pounds per square inch (lb/in2), 1.02 kilograms per square centimetre (kg/cm2), 29.53 inches of mercury (in Hg), or 0.9869 atmosphere.</rdfs:comment>
        <rdfs:label xml:lang="en">Bar</rdfs:label>
        <rdfs:seeAlso>http://qudt.org/vocab/unit#Bar</rdfs:seeAlso>
        <rdfs:isDefinedBy rdf:resource="http://purl.org/iot/vocab/m3-lite#"/>
    </owl:Class>



    <!-- http://purl.org/iot/vocab/iot-taxonomy-lite#DegreeAngle -->

    <owl:Class rdf:about="&iottaxolite;DegreeAngle">
        <rdfs:subClassOf rdf:resource="&iottaxolite;Degree"/>
        <rdfs:comment xml:lang="en">A plane angle unit which is equal to 1/360 of a full rotation or pi/180 rad.</rdfs:comment>
        <rdfs:label xml:lang="en">Degree Angle</rdfs:label>
        <rdfs:seeAlso>http://qudt.org/vocab/unit#DegreeAngle</rdfs:seeAlso>
        <rdfs:isDefinedBy rdf:resource="http://purl.org/iot/vocab/m3-lite#"/>
    </owl:Class>



    <!-- http://purl.org/iot/vocab/iot-taxonomy-lite#ElectricCurrent -->

    <owl:Class rdf:about="&iottaxolite;ElectricCurrent">
        <rdfs:subClassOf rdf:resource="&sosa;ObservableProperty"/>
        <rdfs:comment xml:lang="en">Electric current is the flow of electric charge. It is a base quantity in the International System of Units. Electric current is electric charge divided by time. Electric Current is the flow (movement) of electric charge. The amount of electric current through some surface, e.g., a section through a copper conductor, is defined as the amount of electric charge flowing through that surface over time.</rdfs:comment>
        <rdfs:label xml:lang="en">Electric Current</rdfs:label>
        <rdfs:seeAlso>http://qudt.org/vocab/quantity#ElectricCurrent</rdfs:seeAlso>
        <rdfs:isDefinedBy rdf:resource="http://purl.org/iot/vocab/m3-lite#"/>
    </owl:Class>


    <!-- http://purl.org/iot/vocab/iot-taxonomy-lite#ABS -->

    <owl:Class rdf:about="&iottaxolite;ABS">
        <rdfs:subClassOf rdf:resource="&sosa;Actuator"/>
        <rdfs:comment xml:lang="en">The ABS (Anti-lock Braking System) receives information from ABS computer to control the pressure on the breaks, This helps the wheels not to get locked up, it adjust the break pressure and prevents the wheels from locking. (Definition Source Google).</rdfs:comment>
        <rdfs:label xml:lang="en">ABS (Anti-lock Braking System) Actuating Device</rdfs:label>
        <rdfs:isDefinedBy rdf:resource="http://purl.org/iot/vocab/m3-lite#"/>
    </owl:Class>



    <!-- http://purl.org/iot/vocab/iot-taxonomy-lite#AccInitialERabEstabSuccRate -->

    <owl:Class rdf:about="&iottaxolite;AccInitialERabEstabSuccRate">
        <rdfs:subClassOf rdf:resource="&iottaxolite;Communication"/>
        <rdfs:comment xml:lang="en">Initial E-UTRAN Radio Access Bearer establishment success rate.</rdfs:comment>
        <rdfs:label xml:lang="en">Initial E-RAB Establishment Success Rate</rdfs:label>
        <rdfs:isDefinedBy rdf:resource="http://purl.org/iot/vocab/m3-lite#"/>
    </owl:Class>



    <!-- http://purl.org/iot/vocab/iot-taxonomy-lite#AccInitialERabSetupSuccRate -->

    <owl:Class rdf:about="&iottaxolite;AccInitialERabSetupSuccRate">
        <rdfs:subClassOf rdf:resource="&iottaxolite;Communication"/>
        <rdfs:comment xml:lang="en">Initial E-UTRAN Radio Access Bearer setup success rate.</rdfs:comment>
        <rdfs:label xml:lang="en">Initial E-RAB Setup Success Rate</rdfs:label>
        <rdfs:isDefinedBy rdf:resource="http://purl.org/iot/vocab/m3-lite#"/>
    </owl:Class>



    <!-- http://purl.org/iot/vocab/iot-taxonomy-lite#AccRrcConnSetupSuccRate -->

    <owl:Class rdf:about="&iottaxolite;AccRrcConnSetupSuccRate">
        <rdfs:subClassOf rdf:resource="&iottaxolite;Communication"/>
        <rdfs:comment xml:lang="en">Radio Resource Control connection setup success rate.</rdfs:comment>
        <rdfs:label xml:lang="en">RRC Connection Setup Success Rate</rdfs:label>
        <rdfs:isDefinedBy rdf:resource="http://purl.org/iot/vocab/m3-lite#"/>
    </owl:Class>



    <!-- http://purl.org/iot/vocab/iot-taxonomy-lite#AccS1SigEstabSuccRate -->

    <owl:Class rdf:about="&iottaxolite;AccS1SigEstabSuccRate">
        <rdfs:subClassOf rdf:resource="&iottaxolite;Communication"/>
        <rdfs:comment xml:lang="en">S1 (S1 standardized interface between eNB and Evolved Packet Core) signalling establishment success rate.</rdfs:comment>
        <rdfs:label xml:lang="en">S1 Signalling Establishment Success Rate</rdfs:label>
        <rdfs:isDefinedBy rdf:resource="http://purl.org/iot/vocab/m3-lite#"/>
    </owl:Class>



    <!-- http://purl.org/iot/vocab/iot-taxonomy-lite#Acceleration -->

    <owl:Class rdf:about="&iottaxolite;Acceleration">
        <rdfs:subClassOf rdf:resource="&sosa;ObservableProperty"/>
        <rdfs:comment xml:lang="en">The rate of change of the velocity of a particle with respect to time.</rdfs:comment>
        <rdfs:label xml:lang="en">Acceleration</rdfs:label>
        <rdfs:seeAlso>http://purl.oclc.org/NET/ssnx/qu/dim#Acceleration</rdfs:seeAlso>
        <rdfs:isDefinedBy rdf:resource="http://purl.org/iot/vocab/m3-lite#"/>
    </owl:Class>



    <!-- http://purl.org/iot/vocab/iot-taxonomy-lite#AccelerationInstantaneous -->

    <owl:Class rdf:about="&iottaxolite;AccelerationInstantaneous">
        <rdfs:subClassOf rdf:resource="&iottaxolite;Acceleration"/>
        <rdfs:label xml:lang="en">Instantaneous Acceleration</rdfs:label>
        <rdfs:comment xml:lang="en">The acceleration at a given instant of time.</rdfs:comment>
        <rdfs:isDefinedBy rdf:resource="http://purl.org/iot/vocab/m3-lite#"/>
    </owl:Class>



    <!-- http://purl.org/iot/vocab/iot-taxonomy-lite#Accelerometer -->

    <owl:Class rdf:about="&iottaxolite;Accelerometer">
        <rdfs:subClassOf rdf:resource="&sosa;Sensor"/>
        <rdfs:comment xml:lang="en"> Accelerometers are used to automatically determine the orientation in which the user is holding the IoT Object (portrait or landscape).</rdfs:comment>
        <rdfs:label xml:lang="en">Accelerometer</rdfs:label>
        <rdfs:seeAlso rdf:resource="http://casas.wsu.edu/owl/cose.owl#Accelerometer"/>
        <rdfs:isDefinedBy rdf:resource="http://purl.org/iot/vocab/m3-lite#"/>
    </owl:Class>



    <!-- http://purl.org/iot/vocab/iot-taxonomy-lite#ActivePower -->

    <owl:Class rdf:about="&iottaxolite;ActivePower">
        <rdfs:subClassOf rdf:resource="&iottaxolite;Power"/>
        <rdfs:comment xml:lang="en">The product of the voltage across a branch of an alternating-current circuit and the component of the electric current that is in phase with the voltage.</rdfs:comment>
        <rdfs:label xml:lang="en">Active Power</rdfs:label>
        <rdfs:seeAlso>http://purl.oclc.org/NET/ssnx/qu/quantity#activePower</rdfs:seeAlso>
        <rdfs:isDefinedBy rdf:resource="http://purl.org/iot/vocab/m3-lite#"/>
    </owl:Class>



    <!-- http://purl.org/iot/vocab/iot-taxonomy-lite#Agriculture -->

    <owl:Class rdf:about="&iottaxolite;Agriculture">
        <rdfs:subClassOf rdf:resource="&iottaxolite;DomainOfInterest"/>
        <rdfs:comment xml:lang="en">Agriculture, Smart farm as an Internet of Things (IoT) applicative domain.</rdfs:comment>
        <rdfs:label xml:lang="en">Agriculture DOI</rdfs:label>
        <rdfs:isDefinedBy rdf:resource="http://purl.org/iot/vocab/m3-lite#"/>
    </owl:Class>



    <!-- http://purl.org/iot/vocab/iot-taxonomy-lite#AirConditioner -->

    <owl:Class rdf:about="&iottaxolite;AirConditioner">
        <rdfs:subClassOf rdf:resource="&sosa;Actuator"/>
        <rdfs:comment xml:lang="en">An actuator to automatically switch on/off the air conditioner.</rdfs:comment>
        <rdfs:label xml:lang="en">Air Conditioner Actuating Device</rdfs:label>
        <rdfs:isDefinedBy rdf:resource="http://purl.org/iot/vocab/m3-lite#"/>
    </owl:Class>



    <!-- http://purl.org/iot/vocab/iot-taxonomy-lite#AirPollutantSensor -->

    <owl:Class rdf:about="&iottaxolite;AirPollutantSensor">
        <rdfs:subClassOf rdf:resource="&sosa;Sensor"/>
        <rdfs:comment xml:lang="en">Air Pollutant Sensor are devices that detect and monitor the presence of air pollution in the surrounding area (source Wikipedia).</rdfs:comment>
        <rdfs:label xml:lang="en">Air Pollutant Sensor</rdfs:label>
        <rdfs:isDefinedBy rdf:resource="http://purl.org/iot/vocab/m3-lite#"/>
    </owl:Class>



    <!-- http://purl.org/iot/vocab/iot-taxonomy-lite#AirPollution -->

    <owl:Class rdf:about="&iottaxolite;AirPollution">
        <rdfs:subClassOf rdf:resource="&sosa;ObservableProperty"/>
        <rdfs:comment xml:lang="en">Usually measured using Air Quality Index (AQI), it is the measure of Air Pollution in the environment. It is similar to Air Quality.</rdfs:comment>
        <rdfs:label xml:lang="en">Air Pollution Quantity Kind</rdfs:label>
        <rdfs:isDefinedBy rdf:resource="http://purl.org/iot/vocab/m3-lite#"/>
    </owl:Class>



    <!-- http://purl.org/iot/vocab/iot-taxonomy-lite#AirQuality -->

    <owl:Class rdf:about="&iottaxolite;AirQuality">
        <rdfs:subClassOf rdf:resource="&sosa;ObservableProperty"/>
        <rdfs:comment xml:lang="en">Usually measured using an air quality index (AQI) that is a number used by government agencies to communicate to the public how polluted the air currently is or how polluted it is forecast to become. Different countries have their own air quality indices, corresponding to different national air quality standards. It is the measure of Air Quality of the environment. It is similar to Air Pollution. (Source Wikipedia).</rdfs:comment>
        <rdfs:label xml:lang="en">Air Quality Quantity Kind</rdfs:label>
        <rdfs:isDefinedBy rdf:resource="http://purl.org/iot/vocab/m3-lite#"/>
    </owl:Class>



    <!-- http://purl.org/iot/vocab/iot-taxonomy-lite#AirTemperature -->

    <owl:Class rdf:about="&iottaxolite;AirTemperature">
        <rdfs:subClassOf rdf:resource="&iottaxolite;Temperature"/>
        <rdfs:comment xml:lang="en">The temperature of the air that would be indicated by a thermometer exposed to the air at a location sheltered from direct solar radiation.</rdfs:comment>
        <rdfs:label xml:lang="en">Air Temperature, Weather Temperature, Ambient Temperature</rdfs:label>
        <rdfs:seeAlso rdf:resource="http://openiot.eu/ontology/ns/AirTemperature"/>
        <rdfs:seeAlso rdf:resource="http://paul.staroch.name/thesis/SmartHomeWeather.owl#Temperature"/>
        <rdfs:isDefinedBy rdf:resource="http://purl.org/iot/vocab/m3-lite#"/>
    </owl:Class>



    <!-- http://purl.org/iot/vocab/iot-taxonomy-lite#AirThermometer -->

    <owl:Class rdf:about="&iottaxolite;AirThermometer">
        <rdfs:subClassOf rdf:resource="&iottaxolite;Thermometer"/>
        <rdfs:comment xml:lang="en">Device to measure the Air temperature of either indoor or outdoor atmosphere.</rdfs:comment>
        <rdfs:label xml:lang="en">Air Thermometer</rdfs:label>
        <rdfs:isDefinedBy rdf:resource="http://purl.org/iot/vocab/m3-lite#"/>
    </owl:Class>



    <!-- http://purl.org/iot/vocab/iot-taxonomy-lite#AlarmSystem -->

    <owl:Class rdf:about="&iottaxolite;AlarmSystem">
        <rdfs:subClassOf rdf:resource="&sosa;Actuator"/>
        <rdfs:comment xml:lang="en">An actuator to automatically switch on/off the alarm system.</rdfs:comment>
        <rdfs:label xml:lang="en">Alarm System Actuating Device</rdfs:label>
        <rdfs:isDefinedBy rdf:resource="http://purl.org/iot/vocab/m3-lite#"/>
    </owl:Class>



    <!-- http://purl.org/iot/vocab/iot-taxonomy-lite#AlcoholLevel -->

    <owl:Class rdf:about="&iottaxolite;AlcoholLevel">
        <rdfs:subClassOf rdf:resource="&sosa;ObservableProperty"/>
        <rdfs:comment xml:lang="en">Measure of Alcohol Level in the system.</rdfs:comment>
        <rdfs:label xml:lang="en">Alcohol Level Quantity Kind</rdfs:label>
        <rdfs:isDefinedBy rdf:resource="http://purl.org/iot/vocab/m3-lite#"/>
    </owl:Class>



    <!-- http://purl.org/iot/vocab/iot-taxonomy-lite#AlcoholLevelSensor -->

    <owl:Class rdf:about="&iottaxolite;AlcoholLevelSensor">
        <rdfs:subClassOf rdf:resource="&sosa;Sensor"/>
        <rdfs:comment xml:lang="en">Device used to detect and measure Alcohol Level in the system.</rdfs:comment>
        <rdfs:label xml:lang="en">Alcohol Level Sensor</rdfs:label>
        <rdfs:isDefinedBy rdf:resource="http://purl.org/iot/vocab/m3-lite#"/>
    </owl:Class>




    <!-- http://purl.org/iot/vocab/iot-taxonomy-lite#Ampere -->

    <owl:Class rdf:about="&iottaxolite;Ampere">
        <rdfs:subClassOf rdf:resource="&qu;Unit"/>
        <rdfs:comment xml:lang="en">The ampere is the SI unit for measuring an electric current which is the flow of electric charges through a surface at the rate of one coulomb per second.The ampere is the SI unit for measuring an electric current which is the flow of electric charges through a surface at the rate of one coulomb per second.</rdfs:comment>
        <rdfs:label xml:lang="en">Ampere (A)</rdfs:label>
        <rdfs:seeAlso rdf:resource="&qudt;Ampere"/>
        <rdfs:seeAlso rdf:resource="http://sweet.jpl.nasa.gov/ontology/units.owl#ampere"/>
        <rdfs:seeAlso>http://purl.oclc.org/NET/ssnx/qu/unit#ampere</rdfs:seeAlso>
        <rdfs:isDefinedBy rdf:resource="http://purl.org/iot/vocab/m3-lite#"/>
    </owl:Class>


    <!-- http://purl.org/iot/vocab/iot-taxonomy-lite#AngularSpeed -->

    <owl:Class rdf:about="&iottaxolite;AngularSpeed">
        <rdfs:subClassOf rdf:resource="&sosa;ObservableProperty"/>
        <rdfs:comment xml:lang="en">It is the rate of change of angular displacement and is a vector quantity (more precisely, a pseudovector) that specifies the angular speed (rotational speed) of an object and the axis about which the object is rotating. (Source Wikipedia).</rdfs:comment>
        <rdfs:label xml:lang="en">Angular Speed</rdfs:label>
        <rdfs:isDefinedBy rdf:resource="http://purl.org/iot/vocab/m3-lite#"/>
    </owl:Class>




    <!-- http://purl.org/iot/vocab/iot-taxonomy-lite#Animals -->

    <owl:Class rdf:about="&iottaxolite;Animals">
        <rdfs:subClassOf rdf:resource="&iottaxolite;SoundSource"/>
        <rdfs:comment xml:lang="en">when the source of the sound were animals.</rdfs:comment>
        <rdfs:label xml:lang="en">Animals as Sound Source</rdfs:label>
        <rdfs:isDefinedBy rdf:resource="http://purl.org/iot/vocab/m3-lite#"/>
    </owl:Class>



    <!-- http://purl.org/iot/vocab/iot-taxonomy-lite#AtmosphericPressure -->

    <owl:Class rdf:about="&iottaxolite;AtmosphericPressure">
        <rdfs:subClassOf rdf:resource="&iottaxolite;Pressure"/>
        <rdfs:comment xml:lang="en">The pressure exerted by the atmosphere as a consequence of gravitational attraction exerted upon the column of air lying directly above the point in question.</rdfs:comment>
        <rdfs:label xml:lang="en">Atmospheric Pressure</rdfs:label>
        <rdfs:seeAlso rdf:resource="http://openiot.eu/ontology/ns/AtmospherePressure"/>
        <rdfs:seeAlso rdf:resource="http://paul.staroch.name/thesis/SmartHomeWeather.owl#AtmosphericPressure"/>
        <rdfs:seeAlso>http://purl.oclc.org/NET/ssnx/qu/quantity#atmosphericPressure</rdfs:seeAlso>
        <rdfs:isDefinedBy rdf:resource="http://purl.org/iot/vocab/m3-lite#"/>
    </owl:Class>



    <!-- http://purl.org/iot/vocab/iot-taxonomy-lite#AtmosphericPressureSensor -->

    <owl:Class rdf:about="&iottaxolite;AtmosphericPressureSensor">
        <rdfs:subClassOf rdf:resource="&sosa;Sensor"/>
        <rdfs:comment xml:lang="en">Atmospheric Pressure Sensor, Barometer or Barometric Pressure Sensor is a scientific instrument used in meteorology to measure atmospheric pressure.</rdfs:comment>
        <rdfs:label xml:lang="en">Atmospheric Pressure Sensor</rdfs:label>
        <rdfs:seeAlso rdf:resource="http://archive.knoesis.org/research/semsci/application_domain/sem_sensor/ont/weather.owlPressure"/>
        <rdfs:seeAlso rdf:resource="http://casas.wsu.edu/owl/cose.owl#BarometricPressureSensor"/>
        <rdfs:seeAlso rdf:resource="http://purl.oclc.org/NET/ssnx/meteo/aws#AtmosphericPressureSensor"/>
        <rdfs:isDefinedBy rdf:resource="http://purl.org/iot/vocab/m3-lite#"/>
    </owl:Class>



    <!-- http://purl.org/iot/vocab/iot-taxonomy-lite#AutomaticSensing -->

    <owl:Class rdf:about="&iottaxolite;AutomaticSensing">
        <rdfs:subClassOf rdf:resource="&iottaxolite;MeasurementType"/>
        <rdfs:comment xml:lang="en">When the devices are set to take the observations Automatically without any external aid.</rdfs:comment>
        <rdfs:label xml:lang="en">Automatic Measurement Type</rdfs:label>
        <rdfs:isDefinedBy rdf:resource="http://purl.org/iot/vocab/m3-lite#"/>
    </owl:Class>



    <!-- http://purl.org/iot/vocab/iot-taxonomy-lite#Barcode -->

    <owl:Class rdf:about="&iottaxolite;Barcode">
        <rdfs:subClassOf rdf:resource="&iot-lite;Tag"/>
        <rdfs:comment xml:lang="en">A tagging device can be Barcode.</rdfs:comment>
        <rdfs:label xml:lang="en">Barcode Tagging Device</rdfs:label>
        <rdfs:isDefinedBy rdf:resource="http://purl.org/iot/vocab/m3-lite#"/>
    </owl:Class>



    <!-- http://purl.org/iot/vocab/iot-taxonomy-lite#BatteryLevel -->

    <owl:Class rdf:about="&iottaxolite;BatteryLevel">
        <rdfs:subClassOf rdf:resource="&sosa;ObservableProperty"/>
        <rdfs:comment xml:lang="en">Measure of the percentage of the battery capacity that remains available.</rdfs:comment>
        <rdfs:label xml:lang="en">Battery Level Quantity Kind</rdfs:label>
        <rdfs:seeAlso>http://www.w3.org/2007/uwa/context/deliveryContext.owl#BatteryLevel</rdfs:seeAlso>
        <rdfs:isDefinedBy rdf:resource="http://purl.org/iot/vocab/m3-lite#"/>
    </owl:Class>



    <!-- http://purl.org/iot/vocab/iot-taxonomy-lite#BeatPerMinute -->

    <owl:Class rdf:about="&iottaxolite;BeatPerMinute">
        <rdfs:subClassOf rdf:resource="&qu;Unit"/>
        <rdfs:comment xml:lang="en">Beat Per Minute (bpm) is the unit to measure heart rate.</rdfs:comment>
        <rdfs:label xml:lang="en">Beat Per Minute (bpm)</rdfs:label>
        <rdfs:isDefinedBy rdf:resource="http://purl.org/iot/vocab/m3-lite#"/>
    </owl:Class>



    <!-- http://purl.org/iot/vocab/iot-taxonomy-lite#Blind -->

    <owl:Class rdf:about="&iottaxolite;Blind">
        <rdfs:subClassOf rdf:resource="&sosa;Actuator"/>
        <rdfs:comment xml:lang="en">An actuator to automatically switch on/off the window blinds.</rdfs:comment>
        <rdfs:label xml:lang="en">Blind Actuating Device</rdfs:label>
        <rdfs:isDefinedBy rdf:resource="http://purl.org/iot/vocab/m3-lite#"/>
    </owl:Class>



    <!-- http://purl.org/iot/vocab/iot-taxonomy-lite#BloodGlucose -->

    <owl:Class rdf:about="&iottaxolite;BloodGlucose">
        <rdfs:subClassOf rdf:resource="&sosa;ObservableProperty"/>
        <rdfs:comment xml:lang="en">Measure of Blood glucose level or blood sugar level.</rdfs:comment>
        <rdfs:label xml:lang="en">Blood Glucose Quantity Kind</rdfs:label>
        <rdfs:isDefinedBy rdf:resource="http://purl.org/iot/vocab/m3-lite#"/>
    </owl:Class>



    <!-- http://purl.org/iot/vocab/iot-taxonomy-lite#BloodPressure -->

    <owl:Class rdf:about="&iottaxolite;BloodPressure">
        <rdfs:subClassOf rdf:resource="&iottaxolite;Pressure"/>
        <rdfs:comment xml:lang="en">Measure of the pressure in your blood vessels when your heart rests between beats.</rdfs:comment>
        <rdfs:label xml:lang="en">Blood Pressure</rdfs:label>
        <rdfs:isDefinedBy rdf:resource="http://purl.org/iot/vocab/m3-lite#"/>
    </owl:Class>



    <!-- http://purl.org/iot/vocab/iot-taxonomy-lite#BloodPressureSensor -->

    <owl:Class rdf:about="&iottaxolite;BloodPressureSensor">
        <rdfs:subClassOf rdf:resource="&sosa;Sensor"/>
        <rdfs:comment xml:lang="en">Device used to measure Blood Pressure.</rdfs:comment>
        <rdfs:label xml:lang="en">Blood Pressure Sensor</rdfs:label>
        <rdfs:isDefinedBy rdf:resource="http://purl.org/iot/vocab/m3-lite#"/>
    </owl:Class>



    <!-- http://purl.org/iot/vocab/iot-taxonomy-lite#BoardTemperature -->

    <owl:Class rdf:about="&iottaxolite;BoardTemperature">
        <rdfs:subClassOf rdf:resource="&iottaxolite;Temperature"/>
        <rdfs:comment xml:lang="en">Measure of board temperature.</rdfs:comment>
        <rdfs:label xml:lang="en">Board Temperature</rdfs:label>
        <rdfs:isDefinedBy rdf:resource="http://purl.org/iot/vocab/m3-lite#"/>
    </owl:Class>



    <!-- http://purl.org/iot/vocab/iot-taxonomy-lite#BoardThermometer -->

    <owl:Class rdf:about="&iottaxolite;BoardThermometer">
        <rdfs:subClassOf rdf:resource="&iottaxolite;Thermometer"/>
        <rdfs:comment xml:lang="en">Device used to measure board temperature.</rdfs:comment>
        <rdfs:label xml:lang="en">Board Thermometer</rdfs:label>
        <rdfs:isDefinedBy rdf:resource="http://purl.org/iot/vocab/m3-lite#"/>
    </owl:Class>



    <!-- http://purl.org/iot/vocab/iot-taxonomy-lite#BodyTemperature -->

    <owl:Class rdf:about="&iottaxolite;BodyTemperature">
        <rdfs:subClassOf rdf:resource="&iottaxolite;Temperature"/>
        <rdfs:comment xml:lang="en">Measure of body temperature.</rdfs:comment>
        <rdfs:label xml:lang="en">Body Temperature</rdfs:label>
        <rdfs:isDefinedBy rdf:resource="http://purl.org/iot/vocab/m3-lite#"/>
    </owl:Class>



    <!-- http://purl.org/iot/vocab/iot-taxonomy-lite#BodyThermometer -->

    <owl:Class rdf:about="&iottaxolite;BodyThermometer">
        <rdfs:subClassOf rdf:resource="&iottaxolite;Thermometer"/>
        <rdfs:comment xml:lang="en">Device used to measure body temperature.</rdfs:comment>
        <rdfs:label xml:lang="en">Body Thermometer</rdfs:label>
        <rdfs:isDefinedBy rdf:resource="http://purl.org/iot/vocab/m3-lite#"/>
    </owl:Class>



    <!-- http://purl.org/iot/vocab/iot-taxonomy-lite#Boiler -->

    <owl:Class rdf:about="&iottaxolite;Boiler">
        <rdfs:subClassOf rdf:resource="&sosa;Actuator"/>
        <rdfs:comment xml:lang="en">An actuator to automatically switch on/off the boiler.</rdfs:comment>
        <rdfs:label xml:lang="en">Boiler Actuating Device</rdfs:label>
        <rdfs:isDefinedBy rdf:resource="http://purl.org/iot/vocab/m3-lite#"/>
    </owl:Class>






    <!-- http://purl.org/iot/vocab/iot-taxonomy-lite#BuildingAutomation -->

    <owl:Class rdf:about="&iottaxolite;BuildingAutomation">
        <rdfs:subClassOf rdf:resource="&iottaxolite;DomainOfInterest"/>
        <rdfs:comment xml:lang="en">Smart Home/Building Automation as an Internet of Things (IoT) applicative domain.</rdfs:comment>
        <rdfs:label xml:lang="en">Smart Building DOI</rdfs:label>
        <rdfs:seeAlso rdf:resource="http://elite.polito.it/ontologies/dogont.owl#BuildingEnvironment"/>
        <rdfs:isDefinedBy rdf:resource="http://purl.org/iot/vocab/m3-lite#"/>
    </owl:Class>



    <!-- http://purl.org/iot/vocab/iot-taxonomy-lite#BuildingTemperature -->

    <owl:Class rdf:about="&iottaxolite;BuildingTemperature">
        <rdfs:subClassOf rdf:resource="&iottaxolite;Temperature"/>
        <rdfs:comment xml:lang="en">Measure of building or room temperature.</rdfs:comment>
        <rdfs:label xml:lang="en">Building/Room Temperature</rdfs:label>
        <rdfs:isDefinedBy rdf:resource="http://purl.org/iot/vocab/m3-lite#"/>
    </owl:Class>

    <!-- http://purl.org/iot/vocab/iot-taxonomy-lite#Coordinates -->

    <owl:Class rdf:about="&iottaxolite;Coordinates">
        <rdfs:subClassOf rdf:resource="&qu;Unit"/>
        <rdfs:comment xml:lang="en">Triples for location in the (Latitude, Longitude, Altitude) format.</rdfs:comment>
        <rdfs:label xml:lang="en">Coordinates</rdfs:label>
        <rdfs:isDefinedBy rdf:resource="http://purl.org/iot/vocab/m3-lite#"/>
    </owl:Class>



    <!-- http://purl.org/iot/vocab/iot-taxonomy-lite#CO2 -->

    <owl:Class rdf:about="&iottaxolite;CO2">
        <rdfs:subClassOf rdf:resource="&sosa;ObservableProperty"/>
        <rdfs:comment xml:lang="en">Carbon Dioxide (CO2) measure in the atmosphere.</rdfs:comment>
        <rdfs:label xml:lang="en">Carbon Dioxide (CO2) Quantity Kind</rdfs:label>
        <rdfs:isDefinedBy rdf:resource="http://purl.org/iot/vocab/m3-lite#"/>
    </owl:Class>



    <!-- http://purl.org/iot/vocab/iot-taxonomy-lite#CO2Sensor -->

    <owl:Class rdf:about="&iottaxolite;CO2Sensor">
        <rdfs:subClassOf rdf:resource="&iottaxolite;GaseousPollutantSensor"/>
        <rdfs:comment xml:lang="en">Carbon Dioxide (CO2) Sensor used to measure level of CO2 in the atmosphere.</rdfs:comment>
        <rdfs:label xml:lang="en">Carbon Dioxide (CO2) Sensor</rdfs:label>
        <rdfs:isDefinedBy rdf:resource="http://purl.org/iot/vocab/m3-lite#"/>
    </owl:Class>



    <!-- http://purl.org/iot/vocab/iot-taxonomy-lite#COSensor -->

    <owl:Class rdf:about="&iottaxolite;COSensor">
        <rdfs:subClassOf rdf:resource="&iottaxolite;GaseousPollutantSensor"/>
        <rdfs:comment xml:lang="en">Device to detect Carbon Monoxide (CO) in the environment.</rdfs:comment>
        <rdfs:label xml:lang="en">Carbon Monoxide (CO) Sensor</rdfs:label>
        <rdfs:isDefinedBy rdf:resource="http://purl.org/iot/vocab/m3-lite#"/>
    </owl:Class>



    <!-- http://purl.org/iot/vocab/iot-taxonomy-lite#Calcium -->

    <owl:Class rdf:about="&iottaxolite;Calcium">
        <rdfs:subClassOf rdf:resource="&sosa;ObservableProperty"/>
        <rdfs:comment xml:lang="en">Measure of blood calcium level.</rdfs:comment>
        <rdfs:label xml:lang="en">Calcium Quantity Kind</rdfs:label>
        <rdfs:isDefinedBy rdf:resource="http://purl.org/iot/vocab/m3-lite#"/>
    </owl:Class>



    <!-- http://purl.org/iot/vocab/iot-taxonomy-lite#Calibration -->

    <owl:Class rdf:about="&iottaxolite;CalibrationSensing">
        <rdfs:subClassOf rdf:resource="&iottaxolite;MeasurementType"/>
        <rdfs:comment xml:lang="en">If the measurement was taken when the sensor was being calibrated.</rdfs:comment>
        <rdfs:label xml:lang="en">Calibration Measurement Type</rdfs:label>
        <rdfs:isDefinedBy rdf:resource="http://purl.org/iot/vocab/m3-lite#"/>
    </owl:Class>



    <!-- http://purl.org/iot/vocab/iot-taxonomy-lite#Candela -->

    <owl:Class rdf:about="&iottaxolite;Candela">
        <rdfs:subClassOf rdf:resource="&qu;Unit"/>
        <rdfs:comment xml:lang="en">Candela is the luminous intensity, in a given direction, of a source that emits monochromatic radiation of frequency 540 x 10^12 hertz and that has a radiant intensity in that direction of 1/683 watt per steradian. (Source Wikipedia).</rdfs:comment>
        <rdfs:label xml:lang="en">Candela</rdfs:label>
        <rdfs:seeAlso rdf:resource="http://sweet.jpl.nasa.gov/ontology/units.owl#candela"/>
        <rdfs:isDefinedBy rdf:resource="http://purl.org/iot/vocab/m3-lite#"/>
    </owl:Class>



    <!-- http://purl.org/iot/vocab/iot-taxonomy-lite#Capacitance -->

    <owl:Class rdf:about="&iottaxolite;Capacitance">
        <rdfs:subClassOf rdf:resource="&sosa;ObservableProperty"/>
        <rdfs:comment xml:lang="en">Measure of the ability of a system to store an electric charge.</rdfs:comment>
        <rdfs:label xml:lang="en">Capacitance</rdfs:label>
        <rdfs:isDefinedBy rdf:resource="http://purl.org/iot/vocab/m3-lite#"/>
    </owl:Class>



    <!-- http://purl.org/iot/vocab/iot-taxonomy-lite#Centibar -->

    <owl:Class rdf:about="&iottaxolite;Centibar">
        <rdfs:subClassOf rdf:resource="&iottaxolite;Bar"/>
        <rdfs:comment xml:lang="en">The centibar is a unit of pressure defined as 1e-2 bar.</rdfs:comment>
        <rdfs:label xml:lang="en">Centibar</rdfs:label>
        <rdfs:isDefinedBy rdf:resource="http://purl.org/iot/vocab/m3-lite#"/>
    </owl:Class>



    <!-- http://purl.org/iot/vocab/iot-taxonomy-lite#Centimetre -->

    <owl:Class rdf:about="&iottaxolite;Centimetre">
        <rdfs:subClassOf rdf:resource="&iottaxolite;Metre"/>
        <rdfs:label xml:lang="en">Centimetre, Centimeter</rdfs:label>
        <rdfs:comment xml:lang="en">A metric unit of length, equal to one hundredth of a metre.</rdfs:comment>
        <rdfs:isDefinedBy rdf:resource="http://purl.org/iot/vocab/m3-lite#"/>
    </owl:Class>



    <!-- http://purl.org/iot/vocab/iot-taxonomy-lite#ChemicalAgentAtmosphericConcentration -->

    <owl:Class rdf:about="&iottaxolite;ChemicalAgentAtmosphericConcentration">
        <rdfs:subClassOf rdf:resource="&iottaxolite;ChemicalAgentConcentration"/>
        <rdfs:comment xml:lang="en">Measure of Chemical Agent Atmospheric Concentration</rdfs:comment>
        <rdfs:label xml:lang="en">Chemical Agent Atmospheric Concentration Quantity Kind</rdfs:label>
        <rdfs:isDefinedBy rdf:resource="http://purl.org/iot/vocab/m3-lite#"/>
    </owl:Class>



    <!-- http://purl.org/iot/vocab/iot-taxonomy-lite#ChemicalAgentAtmosphericConcentrationAirParticles -->

    <owl:Class rdf:about="&iottaxolite;ChemicalAgentAtmosphericConcentrationAirParticles">
        <rdfs:subClassOf rdf:resource="&iottaxolite;ChemicalAgentAtmosphericConcentration"/>
        <rdfs:comment xml:lang="en">Measure of the concentration of chemical particles suspended in the atmosphere.</rdfs:comment>
        <rdfs:label xml:lang="en">Air Particles Chemical Agent Atmospheric Concentration</rdfs:label>
        <rdfs:isDefinedBy rdf:resource="http://purl.org/iot/vocab/m3-lite#"/>
    </owl:Class>



    <!-- http://purl.org/iot/vocab/iot-taxonomy-lite#ChemicalAgentAtmosphericConcentrationCO -->

    <owl:Class rdf:about="&iottaxolite;ChemicalAgentAtmosphericConcentrationCO">
        <rdfs:subClassOf rdf:resource="&iottaxolite;ChemicalAgentAtmosphericConcentration"/>
        <rdfs:comment xml:lang="en">Measure of the concentration of Carbon Monoxide (CO) gas suspended in the atmosphere.</rdfs:comment>
        <rdfs:label xml:lang="en">Carbon Monoxide (CO) Chemical Agent Atmospheric Concentration</rdfs:label>
        <rdfs:isDefinedBy rdf:resource="http://purl.org/iot/vocab/m3-lite#"/>
    </owl:Class>



    <!-- http://purl.org/iot/vocab/iot-taxonomy-lite#ChemicalAgentAtmosphericConcentrationNO2 -->

    <owl:Class rdf:about="&iottaxolite;ChemicalAgentAtmosphericConcentrationNO2">
        <rdfs:subClassOf rdf:resource="&iottaxolite;ChemicalAgentAtmosphericConcentration"/>
        <rdfs:comment xml:lang="en">Measure of the concentration of NO2 gas suspended in the atmosphere.</rdfs:comment>
        <rdfs:label xml:lang="en">NO2 Chemical Agent Atmospheric Concentration</rdfs:label>
        <rdfs:isDefinedBy rdf:resource="http://purl.org/iot/vocab/m3-lite#"/>
    </owl:Class>



    <!-- http://purl.org/iot/vocab/iot-taxonomy-lite#Cholesterol -->

    <owl:Class rdf:about="&iottaxolite;Cholesterol">
        <rdfs:subClassOf rdf:resource="&sosa;ObservableProperty"/>
        <rdfs:comment xml:lang="en">Measure of the cholesterol level in a system.</rdfs:comment>
        <rdfs:label xml:lang="en">Cholesterol Quantity Kind</rdfs:label>
        <rdfs:isDefinedBy rdf:resource="http://purl.org/iot/vocab/m3-lite#"/>
    </owl:Class>



    <!-- http://purl.org/iot/vocab/iot-taxonomy-lite#CholesterolSensor -->

    <owl:Class rdf:about="&iottaxolite;CholesterolSensor">
        <rdfs:subClassOf rdf:resource="&sosa;Sensor"/>
        <rdfs:comment xml:lang="en">Device used to measure the cholesterol level in a system.</rdfs:comment>
        <rdfs:label xml:lang="en">Cholesterol Sensor</rdfs:label>
        <rdfs:isDefinedBy rdf:resource="http://purl.org/iot/vocab/m3-lite#"/>
    </owl:Class>



    <!-- http://purl.org/iot/vocab/iot-taxonomy-lite#City -->

    <owl:Class rdf:about="&iottaxolite;City">
        <rdfs:subClassOf rdf:resource="&iottaxolite;DomainOfInterest"/>
        <rdfs:comment xml:lang="en">Smart City as an Internet of Things (IoT) applicative domain.</rdfs:comment>
        <rdfs:label xml:lang="en">Smart City DOI</rdfs:label>
        <rdfs:isDefinedBy rdf:resource="http://purl.org/iot/vocab/m3-lite#"/>
    </owl:Class>





    <!-- http://purl.org/iot/vocab/iot-taxonomy-lite#CloudCover -->

    <owl:Class rdf:about="&iottaxolite;CloudCover">
        <rdfs:subClassOf rdf:resource="&sosa;ObservableProperty"/>
        <rdfs:comment xml:lang="en">Measure of cloud cover at a certain time. </rdfs:comment>
        <rdfs:label xml:lang="en">Cloud Cover Quantity Kind</rdfs:label>
        <rdfs:isDefinedBy rdf:resource="http://purl.org/iot/vocab/m3-lite#"/>
    </owl:Class>



    <!-- http://purl.org/iot/vocab/iot-taxonomy-lite#CloudCoverSensor -->

    <owl:Class rdf:about="&iottaxolite;CloudCoverSensor">
        <rdfs:subClassOf rdf:resource="&sosa;Sensor"/>
        <rdfs:comment xml:lang="en">Cloud Cover Sensor is used to detect whether it is sunny, cloudy, etc.</rdfs:comment>
        <rdfs:label xml:lang="en">Cloud Cover Sensor</rdfs:label>
        <rdfs:isDefinedBy rdf:resource="http://purl.org/iot/vocab/m3-lite#"/>
    </owl:Class>



    <!-- http://purl.org/iot/vocab/iot-taxonomy-lite#CoffeeMachine -->

    <owl:Class rdf:about="&iottaxolite;CoffeeMachine">
        <rdfs:subClassOf rdf:resource="&sosa;Actuator"/>
        <rdfs:comment xml:lang="en">An actuator to automatically switch on/off the coffee machine.</rdfs:comment>
        <rdfs:label xml:lang="en">Coffee Machine, Coffee Maker Actuating Device</rdfs:label>
        <rdfs:isDefinedBy rdf:resource="http://purl.org/iot/vocab/m3-lite#"/>
    </owl:Class>



    <!-- http://purl.org/iot/vocab/iot-taxonomy-lite#Communication -->

    <owl:Class rdf:about="&iottaxolite;Communication">
        <rdfs:subClassOf rdf:resource="&sosa;ObservableProperty"/>
        <rdfs:comment xml:lang="en">Communication related properties.</rdfs:comment>
        <rdfs:label xml:lang="en">Communication</rdfs:label>
        <rdfs:isDefinedBy rdf:resource="http://purl.org/iot/vocab/m3-lite#"/>
    </owl:Class>



    <!-- http://purl.org/iot/vocab/iot-taxonomy-lite#Computer -->

    <owl:Class rdf:about="&iottaxolite;Computer">
        <rdfs:subClassOf rdf:resource="&sosa;Actuator"/>
        <rdfs:comment xml:lang="en">Actuating devices for Computer or PC.</rdfs:comment>
        <rdfs:label xml:lang="en">Computer, PC Actuating Device</rdfs:label>
        <rdfs:isDefinedBy rdf:resource="http://purl.org/iot/vocab/m3-lite#"/>
    </owl:Class>



    <!-- http://purl.org/iot/vocab/iot-taxonomy-lite#Conductivity -->

    <owl:Class rdf:about="&iottaxolite;Conductivity">
        <rdfs:subClassOf rdf:resource="&sosa;ObservableProperty"/>
        <rdfs:comment xml:lang="en">Measure of ability to conduct electricity. It is measured in siemens per metre (S/m).</rdfs:comment>
        <rdfs:label xml:lang="en">Conductivity</rdfs:label>
        <rdfs:isDefinedBy rdf:resource="http://purl.org/iot/vocab/m3-lite#"/>
    </owl:Class>



    <!-- http://purl.org/iot/vocab/iot-taxonomy-lite#ConductivitySensor -->

    <owl:Class rdf:about="&iottaxolite;ConductivitySensor">
        <rdfs:subClassOf rdf:resource="&sosa;Sensor"/>
        <rdfs:comment xml:lang="en">Device used to measure the conductivity of a system.</rdfs:comment>
        <rdfs:label xml:lang="en">Conductivity Sensor</rdfs:label>
        <rdfs:isDefinedBy rdf:resource="http://purl.org/iot/vocab/m3-lite#"/>
    </owl:Class>



    <!-- http://purl.org/iot/vocab/iot-taxonomy-lite#ConstructionWork -->

    <owl:Class rdf:about="&iottaxolite;ConstructionWork">
        <rdfs:subClassOf rdf:resource="&iottaxolite;SoundSource"/>
        <rdfs:comment xml:lang="en">When the source of the sound was a construction work.</rdfs:comment>
        <rdfs:label xml:lang="en">Construction Work Sound Source</rdfs:label>
        <rdfs:isDefinedBy rdf:resource="http://purl.org/iot/vocab/m3-lite#"/>
    </owl:Class>



    <!-- http://purl.org/iot/vocab/iot-taxonomy-lite#Coulomb -->

    <owl:Class rdf:about="&iottaxolite;Coulomb">
        <rdfs:subClassOf rdf:resource="&qu;Unit"/>
        <rdfs:comment xml:lang="en">SI unit of electric charge.</rdfs:comment>
        <rdfs:label xml:lang="en">Coulomb</rdfs:label>
        <rdfs:seeAlso rdf:resource="http://sweet.jpl.nasa.gov/ontology/units.owl#coulomb"/>
        <rdfs:isDefinedBy rdf:resource="http://purl.org/iot/vocab/m3-lite#"/>
    </owl:Class>



    <!-- http://purl.org/iot/vocab/iot-taxonomy-lite#Crowd -->

    <owl:Class rdf:about="&iottaxolite;Crowd">
        <rdfs:subClassOf rdf:resource="&iottaxolite;SoundSource"/>
        <rdfs:comment xml:lang="en">When the source of the sound was crowd.</rdfs:comment>
        <rdfs:label xml:lang="en">Crowd Sound Source</rdfs:label>
        <rdfs:isDefinedBy rdf:resource="http://purl.org/iot/vocab/m3-lite#"/>
    </owl:Class>



    <!-- http://purl.org/iot/vocab/iot-taxonomy-lite#Cupboard -->

    <owl:Class rdf:about="&iottaxolite;Cupboard">
        <rdfs:subClassOf rdf:resource="&sosa;Actuator"/>
        <rdfs:comment xml:lang="en">An actuator to automatically open/close the cupboard.</rdfs:comment>
        <rdfs:label xml:lang="en">Cupboard Actuating Device</rdfs:label>
        <rdfs:isDefinedBy rdf:resource="http://purl.org/iot/vocab/m3-lite#"/>
    </owl:Class>



    <!-- http://purl.org/iot/vocab/iot-taxonomy-lite#Curtain -->

    <owl:Class rdf:about="&iottaxolite;Curtain">
        <rdfs:subClassOf rdf:resource="&sosa;Actuator"/>
        <rdfs:comment xml:lang="en">An actuator to automatically open/close the curtain.</rdfs:comment>
        <rdfs:label xml:lang="en">Curtain Actuating Device</rdfs:label>
        <rdfs:isDefinedBy rdf:resource="http://purl.org/iot/vocab/m3-lite#"/>
    </owl:Class>




    <!-- http://purl.org/iot/vocab/iot-taxonomy-lite#Day -->

    <owl:Class rdf:about="&iottaxolite;Day">
        <rdfs:subClassOf rdf:resource="&iottaxolite;SecondTime"/>
        <rdfs:comment xml:lang="en">Day is a unit of time.</rdfs:comment>
        <rdfs:label xml:lang="en">Day</rdfs:label>
        <rdfs:isDefinedBy rdf:resource="http://purl.org/iot/vocab/m3-lite#"/>
    </owl:Class>



    <!-- http://purl.org/iot/vocab/iot-taxonomy-lite#Decibel -->

    <owl:Class rdf:about="&iottaxolite;Decibel">
        <rdfs:subClassOf rdf:resource="&qu;Unit"/>
        <rdfs:comment xml:lang="en">Decibel is a logarithmic unit used to express the ratio of two values of a physical quantity. It is often used to measure sound level.</rdfs:comment>
        <rdfs:label xml:lang="en">Decibel (dB)</rdfs:label>
        <rdfs:seeAlso>http://purl.oclc.org/NET/ssnx/qu/unit#decibel</rdfs:seeAlso>
        <rdfs:isDefinedBy rdf:resource="http://purl.org/iot/vocab/m3-lite#"/>
    </owl:Class>



    <!-- http://purl.org/iot/vocab/iot-taxonomy-lite#DecibelA -->

    <owl:Class rdf:about="&iottaxolite;DecibelA">
        <rdfs:subClassOf rdf:resource="&iottaxolite;Decibel"/>
        <rdfs:comment xml:lang="en">Sound pressure sensed by the human ear.</rdfs:comment>
        <rdfs:label xml:lang="en">DecibelA (dB(A))</rdfs:label>
        <rdfs:isDefinedBy rdf:resource="http://purl.org/iot/vocab/m3-lite#"/>
    </owl:Class>



    <!-- http://purl.org/iot/vocab/iot-taxonomy-lite#Degree -->

    <owl:Class rdf:about="&iottaxolite;Degree">
        <rdfs:subClassOf rdf:resource="&qu;Unit"/>
        <rdfs:comment xml:lang="en">Degree.</rdfs:comment>
        <rdfs:label xml:lang="en">Degree</rdfs:label>
        <rdfs:isDefinedBy rdf:resource="http://purl.org/iot/vocab/m3-lite#"/>
    </owl:Class>



    <!-- http://purl.org/iot/vocab/iot-taxonomy-lite#DegreeCelsius -->

    <owl:Class rdf:about="&iottaxolite;DegreeCelsius">
        <rdfs:subClassOf rdf:resource="&iottaxolite;Degree"/>
        <rdfs:comment xml:lang="en">A temperature unit which is equal to one kelvin degree. However, they have their zeros at different points. The centigrade scale has its zero at 273.15 K.</rdfs:comment>
        <rdfs:label xml:lang="en">Degree Celsius</rdfs:label>
        <rdfs:seeAlso rdf:resource="&qudt;DegreeCelsius"/>
        <rdfs:seeAlso rdf:resource="http://sweet.jpl.nasa.gov/ontology/units.owl#degreeC"/>
        <rdfs:seeAlso rdf:resource="http://purl.oclc.org/NET/ssnx/qu/unit#degreeCelsius"/>
        <rdfs:isDefinedBy rdf:resource="http://purl.org/iot/vocab/m3-lite#"/>
    </owl:Class>



    <!-- http://purl.org/iot/vocab/iot-taxonomy-lite#DegreeFahrenheit -->

    <owl:Class rdf:about="&iottaxolite;DegreeFahrenheit">
        <rdfs:subClassOf rdf:resource="&iottaxolite;Degree"/>
        <rdfs:comment xml:lang="en">Measurement Unit to represent temperature on the Fahrenheit scale.</rdfs:comment>
        <rdfs:label xml:lang="en">Degree Fahrenheit</rdfs:label>
        <rdfs:seeAlso rdf:resource="http://archive.knoesis.org/research/semsci/application_domain/sem_sensor/ont/weather.owlfahrenheit"/>
        <rdfs:seeAlso rdf:resource="http://sweet.jpl.nasa.gov/ontology/units.owl#degreeF"/>
        <rdfs:isDefinedBy rdf:resource="http://purl.org/iot/vocab/m3-lite#"/>
    </owl:Class>



    <!-- http://purl.org/iot/vocab/iot-taxonomy-lite#DeltaDewPoint -->

    <owl:Class rdf:about="&iottaxolite;DeltaDewPoint">
        <rdfs:subClassOf rdf:resource="&iottaxolite;DewPoint"/>
        <rdfs:comment xml:lang="en">Difference between Dewpoint and surface temperatures.</rdfs:comment>
        <rdfs:label xml:lang="en">Delta Dew Point</rdfs:label>
        <rdfs:isDefinedBy rdf:resource="http://purl.org/iot/vocab/m3-lite#"/>
    </owl:Class>



    <!-- http://purl.org/iot/vocab/iot-taxonomy-lite#DeltaDewPointSensor -->

    <owl:Class rdf:about="&iottaxolite;DeltaDewPointSensor">
        <rdfs:subClassOf rdf:resource="&sosa;Sensor"/>
        <rdfs:comment xml:lang="en">Device that measures the difference between Dewpoint and surface temperatures.</rdfs:comment>
        <rdfs:label xml:lang="en">Delta Dew Point Sensor</rdfs:label>
        <rdfs:isDefinedBy rdf:resource="http://purl.org/iot/vocab/m3-lite#"/>
    </owl:Class>



    <!-- http://purl.org/iot/vocab/iot-taxonomy-lite#DewPoint -->

    <owl:Class rdf:about="&iottaxolite;DewPoint">
        <rdfs:subClassOf rdf:resource="&sosa;ObservableProperty"/>
        <rdfs:comment xml:lang="en">It is the temperature to which air must be cooled at constant pressure to condense to form liquid.</rdfs:comment>
        <rdfs:label xml:lang="en">Dew Point</rdfs:label>
        <rdfs:isDefinedBy rdf:resource="http://purl.org/iot/vocab/m3-lite#"/>
    </owl:Class>



    <!-- http://purl.org/iot/vocab/iot-taxonomy-lite#DewPointSensor -->

    <owl:Class rdf:about="&iottaxolite;DewPointSensor">
        <rdfs:subClassOf rdf:resource="&sosa;Sensor"/>
        <rdfs:comment xml:lang="en">Device that measures dew point.</rdfs:comment>
        <rdfs:label xml:lang="en">Dew Point Sensor</rdfs:label>
        <rdfs:isDefinedBy rdf:resource="http://purl.org/iot/vocab/m3-lite#"/>
    </owl:Class>



    <!-- http://purl.org/iot/vocab/iot-taxonomy-lite#DewPointTemperature -->

    <owl:Class rdf:about="&iottaxolite;DewPointTemperature">
        <rdfs:subClassOf rdf:resource="&iottaxolite;DewPoint"/>
        <rdfs:comment xml:lang="en">The temperature at which dew forms and is a measure of atmospheric moisture. It is the temperature to which air must be cooled at constant pressure and water content to reach saturation. A higher dew point indicates more moisture in the air; a dew point greater than 20 Degree C (68 Degree F) is considered uncomfortable and greater than 22 Degree C (72 Degree F) is considered to be extremely humid.</rdfs:comment>
        <rdfs:label xml:lang="en">Dew Point Temperature</rdfs:label>
        <rdfs:isDefinedBy rdf:resource="http://purl.org/iot/vocab/m3-lite#"/>
    </owl:Class>



    <!-- http://purl.org/iot/vocab/iot-taxonomy-lite#DiastolicBloodPressure -->

    <owl:Class rdf:about="&iottaxolite;DiastolicBloodPressure">
        <rdfs:subClassOf rdf:resource="&iottaxolite;BloodPressure"/>
        <rdfs:comment xml:lang="en"> Measure of the pressure in the arteries when the heart rests between beats.</rdfs:comment>
        <rdfs:label xml:lang="en">Diastolic Blood Pressure</rdfs:label>
        <rdfs:isDefinedBy rdf:resource="http://purl.org/iot/vocab/m3-lite#"/>
    </owl:Class>



    <!-- http://purl.org/iot/vocab/iot-taxonomy-lite#Dimensionless -->

    <owl:Class rdf:about="&iottaxolite;Dimensionless">
        <rdfs:subClassOf rdf:resource="&qu;Unit"/>
        <rdfs:comment xml:lang="en">Without dimensions; having no appreciable or noteworthy extent. Without physical meaning.</rdfs:comment>
        <rdfs:label xml:lang="en">Dimensionless</rdfs:label>
        <rdfs:seeAlso rdf:resource="http://purl.oclc.org/NET/ssnx/qu/dim#Dimensionless"/>
        <rdfs:isDefinedBy rdf:resource="http://purl.org/iot/vocab/m3-lite#"/>
    </owl:Class>



    <!-- http://purl.org/iot/vocab/iot-taxonomy-lite#Direction -->

    <owl:Class rdf:about="&iottaxolite;Direction">
        <rdfs:label xml:lang="en">Direction</rdfs:label>
        <rdfs:comment xml:lang="en">Measurements of sensors are affected by the direction of the sensing device. This concept is used to reflect it.</rdfs:comment>
        <rdfs:isDefinedBy rdf:resource="http://purl.org/iot/vocab/m3-lite#"/>
    </owl:Class>



    <!-- http://purl.org/iot/vocab/iot-taxonomy-lite#DirectionAzimuth -->

    <owl:Class rdf:about="&iottaxolite;DirectionAzimuth">
        <rdfs:subClassOf rdf:resource="&iottaxolite;Direction"/>
        <rdfs:comment xml:lang="en">The geodetic azimuth of the direction towards which an object is point to.</rdfs:comment>
        <rdfs:label xml:lang="en">Direction Azimuth</rdfs:label>
        <rdfs:isDefinedBy rdf:resource="http://purl.org/iot/vocab/m3-lite#"/>
    </owl:Class>



    <!-- http://purl.org/iot/vocab/iot-taxonomy-lite#DirectionHeading -->

    <owl:Class rdf:about="&iottaxolite;DirectionHeading">
        <rdfs:subClassOf rdf:resource="&iottaxolite;Direction"/>
        <rdfs:comment xml:lang="en">The course or direction in which a object (vehicle, person, ...) is moving.</rdfs:comment>
        <rdfs:label xml:lang="en">Direction Heading</rdfs:label>
        <rdfs:isDefinedBy rdf:resource="http://purl.org/iot/vocab/m3-lite#"/>
    </owl:Class>



    <!-- http://purl.org/iot/vocab/iot-taxonomy-lite#DishWasher -->

    <owl:Class rdf:about="&iottaxolite;DishWasher">
        <rdfs:subClassOf rdf:resource="&sosa;Actuator"/>
        <rdfs:comment xml:lang="en">An actuator to automatically switch on/off the dishwasher.</rdfs:comment>
        <rdfs:label xml:lang="en">Dish Washer Actuating Device</rdfs:label>
        <rdfs:isDefinedBy rdf:resource="http://purl.org/iot/vocab/m3-lite#"/>
    </owl:Class>



    <!-- http://purl.org/iot/vocab/iot-taxonomy-lite#Distance -->

    <owl:Class rdf:about="&iottaxolite;Distance">
        <rdfs:subClassOf rdf:resource="&sosa;ObservableProperty"/>
        <rdfs:comment xml:lang="en">Measure of how far apart objects are.</rdfs:comment>
        <rdfs:label xml:lang="en">Distance</rdfs:label>
        <rdfs:isDefinedBy rdf:resource="http://purl.org/iot/vocab/m3-lite#"/>
    </owl:Class>



    <!-- http://purl.org/iot/vocab/iot-taxonomy-lite#DistanceSensor -->

    <owl:Class rdf:about="&iottaxolite;DistanceSensor">
        <rdfs:subClassOf rdf:resource="&sosa;Sensor"/>
        <rdfs:comment xml:lang="en">Distance Sensor is used to detect distance between two objects for example:  the safety distance with other cars. Distance sensor can be a laser.</rdfs:comment>
        <rdfs:label xml:lang="en">Distance Sensor</rdfs:label>
        <rdfs:isDefinedBy rdf:resource="http://purl.org/iot/vocab/m3-lite#"/>
    </owl:Class>



    <!-- http://purl.org/iot/vocab/iot-taxonomy-lite#DomainOfInterest -->

    <owl:Class rdf:about="&iottaxolite;DomainOfInterest">
        <rdfs:comment xml:lang="en">Application Domain for example: health, environment, etc.</rdfs:comment>
        <rdfs:label xml:lang="en">Domain Of Interest</rdfs:label>
        <rdfs:isDefinedBy rdf:resource="http://purl.org/iot/vocab/m3-lite#"/>
    </owl:Class>



    <!-- http://purl.org/iot/vocab/iot-taxonomy-lite#Door -->

    <owl:Class rdf:about="&iottaxolite;Door">
        <rdfs:subClassOf rdf:resource="&sosa;Actuator"/>
        <rdfs:comment xml:lang="en">An actuator to automatically open/close the door.</rdfs:comment>
        <rdfs:label xml:lang="en">Door Actuating Device</rdfs:label>
        <rdfs:isDefinedBy rdf:resource="http://purl.org/iot/vocab/m3-lite#"/>
    </owl:Class>



    <!-- http://purl.org/iot/vocab/iot-taxonomy-lite#Drawer -->

    <owl:Class rdf:about="&iottaxolite;Drawer">
        <rdfs:subClassOf rdf:resource="&sosa;Actuator"/>
        <rdfs:comment xml:lang="en">An actuator to automatically open/close the drawer.</rdfs:comment>
        <rdfs:label xml:lang="en">Drawer Actuating Device</rdfs:label>
        <rdfs:isDefinedBy rdf:resource="http://purl.org/iot/vocab/m3-lite#"/>
    </owl:Class>



    <!-- http://purl.org/iot/vocab/iot-taxonomy-lite#EAQI -->

    <owl:Class rdf:about="&iottaxolite;EAQI">
        <rdfs:subClassOf rdf:resource="&qu;Unit"/>
        <rdfs:comment xml:lang="en">Unit to measure Air Quality in European cities.</rdfs:comment>
        <rdfs:label xml:lang="en">European Air Quality Index (EAQI)</rdfs:label>
        <rdfs:isDefinedBy rdf:resource="http://purl.org/iot/vocab/m3-lite#"/>
    </owl:Class>



    <!-- http://purl.org/iot/vocab/iot-taxonomy-lite#ECG -->

    <owl:Class rdf:about="&iottaxolite;ECG">
        <rdfs:subClassOf rdf:resource="&sosa;Sensor"/>
        <rdfs:comment xml:lang="en">ECG or EKG (Electrocardiogram) device.</rdfs:comment>
        <rdfs:label xml:lang="en">ECG or EKG (Electrocardiogram)</rdfs:label>
        <rdfs:isDefinedBy rdf:resource="http://purl.org/iot/vocab/m3-lite#"/>
    </owl:Class>



    <!-- http://purl.org/iot/vocab/iot-taxonomy-lite#ESP -->

    <owl:Class rdf:about="&iottaxolite;ESP">
        <rdfs:subClassOf rdf:resource="&sosa;Actuator"/>
        <rdfs:comment xml:lang="en">The actuator for turning ESP on/off.</rdfs:comment>
        <rdfs:label xml:lang="en">ESP (Electronic Stability Program) Actuating device</rdfs:label>
        <rdfs:isDefinedBy rdf:resource="http://purl.org/iot/vocab/m3-lite#"/>
    </owl:Class>



    <!-- http://purl.org/iot/vocab/iot-taxonomy-lite#ElectricCharge -->

    <owl:Class rdf:about="&iottaxolite;ElectricCharge">
        <rdfs:subClassOf rdf:resource="&sosa;ObservableProperty"/>
        <rdfs:comment xml:lang="en">It is the physical property of matter that causes it to experience a force when placed in an electromagnetic field. (Source Wikipedia).</rdfs:comment>
        <rdfs:label xml:lang="en">Electric Charge</rdfs:label>
        <rdfs:isDefinedBy rdf:resource="http://purl.org/iot/vocab/m3-lite#"/>
    </owl:Class>



    <!-- http://purl.org/iot/vocab/iot-taxonomy-lite#ElectricField -->

    <owl:Class rdf:about="&iottaxolite;ElectricField">
        <rdfs:subClassOf rdf:resource="&sosa;ObservableProperty"/>
        <rdfs:label xml:lang="en">Electric Field</rdfs:label>
        <rdfs:comment xml:lang="en">Electric field is the electric force per unit charge.</rdfs:comment>
        <rdfs:seeAlso>http://qudt.org/vocab/quantity#ElectricField</rdfs:seeAlso>
        <rdfs:isDefinedBy rdf:resource="http://purl.org/iot/vocab/m3-lite#"/>
    </owl:Class>



    <!-- http://purl.org/iot/vocab/iot-taxonomy-lite#ElectricField1800MHz -->

    <owl:Class rdf:about="&iottaxolite;ElectricField1800MHz">
        <rdfs:subClassOf rdf:resource="&iottaxolite;ElectricField"/>
        <rdfs:comment xml:lang="en">A field of force associated with a moving electric charge equivalent to an electric field and a magnetic field at right angles to each other and to the direction of propagation. Applied to the 1800 MHz UHF band.</rdfs:comment>
        <rdfs:label xml:lang="en">Electric Field 1800 MHz</rdfs:label>
        <rdfs:isDefinedBy rdf:resource="http://purl.org/iot/vocab/m3-lite#"/>
    </owl:Class>



    <!-- http://purl.org/iot/vocab/iot-taxonomy-lite#ElectricField2100MHz -->

    <owl:Class rdf:about="&iottaxolite;ElectricField2100MHz">
        <rdfs:subClassOf rdf:resource="&iottaxolite;ElectricField"/>
        <rdfs:comment xml:lang="en">A field of force associated with a moving electric charge equivalent to an electric field and a magnetic field at right angles to each other and to the direction of propagation. Applied to the 2100 MHz UHF band.</rdfs:comment>
        <rdfs:label xml:lang="en">Electric Field 2100 MHz</rdfs:label>
        <rdfs:isDefinedBy rdf:resource="http://purl.org/iot/vocab/m3-lite#"/>
    </owl:Class>



    <!-- http://purl.org/iot/vocab/iot-taxonomy-lite#ElectricField2400MHz -->

    <owl:Class rdf:about="&iottaxolite;ElectricField2400MHz">
        <rdfs:subClassOf rdf:resource="&iottaxolite;ElectricField"/>
        <rdfs:comment xml:lang="en">A field of force associated with a moving electric charge equivalent to an electric field and a magnetic field at right angles to each other and to the direction of propagation. Applied to the 2400 MHz UHF band.</rdfs:comment>
        <rdfs:label xml:lang="en">Electric Field 2400 MHz</rdfs:label>
        <rdfs:isDefinedBy rdf:resource="http://purl.org/iot/vocab/m3-lite#"/>
    </owl:Class>



    <!-- http://purl.org/iot/vocab/iot-taxonomy-lite#ElectricField900Mhz -->

    <owl:Class rdf:about="&iottaxolite;ElectricField900Mhz">
        <rdfs:subClassOf rdf:resource="&iottaxolite;ElectricField"/>
        <rdfs:comment xml:lang="en">A field of force associated with a moving electric charge equivalent to an electric field and a magnetic field at right angles to each other and to the direction of propagation. Applied to the 900 MHz UHF band.</rdfs:comment>
        <rdfs:label xml:lang="en">Electric Field 900 MHz</rdfs:label>
        <rdfs:isDefinedBy rdf:resource="http://purl.org/iot/vocab/m3-lite#"/>
    </owl:Class>



    <!-- http://purl.org/iot/vocab/iot-taxonomy-lite#ElectricPotential -->

    <owl:Class rdf:about="&iottaxolite;ElectricPotential">
        <rdfs:subClassOf rdf:resource="&sosa;ObservableProperty"/>
        <rdfs:comment xml:lang="en">Electric potential is the potential energy per unit charge associated with static (time-invariant) electric field.</rdfs:comment>
        <rdfs:label xml:lang="en">Electric Potential</rdfs:label>
        <rdfs:seeAlso>http://purl.oclc.org/NET/ssnx/qu/dim#ElectricPotential</rdfs:seeAlso>
        <rdfs:isDefinedBy rdf:resource="http://purl.org/iot/vocab/m3-lite#"/>
    </owl:Class>



    <!-- http://purl.org/iot/vocab/iot-taxonomy-lite#ElectricalResistance -->

    <owl:Class rdf:about="&iottaxolite;ElectricalResistance">
        <rdfs:subClassOf rdf:resource="&sosa;ObservableProperty"/>
        <rdfs:comment xml:lang="en">The electrical resistance of an electrical conductor is the opposition to the passage of an electric current through that conductor.</rdfs:comment>
        <rdfs:label xml:lang="en">Electrical Resistance</rdfs:label>
        <rdfs:isDefinedBy rdf:resource="http://purl.org/iot/vocab/m3-lite#"/>
    </owl:Class>



    <!-- http://purl.org/iot/vocab/iot-taxonomy-lite#ElectricalSensor -->

    <owl:Class rdf:about="&iottaxolite;ElectricalSensor">
        <rdfs:subClassOf rdf:resource="&sosa;Sensor"/>
        <rdfs:comment xml:lang="en">Sensor that measures the changes in electrical or magnetic signals based on an environmental input.</rdfs:comment>
        <rdfs:label xml:lang="en">Electrical Sensor</rdfs:label>
        <rdfs:isDefinedBy rdf:resource="http://purl.org/iot/vocab/m3-lite#"/>
    </owl:Class>



    <!-- http://purl.org/iot/vocab/iot-taxonomy-lite#Emotion -->

    <owl:Class rdf:about="&iottaxolite;Emotion">
        <rdfs:subClassOf rdf:resource="&iottaxolite;DomainOfInterest"/>
        <rdfs:comment xml:lang="en">Affective Science, Emotion, Mood, Emotional State, Brain Wave as an Internet of Things (IoT) applicative domain.</rdfs:comment>
        <rdfs:label xml:lang="en">Emotion DOI</rdfs:label>
        <rdfs:seeAlso rdf:resource="http://ns.inria.fr/emoca#Emotion"/>
        <rdfs:seeAlso rdf:resource="http://sensormeasurement.appspot.com/naturopathy#Emotion"/>
        <rdfs:isDefinedBy rdf:resource="http://purl.org/iot/vocab/m3-lite#"/>
    </owl:Class>



    <!-- http://purl.org/iot/vocab/iot-taxonomy-lite#Energy -->

    <owl:Class rdf:about="&iottaxolite;Energy">
        <rdfs:subClassOf rdf:resource="&sosa;ObservableProperty"/>
        <rdfs:comment xml:lang="en">Energy is the property that must be transferred to an object in order to perform work on. (Source Wikipedia).</rdfs:comment>
        <rdfs:label xml:lang="en">Energy</rdfs:label>
        <rdfs:isDefinedBy rdf:resource="http://purl.org/iot/vocab/m3-lite#"/>
    </owl:Class>



    <!-- http://purl.org/iot/vocab/iot-taxonomy-lite#EnergyDOI -->

    <owl:Class rdf:about="&iottaxolite;EnergyDOI">
        <rdfs:subClassOf rdf:resource="&iottaxolite;DomainOfInterest"/>
        <rdfs:comment xml:lang="en">Energy or Smart Grid as an Internet of Things (IoT) applicative domain.</rdfs:comment>
        <rdfs:label xml:lang="en">Energy DOI</rdfs:label>
        <rdfs:isDefinedBy rdf:resource="http://purl.org/iot/vocab/m3-lite#"/>
    </owl:Class>



    <!-- http://purl.org/iot/vocab/iot-taxonomy-lite#EnergyMeter -->

    <owl:Class rdf:about="&iottaxolite;EnergyMeter">
        <rdfs:subClassOf rdf:resource="&sosa;Sensor"/>
        <rdfs:comment xml:lang="en">Sensor to measure power or energy consumption.</rdfs:comment>
        <rdfs:label xml:lang="en">Energy Meter</rdfs:label>
        <rdfs:isDefinedBy rdf:resource="http://purl.org/iot/vocab/m3-lite#"/>
    </owl:Class>



    <!-- http://purl.org/iot/vocab/iot-taxonomy-lite#Environment -->

    <owl:Class rdf:about="&iottaxolite;Environment">
        <rdfs:subClassOf rdf:resource="&iottaxolite;DomainOfInterest"/>
        <rdfs:comment xml:lang="en">Environment (earthquake, flooding, fire, pollution) as an Internet of Things (IoT) applicative domain.</rdfs:comment>
        <rdfs:label xml:lang="en">Environment DOI</rdfs:label>
        <rdfs:isDefinedBy rdf:resource="http://purl.org/iot/vocab/m3-lite#"/>
    </owl:Class>



    <!-- http://purl.org/iot/vocab/iot-taxonomy-lite#Experiment -->

    <owl:Class rdf:about="&iottaxolite;Experiment">
        <rdfs:subClassOf rdf:resource="&iottaxolite;MeasurementType"/>
        <rdfs:comment xml:lang="en">Experiment based measurements.</rdfs:comment>
        <rdfs:label xml:lang="en">Experiment Measurement Type</rdfs:label>
        <rdfs:isDefinedBy rdf:resource="http://purl.org/iot/vocab/m3-lite#"/>
    </owl:Class>



    <!-- http://purl.org/iot/vocab/iot-taxonomy-lite#FallDetector -->

    <owl:Class rdf:about="&iottaxolite;FallDetector">
        <rdfs:subClassOf rdf:resource="&sosa;Sensor"/>
        <rdfs:comment xml:lang="en">Device to detect is a person has fallen.</rdfs:comment>
        <rdfs:label xml:lang="en">Fall Detector</rdfs:label>
        <rdfs:isDefinedBy rdf:resource="http://purl.org/iot/vocab/m3-lite#"/>
    </owl:Class>



    <!-- http://purl.org/iot/vocab/iot-taxonomy-lite#Fan -->

    <owl:Class rdf:about="&iottaxolite;Fan">
        <rdfs:subClassOf rdf:resource="&iottaxolite;SoundSource"/>
        <rdfs:comment xml:lang="en">When the source of the sound was Fan.</rdfs:comment>
        <rdfs:label xml:lang="en">Fan Sound Source</rdfs:label>
        <rdfs:isDefinedBy rdf:resource="http://purl.org/iot/vocab/m3-lite#"/>
    </owl:Class>



    <!-- http://purl.org/iot/vocab/iot-taxonomy-lite#Farad -->

    <owl:Class rdf:about="&iottaxolite;Farad">
        <rdfs:subClassOf rdf:resource="&qu;Unit"/>
        <rdfs:comment xml:lang="en">SI unit of electrical capacitance.</rdfs:comment>
        <rdfs:label xml:lang="en">Farad</rdfs:label>
        <rdfs:seeAlso rdf:resource="http://sweet.jpl.nasa.gov/ontology/units.owl#farad"/>
        <rdfs:isDefinedBy rdf:resource="http://purl.org/iot/vocab/m3-lite#"/>
    </owl:Class>



    <!-- http://purl.org/iot/vocab/iot-taxonomy-lite#FillLevel -->

    <owl:Class rdf:about="&iottaxolite;FillLevel">
        <rdfs:subClassOf rdf:resource="&sosa;ObservableProperty"/>
        <rdfs:label xml:lang="en">Fill Level</rdfs:label>
        <rdfs:comment xml:lang="en">Property used to determine the level a certain object such as waste bin is filled upto.</rdfs:comment>
        <rdfs:isDefinedBy rdf:resource="http://purl.org/iot/vocab/m3-lite#"/>
    </owl:Class>



    <!-- http://purl.org/iot/vocab/iot-taxonomy-lite#FillLevelGasTank -->

    <owl:Class rdf:about="&iottaxolite;FillLevelGasTank">
        <rdfs:subClassOf rdf:resource="&iottaxolite;FillLevel"/>
        <rdfs:comment xml:lang="en">Ratio of volume of combustible exhaust fluid to the total volume of diesel exhaust fluid storage container.</rdfs:comment>
        <rdfs:label xml:lang="en">Fill Level Gas Tank</rdfs:label>
        <rdfs:isDefinedBy rdf:resource="http://purl.org/iot/vocab/m3-lite#"/>
    </owl:Class>



    <!-- http://purl.org/iot/vocab/iot-taxonomy-lite#FillLevelGasTankOne -->

    <owl:Class rdf:about="&iottaxolite;FillLevelGasTankOne">
        <rdfs:subClassOf rdf:resource="&iottaxolite;FillLevelGasTank"/>
        <rdfs:comment xml:lang="en">Ratio of volume of combustible exhaust fluid to the total volume of diesel exhaust fluid storage container. This is the value for the primary tank of the vehicle.</rdfs:comment>
        <rdfs:label xml:lang="en">Fill Level Gas Tank 1</rdfs:label>
        <rdfs:isDefinedBy rdf:resource="http://purl.org/iot/vocab/m3-lite#"/>
    </owl:Class>



    <!-- http://purl.org/iot/vocab/iot-taxonomy-lite#FillLevelGasTankTwo -->

    <owl:Class rdf:about="&iottaxolite;FillLevelGasTankTwo">
        <rdfs:subClassOf rdf:resource="&iottaxolite;FillLevelGasTank"/>
        <rdfs:comment xml:lang="en">Ratio of volume of combustible exhaust fluid to the total volume of diesel exhaust fluid storage container. This is the value for the secondary tank of the vehicle.</rdfs:comment>
        <rdfs:label xml:lang="en">Fill Level Gas Tank 2</rdfs:label>
        <rdfs:isDefinedBy rdf:resource="http://purl.org/iot/vocab/m3-lite#"/>
    </owl:Class>



    <!-- http://purl.org/iot/vocab/iot-taxonomy-lite#FillLevelWasteContainer -->

    <owl:Class rdf:about="&iottaxolite;FillLevelWasteContainer">
        <rdfs:subClassOf rdf:resource="&iottaxolite;FillLevel"/>
        <rdfs:comment xml:lang="en">Ratio between the current filleage level and the total capacity of a waste container.</rdfs:comment>
        <rdfs:label xml:lang="en">Fill Level Waste Container</rdfs:label>
        <rdfs:isDefinedBy rdf:resource="http://purl.org/iot/vocab/m3-lite#"/>
    </owl:Class>



    <!-- http://purl.org/iot/vocab/iot-taxonomy-lite#FogLamp -->

    <owl:Class rdf:about="&iottaxolite;FogLamp">
        <rdfs:subClassOf rdf:resource="&sosa;Actuator"/>
        <rdfs:comment xml:lang="en">The actuator for turning on or off the fog lamp.</rdfs:comment>
        <rdfs:label xml:lang="en">Fog Lamp Actuating Device</rdfs:label>
        <rdfs:isDefinedBy rdf:resource="http://purl.org/iot/vocab/m3-lite#"/>
    </owl:Class>




    <!-- http://purl.org/iot/vocab/iot-taxonomy-lite#FoodTemperature -->

    <owl:Class rdf:about="&iottaxolite;FoodTemperature">
        <rdfs:subClassOf rdf:resource="&iottaxolite;Temperature"/>
        <rdfs:comment xml:lang="en">Measure of temperature of the food.</rdfs:comment>
        <rdfs:label xml:lang="en">Food Temperature</rdfs:label>
        <rdfs:isDefinedBy rdf:resource="http://purl.org/iot/vocab/m3-lite#"/>
    </owl:Class>



    <!-- http://purl.org/iot/vocab/iot-taxonomy-lite#Freezer -->

    <owl:Class rdf:about="&iottaxolite;Freezer">
        <rdfs:subClassOf rdf:resource="&sosa;Actuator"/>
        <rdfs:comment xml:lang="en">An actuator to automatically open/close the freezer.</rdfs:comment>
        <rdfs:label xml:lang="en">Freezer, Chiller Actuating Device</rdfs:label>
        <rdfs:isDefinedBy rdf:resource="http://purl.org/iot/vocab/m3-lite#"/>
    </owl:Class>



    <!-- http://purl.org/iot/vocab/iot-taxonomy-lite#Frequency -->

    <owl:Class rdf:about="&iottaxolite;Frequency">
        <rdfs:subClassOf rdf:resource="&sosa;ObservableProperty"/>
        <rdfs:comment xml:lang="en">Frequency is the number of occurrences of a repeating event per unit time.</rdfs:comment>
        <rdfs:label xml:lang="en">Frequency</rdfs:label>
        <rdfs:isDefinedBy rdf:resource="http://purl.org/iot/vocab/m3-lite#"/>
    </owl:Class>



    <!-- http://purl.org/iot/vocab/iot-taxonomy-lite#FrequencySensor -->

    <owl:Class rdf:about="&iottaxolite;FrequencySensor">
        <rdfs:subClassOf rdf:resource="&sosa;Sensor"/>
        <rdfs:comment xml:lang="en">Device used to detect the frequency.</rdfs:comment>
        <rdfs:label xml:lang="en">Frequency Sensor</rdfs:label>
        <rdfs:isDefinedBy rdf:resource="http://purl.org/iot/vocab/m3-lite#"/>
    </owl:Class>



    <!-- http://purl.org/iot/vocab/iot-taxonomy-lite#Fridge -->

    <owl:Class rdf:about="&iottaxolite;Fridge">
        <rdfs:subClassOf rdf:resource="&sosa;Actuator"/>
        <rdfs:comment xml:lang="en">An actuator to automatically switch on/off the fridge.</rdfs:comment>
        <rdfs:label xml:lang="en">Fridge, Refrigerator Actuating Device</rdfs:label>
        <rdfs:isDefinedBy rdf:resource="http://purl.org/iot/vocab/m3-lite#"/>
    </owl:Class>



    <!-- http://purl.org/iot/vocab/iot-taxonomy-lite#FuelConsumption -->

    <owl:Class rdf:about="&iottaxolite;FuelConsumption">
        <rdfs:subClassOf rdf:resource="&sosa;ObservableProperty"/>
        <rdfs:label xml:lang="en">Fuel Consumption Quantity Kind</rdfs:label>
        <rdfs:comment xml:lang="en">The amount of fuel a vehicle uses to travel a particular distance at a particular speed.</rdfs:comment>
        <rdfs:isDefinedBy rdf:resource="http://purl.org/iot/vocab/m3-lite#"/>
    </owl:Class>



    <!-- http://purl.org/iot/vocab/iot-taxonomy-lite#FuelConsumptionInstantaneous -->

    <owl:Class rdf:about="&iottaxolite;FuelConsumptionInstantaneous">
        <rdfs:subClassOf rdf:resource="&iottaxolite;FuelConsumption"/>
        <rdfs:comment xml:lang="en">A measure that displays the instantaneous fuel consumption of a vehicle during its operation.</rdfs:comment>
        <rdfs:label xml:lang="en">Fuel Consumption Instantaneous</rdfs:label>
        <rdfs:isDefinedBy rdf:resource="http://purl.org/iot/vocab/m3-lite#"/>
    </owl:Class>



    <!-- http://purl.org/iot/vocab/iot-taxonomy-lite#FuelConsumptionTotal -->

    <owl:Class rdf:about="&iottaxolite;FuelConsumptionTotal">
        <rdfs:subClassOf rdf:resource="&iottaxolite;FuelConsumption"/>
        <rdfs:comment xml:lang="en">Accumulated amount of fuel used during vehicle operation.</rdfs:comment>
        <rdfs:label xml:lang="en">Fuel Consumption Total</rdfs:label>
        <rdfs:isDefinedBy rdf:resource="http://purl.org/iot/vocab/m3-lite#"/>
    </owl:Class>



    <!-- http://purl.org/iot/vocab/iot-taxonomy-lite#FuelLevel -->

    <owl:Class rdf:about="&iottaxolite;FuelLevel">
        <rdfs:subClassOf rdf:resource="&sosa;Sensor"/>
        <rdfs:comment xml:lang="en">Device used to detect fuel level in a system such a car.</rdfs:comment>
        <rdfs:label xml:lang="en">Fuel Level Sensor</rdfs:label>
        <rdfs:isDefinedBy rdf:resource="http://purl.org/iot/vocab/m3-lite#"/>
    </owl:Class>



    <!-- http://purl.org/iot/vocab/iot-taxonomy-lite#GPSSensor -->

    <owl:Class rdf:about="&iottaxolite;GPSSensor">
        <rdfs:subClassOf rdf:resource="&sosa;Sensor"/>
        <rdfs:comment xml:lang="en">Device that allows an object to localize itself.</rdfs:comment>
        <rdfs:label xml:lang="en">GPS Sensor</rdfs:label>
        <rdfs:isDefinedBy rdf:resource="http://purl.org/iot/vocab/m3-lite#"/>
    </owl:Class>



    <!-- http://purl.org/iot/vocab/iot-taxonomy-lite#GasDetector -->

    <owl:Class rdf:about="&iottaxolite;GasDetector">
        <rdfs:subClassOf rdf:resource="&sosa;Sensor"/>
        <rdfs:comment xml:lang="en">Device that detects the presence of gases in an area, often as part of a safety system.</rdfs:comment>
        <rdfs:label xml:lang="en">Gas Detector</rdfs:label>
        <rdfs:isDefinedBy rdf:resource="http://purl.org/iot/vocab/m3-lite#"/>
    </owl:Class>



    <!-- http://purl.org/iot/vocab/iot-taxonomy-lite#GaseousPollutantSensor -->

    <owl:Class rdf:about="&iottaxolite;GaseousPollutantSensor">
        <rdfs:subClassOf rdf:resource="&iottaxolite;AirPollutantSensor"/>
        <rdfs:comment xml:lang="en">Device used to detect poisonous gaseous in the environment.</rdfs:comment>
        <rdfs:label xml:lang="en">Gaseous Pollutant Sensor</rdfs:label>
        <rdfs:isDefinedBy rdf:resource="http://purl.org/iot/vocab/m3-lite#"/>
    </owl:Class>



    <!-- http://purl.org/iot/vocab/iot-taxonomy-lite#Gauss -->

    <owl:Class rdf:about="&iottaxolite;Gauss">
        <rdfs:subClassOf rdf:resource="&qu;Unit"/>
        <rdfs:comment xml:lang="en">Gauss is the CGS unit of measurement of magnetic flux density (or magnetic induction) (B) (Source Wikipedia)</rdfs:comment>
        <rdfs:label xml:lang="en">Gauss</rdfs:label>
        <rdfs:isDefinedBy rdf:resource="http://purl.org/iot/vocab/m3-lite#"/>
    </owl:Class>



    <!-- http://purl.org/iot/vocab/iot-taxonomy-lite#Glucometer -->

    <owl:Class rdf:about="&iottaxolite;Glucometer">
        <rdfs:subClassOf rdf:resource="&sosa;Sensor"/>
        <rdfs:comment xml:lang="en">Device used to detect glucometer, blood sugar, blood glucose level.</rdfs:comment>
        <rdfs:label xml:lang="en">Glucometer Sensor</rdfs:label>
        <rdfs:isDefinedBy rdf:resource="http://purl.org/iot/vocab/m3-lite#"/>
    </owl:Class>



    <!-- http://purl.org/iot/vocab/iot-taxonomy-lite#Gram -->

    <owl:Class rdf:about="&iottaxolite;Gram">
        <rdfs:subClassOf rdf:resource="&qu;Unit"/>
        <rdfs:label>Gram (g)</rdfs:label>
        <rdfs:comment>It is a metric system unit of mass</rdfs:comment>
        <rdfs:isDefinedBy rdf:resource="http://purl.org/iot/vocab/m3-lite#"/>
    </owl:Class>



    <!-- http://purl.org/iot/vocab/iot-taxonomy-lite#GramPerCubicMetre -->

    <owl:Class rdf:about="&iottaxolite;GramPerCubicMetre">
        <rdfs:subClassOf rdf:resource="&qu;Unit"/>
        <rdfs:comment xml:lang="en">It is defined by mass in grams divided by volume in cubic metres.</rdfs:comment>
        <rdfs:label xml:lang="en">Gram Per Cubic Metre, Gram Per Cubic Meter</rdfs:label>
        <rdfs:isDefinedBy rdf:resource="http://purl.org/iot/vocab/m3-lite#"/>
    </owl:Class>



    <!-- http://purl.org/iot/vocab/iot-taxonomy-lite#GramPerLitre -->

    <owl:Class rdf:about="&iottaxolite;GramPerLitre">
        <rdfs:subClassOf rdf:resource="&qu;Unit"/>
        <rdfs:comment xml:lang="en">It shows how many grams of a certain substance are present in one litre of a usually liquid or gaseous mixture.</rdfs:comment>
        <rdfs:label xml:lang="en">Gram Per Litre, Gram Per Liter (g/L)</rdfs:label>
        <rdfs:isDefinedBy rdf:resource="http://purl.org/iot/vocab/m3-lite#"/>
    </owl:Class>



    <!-- http://purl.org/iot/vocab/iot-taxonomy-lite#GyrometerSensor -->

    <owl:Class rdf:about="&iottaxolite;GyrometerSensor">
        <rdfs:subClassOf rdf:resource="&sosa;Sensor"/>
        <rdfs:comment xml:lang="en">A gyrometer is an instrument which measures an angular speed.</rdfs:comment>
        <rdfs:label xml:lang="en">Gyrometer Sensor</rdfs:label>
        <rdfs:isDefinedBy rdf:resource="http://purl.org/iot/vocab/m3-lite#"/>
    </owl:Class>



    <!-- http://purl.org/iot/vocab/iot-taxonomy-lite#GyroscopeSensor -->

    <owl:Class rdf:about="&iottaxolite;GyroscopeSensor">
        <rdfs:subClassOf rdf:resource="&sosa;Sensor"/>
        <rdfs:comment xml:lang="en">A gyroscope is a device for measuring or maintaining orientation.</rdfs:comment>
        <rdfs:label xml:lang="en">Gyroscope Sensor</rdfs:label>
        <rdfs:seeAlso rdf:resource="http://casas.wsu.edu/owl/cose.owl#Gyroscope"/>
        <rdfs:isDefinedBy rdf:resource="http://purl.org/iot/vocab/m3-lite#"/>
    </owl:Class>



    <!-- http://purl.org/iot/vocab/iot-taxonomy-lite#H2SSensor -->

    <owl:Class rdf:about="&iottaxolite;H2SSensor">
        <rdfs:subClassOf rdf:resource="&iottaxolite;GaseousPollutantSensor"/>
        <rdfs:comment xml:lang="en">Device used to measure of hydrogen sulphide in the environment.</rdfs:comment>
        <rdfs:label xml:lang="en">H2S Sensor</rdfs:label>
        <rdfs:isDefinedBy rdf:resource="http://purl.org/iot/vocab/m3-lite#"/>
    </owl:Class>



    <!-- http://purl.org/iot/vocab/iot-taxonomy-lite#Health -->

    <owl:Class rdf:about="&iottaxolite;Health">
        <rdfs:subClassOf rdf:resource="&iottaxolite;DomainOfInterest"/>
        <rdfs:comment xml:lang="en">Healthcare as an Internet of Things (IoT) applicative domain.</rdfs:comment>
        <rdfs:label xml:lang="en">Health Care DOI</rdfs:label>
        <rdfs:isDefinedBy rdf:resource="http://purl.org/iot/vocab/m3-lite#"/>
    </owl:Class>



    <!-- http://purl.org/iot/vocab/iot-taxonomy-lite#HeartBeat -->

    <owl:Class rdf:about="&iottaxolite;HeartBeat">
        <rdfs:subClassOf rdf:resource="&sosa;ObservableProperty"/>
        <rdfs:comment xml:lang="en">The number of times your heart beats each minute (bpm).</rdfs:comment>
        <rdfs:label xml:lang="en">Heart Beat</rdfs:label>
        <rdfs:isDefinedBy rdf:resource="http://purl.org/iot/vocab/m3-lite#"/>
    </owl:Class>



    <!-- http://purl.org/iot/vocab/iot-taxonomy-lite#HeartBeatSensor -->

    <owl:Class rdf:about="&iottaxolite;HeartBeatSensor">
        <rdfs:subClassOf rdf:resource="&sosa;Sensor"/>
        <rdfs:comment xml:lang="en">Device to count heart beats per minute.</rdfs:comment>
        <rdfs:label xml:lang="en">Heart Beat Sensor</rdfs:label>
        <rdfs:isDefinedBy rdf:resource="http://purl.org/iot/vocab/m3-lite#"/>
    </owl:Class>



    <!-- http://purl.org/iot/vocab/iot-taxonomy-lite#Heating -->

    <owl:Class rdf:about="&iottaxolite;Heating">
        <rdfs:subClassOf rdf:resource="&sosa;Actuator"/>
        <rdfs:comment xml:lang="en">An actuator to automatically switch on/off the heating.</rdfs:comment>
        <rdfs:label xml:lang="en">Heating Actuating Device</rdfs:label>
        <rdfs:isDefinedBy rdf:resource="http://purl.org/iot/vocab/m3-lite#"/>
    </owl:Class>



    <!-- http://purl.org/iot/vocab/iot-taxonomy-lite#Hertz -->

    <owl:Class rdf:about="&iottaxolite;Hertz">
        <rdfs:subClassOf rdf:resource="&qu;Unit"/>
        <rdfs:comment xml:lang="en">The SI unit of frequency, equal to one cycle per second.</rdfs:comment>
        <rdfs:label xml:lang="en">Hertz</rdfs:label>
        <rdfs:isDefinedBy rdf:resource="http://purl.org/iot/vocab/m3-lite#"/>
    </owl:Class>



    <!-- http://purl.org/iot/vocab/iot-taxonomy-lite#Hour -->

    <owl:Class rdf:about="&iottaxolite;Hour">
        <rdfs:subClassOf rdf:resource="&iottaxolite;SecondTime"/>
        <rdfs:comment xml:lang="en">Hour of the day.</rdfs:comment>
        <rdfs:label xml:lang="en">Hour</rdfs:label>
        <rdfs:seeAlso rdf:resource="http://sweet.jpl.nasa.gov/ontology/units.owl#hour"/>
        <rdfs:isDefinedBy rdf:resource="http://purl.org/iot/vocab/m3-lite#"/>
    </owl:Class>



    <!-- http://purl.org/iot/vocab/iot-taxonomy-lite#HouseholdApplianceTemperature -->

    <owl:Class rdf:about="&iottaxolite;HouseholdApplianceTemperature">
        <rdfs:subClassOf rdf:resource="&iottaxolite;Temperature"/>
        <rdfs:comment xml:lang="en">Measure of Household Appliance Temperature.</rdfs:comment>
        <rdfs:label xml:lang="en">Household Appliance Temperature</rdfs:label>
        <rdfs:isDefinedBy rdf:resource="http://purl.org/iot/vocab/m3-lite#"/>
    </owl:Class>



    <!-- http://purl.org/iot/vocab/iot-taxonomy-lite#Humidity -->

    <owl:Class rdf:about="&iottaxolite;Humidity">
        <rdfs:subClassOf rdf:resource="&sosa;ObservableProperty"/>
        <rdfs:comment xml:lang="en">A quantity representing the amount of water vapour in the atmosphere or in a gas.</rdfs:comment>
        <rdfs:label xml:lang="en">Humidity</rdfs:label>
        <rdfs:seeAlso rdf:resource="http://elite.polito.it/ontologies/dogont.owl#HumidityMeasurementMNotification"/>
        <rdfs:seeAlso rdf:resource="http://openiot.eu/ontology/ns/AtmosphereHumidity"/>
        <rdfs:seeAlso rdf:resource="http://paul.staroch.name/thesis/SmartHomeWeather.owl#Humidity"/>
        <rdfs:isDefinedBy rdf:resource="http://purl.org/iot/vocab/m3-lite#"/>
    </owl:Class>



    <!-- http://purl.org/iot/vocab/iot-taxonomy-lite#HumiditySensor -->

    <owl:Class rdf:about="&iottaxolite;HumiditySensor">
        <rdfs:subClassOf rdf:resource="&sosa;Sensor"/>
        <rdfs:comment xml:lang="en">Humidity sensor or hygrometer is an instrument used for measuring the moisture concent in the environment.</rdfs:comment>
        <rdfs:label xml:lang="en">Humidity Sensor</rdfs:label>
        <rdfs:seeAlso rdf:resource="http://purl.oclc.org/NET/ssnx/meteo/aws#HumiditySensor"/>
        <rdfs:isDefinedBy rdf:resource="http://purl.org/iot/vocab/m3-lite#"/>
    </owl:Class>



    <!-- http://purl.org/iot/vocab/iot-taxonomy-lite#Hydrophone -->

    <owl:Class rdf:about="&iottaxolite;Hydrophone">
        <rdfs:subClassOf rdf:resource="&sosa;Sensor"/>
        <rdfs:comment xml:lang="en">A hydrophone is a microphone designed to be used underwater for recording or listening to underwater sound.</rdfs:comment>
        <rdfs:label xml:lang="en">Hydrophone</rdfs:label>
        <rdfs:isDefinedBy rdf:resource="http://purl.org/iot/vocab/m3-lite#"/>
    </owl:Class>



    <!-- http://purl.org/iot/vocab/iot-taxonomy-lite#Illuminance -->

    <owl:Class rdf:about="&iottaxolite;Illuminance">
        <rdfs:subClassOf rdf:resource="&sosa;ObservableProperty"/>
        <rdfs:comment xml:lang="en">Illuminance is the total luminous flux incident on a surface, per unit area.</rdfs:comment>
        <rdfs:label xml:lang="en">Illuminance</rdfs:label>
        <rdfs:isDefinedBy rdf:resource="http://purl.org/iot/vocab/m3-lite#"/>
    </owl:Class>



    <!-- http://purl.org/iot/vocab/iot-taxonomy-lite#ImageSensor -->

    <owl:Class rdf:about="&iottaxolite;ImageSensor">
        <rdfs:subClassOf rdf:resource="&sosa;Sensor"/>
        <rdfs:comment xml:lang="en">Sensor that detects and conveys the information that constitutes an image.</rdfs:comment>
        <rdfs:label xml:lang="en">Image Sensor</rdfs:label>
        <rdfs:isDefinedBy rdf:resource="http://purl.org/iot/vocab/m3-lite#"/>
    </owl:Class>



    <!-- http://purl.org/iot/vocab/iot-taxonomy-lite#Inch -->

    <owl:Class rdf:about="&iottaxolite;Inch">
        <rdfs:subClassOf rdf:resource="&iottaxolite;Metre"/>
        <rdfs:comment xml:lang="en">Length in inches.</rdfs:comment>
        <rdfs:label xml:lang="en">Inch</rdfs:label>
        <rdfs:isDefinedBy rdf:resource="http://purl.org/iot/vocab/m3-lite#"/>
    </owl:Class>



    <!-- http://purl.org/iot/vocab/iot-taxonomy-lite#Index -->

    <owl:Class rdf:about="&iottaxolite;Index">
        <rdfs:subClassOf rdf:resource="&qu;Unit"/>
        <rdfs:comment xml:lang="en">Arbitrary indirect reference which should be translated into meaningful measurements by using the corresponding decoding algorithm detailed in the resource description. In this case the returned values can only take certain values from a finite set.</rdfs:comment>
        <rdfs:label xml:lang="en">Index</rdfs:label>
        <rdfs:isDefinedBy rdf:resource="http://purl.org/iot/vocab/m3-lite#"/>
    </owl:Class>



    <!-- http://purl.org/iot/vocab/iot-taxonomy-lite#IntDlLatency -->

    <owl:Class rdf:about="&iottaxolite;IntDlLatency">
        <rdfs:subClassOf rdf:resource="&iottaxolite;Communication"/>
        <rdfs:comment xml:lang="en">Downlink Latency.</rdfs:comment>
        <rdfs:label xml:lang="en">Downlink Latency</rdfs:label>
        <rdfs:isDefinedBy rdf:resource="http://purl.org/iot/vocab/m3-lite#"/>
    </owl:Class>



    <!-- http://purl.org/iot/vocab/iot-taxonomy-lite#Invalid -->

    <owl:Class rdf:about="&iottaxolite;Invalid">
        <rdfs:subClassOf rdf:resource="&iottaxolite;MeasurementType"/>
        <rdfs:comment xml:lang="en">If the measurement was tagged invalid.</rdfs:comment>
        <rdfs:label xml:lang="en">Invalid Measurement Type</rdfs:label>
        <rdfs:isDefinedBy rdf:resource="http://purl.org/iot/vocab/m3-lite#"/>
    </owl:Class>



    <!-- http://purl.org/iot/vocab/iot-taxonomy-lite#Irrigation -->

    <owl:Class rdf:about="&iottaxolite;Irrigation">
        <rdfs:subClassOf rdf:resource="&sosa;Actuator"/>
        <rdfs:comment xml:lang="en">An actuator to automatically irrigate.</rdfs:comment>
        <rdfs:label xml:lang="en">Irrigation Actuation Device</rdfs:label>
        <rdfs:isDefinedBy rdf:resource="http://purl.org/iot/vocab/m3-lite#"/>
    </owl:Class>



    <!-- http://purl.org/iot/vocab/iot-taxonomy-lite#Kelvin -->

    <owl:Class rdf:about="&iottaxolite;Kelvin">
        <rdfs:subClassOf rdf:resource="&qu;Unit"/>
        <rdfs:comment xml:lang="en">Kelvin is a unit of measurement for temperature.</rdfs:comment>
        <rdfs:label xml:lang="en">Kelvin, Degree Kelvin</rdfs:label>
        <rdfs:seeAlso rdf:resource="http://sweet.jpl.nasa.gov/ontology/units.owl#kelvin"/>
        <rdfs:isDefinedBy rdf:resource="http://purl.org/iot/vocab/m3-lite#"/>
    </owl:Class>



    <!-- http://purl.org/iot/vocab/iot-taxonomy-lite#KiloWattHour -->

    <owl:Class rdf:about="&iottaxolite;KiloWattHour">
        <rdfs:subClassOf rdf:resource="&qu;Unit"/>
        <rdfs:comment xml:lang="en">Measure of electrical energy equivalent to a power consumption of one thousand watts for one hour.</rdfs:comment>
        <rdfs:label xml:lang="en">Kilo Watt Hour</rdfs:label>
        <rdfs:seeAlso rdf:resource="&qudt;KiloWatthour"/>
        <rdfs:isDefinedBy rdf:resource="http://purl.org/iot/vocab/m3-lite#"/>
    </owl:Class>



    <!-- http://purl.org/iot/vocab/iot-taxonomy-lite#KilobitsPerSecond -->

    <owl:Class rdf:about="&iottaxolite;KilobitsPerSecond">
        <rdfs:subClassOf rdf:resource="&qu;Unit"/>
        <rdfs:comment xml:lang="en">It is a unit of data transfer rate equal to: 1,000 bits per second.</rdfs:comment>
        <rdfs:label xml:lang="en">Kilobits Per Second</rdfs:label>
        <rdfs:isDefinedBy rdf:resource="http://purl.org/iot/vocab/m3-lite#"/>
    </owl:Class>



    <!-- http://purl.org/iot/vocab/iot-taxonomy-lite#Kilogram -->

    <owl:Class rdf:about="&iottaxolite;Kilogram">
        <rdfs:subClassOf rdf:resource="&iottaxolite;Gram"/>
        <rdfs:comment xml:lang="en">The SI unit of mass, it is equal to the mass of the international prototype of the kilogram.</rdfs:comment>
        <rdfs:label xml:lang="en">Kilogram (kg)</rdfs:label>
        <rdfs:seeAlso>http://purl.oclc.org/NET/ssnx/qu/unit#kilogram</rdfs:seeAlso>
        <rdfs:isDefinedBy rdf:resource="http://purl.org/iot/vocab/m3-lite#"/>
    </owl:Class>



    <!-- http://purl.org/iot/vocab/iot-taxonomy-lite#KilogramPerCubicMetre -->

    <owl:Class rdf:about="&iottaxolite;KilogramPerCubicMetre">
        <rdfs:subClassOf rdf:resource="&iottaxolite;GramPerCubicMetre"/>
        <rdfs:label xml:lang="en">Kilogram Per Cubic Metre, Kilogram Per Cubic Meter</rdfs:label>
        <rdfs:comment xml:lang="en">It is SI derived unit of density, defined by mass in kilograms divided by volume in cubic metres.</rdfs:comment>
        <rdfs:isDefinedBy rdf:resource="http://purl.org/iot/vocab/m3-lite#"/>
    </owl:Class>



    <!-- http://purl.org/iot/vocab/iot-taxonomy-lite#KilometrePerHour -->

    <owl:Class rdf:about="&iottaxolite;KilometrePerHour">
        <rdfs:subClassOf rdf:resource="&iottaxolite;MetrePerSecond"/>
        <rdfs:label xml:lang="en">Kilometre Per Hour, Kilometer Per Hour</rdfs:label>
        <rdfs:comment xml:lang="en">It is a unit of speed, expressing the number of kilometres travelled in one hour.</rdfs:comment>
        <rdfs:seeAlso>http://data.qudt.org/qudt/owl/1.0.0/unit.owl#KilometerPerHour</rdfs:seeAlso>
        <rdfs:isDefinedBy rdf:resource="http://purl.org/iot/vocab/m3-lite#"/>
    </owl:Class>



    <!-- http://purl.org/iot/vocab/iot-taxonomy-lite#Kilometre -->

    <owl:Class rdf:about="&iottaxolite;Kilometre">
        <rdfs:subClassOf rdf:resource="&iottaxolite;Metre"/>
        <rdfs:label xml:lang="en">Kilometre, Kilometer</rdfs:label>
        <rdfs:comment xml:lang="en">A metric unit of measurement equal to 1,000 metres (approx 0.62 miles).</rdfs:comment>
        <rdfs:isDefinedBy rdf:resource="http://purl.org/iot/vocab/m3-lite#"/>
    </owl:Class>



    <!-- http://purl.org/iot/vocab/iot-taxonomy-lite#Lamp -->

    <owl:Class rdf:about="&iottaxolite;Lamp">
        <rdfs:subClassOf rdf:resource="&sosa;Actuator"/>
        <rdfs:comment xml:lang="en">An actuator to automatically switch on/off the lamp.</rdfs:comment>
        <rdfs:label xml:lang="en">Lamp Actuating Device</rdfs:label>
        <rdfs:isDefinedBy rdf:resource="http://purl.org/iot/vocab/m3-lite#"/>
    </owl:Class>



    <!-- http://purl.org/iot/vocab/iot-taxonomy-lite#Lavatory -->

    <owl:Class rdf:about="&iottaxolite;Lavatory">
        <rdfs:subClassOf rdf:resource="&sosa;Actuator"/>
        <rdfs:comment xml:lang="en">An actuator to automatically switch on/off the lavatory.</rdfs:comment>
        <rdfs:label xml:lang="en">Lavatory Actuating Device</rdfs:label>
        <rdfs:isDefinedBy rdf:resource="http://purl.org/iot/vocab/m3-lite#"/>
    </owl:Class>



    <!-- http://purl.org/iot/vocab/iot-taxonomy-lite#LeafWetness -->

    <owl:Class rdf:about="&iottaxolite;LeafWetness">
        <rdfs:subClassOf rdf:resource="&sosa;ObservableProperty"/>
        <rdfs:comment xml:lang="en">Leaf wetness is a meteorological parameter that describes the amount of dew and precipitation left on surfaces. It is used for monitoring leaf moisture for agricultural purposes, such as fungus and disease control, for control of irrigation systems, and for detection of fog and dew conditions, and early detection of rainfall. (Source Wikipedia).</rdfs:comment>
        <rdfs:label xml:lang="en">Leaf Wetness</rdfs:label>
        <rdfs:isDefinedBy rdf:resource="http://purl.org/iot/vocab/m3-lite#"/>
    </owl:Class>



    <!-- http://purl.org/iot/vocab/iot-taxonomy-lite#LeafWetnessSensor -->

    <owl:Class rdf:about="&iottaxolite;LeafWetnessSensor">
        <rdfs:subClassOf rdf:resource="&sosa;Sensor"/>
        <rdfs:comment xml:lang="en">Leaf Wetness Sensor is used in agriculture to check whether the plants need to be watered.</rdfs:comment>
        <rdfs:label xml:lang="en">Leaf Wetness Sensor</rdfs:label>
        <rdfs:isDefinedBy rdf:resource="http://purl.org/iot/vocab/m3-lite#"/>
    </owl:Class>



    <!-- http://purl.org/iot/vocab/iot-taxonomy-lite#LightSensor -->

    <owl:Class rdf:about="&iottaxolite;LightSensor">
        <rdfs:subClassOf rdf:resource="&sosa;Sensor"/>
        <rdfs:comment xml:lang="en">Light/Illuminance Sensor is used to adjust the brightness of the surface.</rdfs:comment>
        <rdfs:label xml:lang="en">Light Sensor</rdfs:label>
        <rdfs:isDefinedBy rdf:resource="http://purl.org/iot/vocab/m3-lite#"/>
    </owl:Class>



    <!-- http://purl.org/iot/vocab/iot-taxonomy-lite#Litre -->

    <owl:Class rdf:about="&iottaxolite;Litre">
        <rdfs:subClassOf rdf:resource="&qu;Unit"/>
        <rdfs:comment xml:lang="en">A metric unit of capacity defined as the volume of one kilogram of water under standard conditions. It is equal to 1,000 cubic centimetres.</rdfs:comment>
        <rdfs:label xml:lang="en">Litre, Liter</rdfs:label>
        <rdfs:seeAlso>http://purl.oclc.org/NET/ssnx/qu/unit#litre</rdfs:seeAlso>
        <rdfs:isDefinedBy rdf:resource="http://purl.org/iot/vocab/m3-lite#"/>
    </owl:Class>



    <!-- http://purl.org/iot/vocab/iot-taxonomy-lite#LitrePer100Kilometres -->

    <owl:Class rdf:about="&iottaxolite;LitrePer100Kilometres">
        <rdfs:subClassOf rdf:resource="&qu;Unit"/>
        <rdfs:comment xml:lang="en">A consumption unit which is equal to the one of a vehicle which needs 1 fuel litre in order to traverse 100 kilometres.</rdfs:comment>
        <rdfs:label xml:lang="en">Litre Per 100 Kilometres, Liter Per 100 Kilometers</rdfs:label>
        <rdfs:isDefinedBy rdf:resource="http://purl.org/iot/vocab/m3-lite#"/>
    </owl:Class>



    <!-- http://purl.org/iot/vocab/iot-taxonomy-lite#LocationQK -->

    <owl:Class rdf:about="&iottaxolite;LocationQK">
        <rdfs:subClassOf rdf:resource="&sosa;ObservableProperty"/>
        <rdfs:comment xml:lang="en">A particular place or position.</rdfs:comment>
        <rdfs:label xml:lang="en">Location Quantity Kind</rdfs:label>
        <rdfs:seeAlso rdf:resource="&geo;SpatialThing"/>
        <rdfs:isDefinedBy rdf:resource="http://purl.org/iot/vocab/m3-lite#"/>
    </owl:Class>



    <!-- http://purl.org/iot/vocab/iot-taxonomy-lite#Lumen -->

    <owl:Class rdf:about="&iottaxolite;Lumen">
        <rdfs:subClassOf rdf:resource="&qu;Unit"/>
        <rdfs:comment xml:lang="en">The SI unit of luminous flux, equal to the amount of light emitted per second in a unit solid angle of one steradian from a uniform source of one candela.</rdfs:comment>
        <rdfs:label xml:lang="en">Lumen (lm)</rdfs:label>
        <rdfs:seeAlso>http://purl.oclc.org/NET/ssnx/qu/unit#lumen</rdfs:seeAlso>
        <rdfs:isDefinedBy rdf:resource="http://purl.org/iot/vocab/m3-lite#"/>
    </owl:Class>



    <!-- http://purl.org/iot/vocab/iot-taxonomy-lite#LuminousFlux -->

    <owl:Class rdf:about="&iottaxolite;LuminousFlux">
        <rdfs:subClassOf rdf:resource="&sosa;ObservableProperty"/>
        <rdfs:comment xml:lang="en">Luminous Flux is the measure of the perceived power of light.</rdfs:comment>
        <rdfs:label xml:lang="en">Luminous Flux</rdfs:label>
        <rdfs:isDefinedBy rdf:resource="http://purl.org/iot/vocab/m3-lite#"/>
    </owl:Class>



    <!-- http://purl.org/iot/vocab/iot-taxonomy-lite#LuminousIntensity -->

    <owl:Class rdf:about="&iottaxolite;LuminousIntensity">
        <rdfs:subClassOf rdf:resource="&sosa;ObservableProperty"/>
        <rdfs:comment xml:lang="en"> It is a measure of the wavelength-weighted power emitted by a light source in a particular direction per unit solid angle, based on the luminosity function, a standardized model of the sensitivity of the human eye. The SI unit of luminous intensity is the candela (cd), an SI base unit. (Source Wikipedia)</rdfs:comment>
        <rdfs:label xml:lang="en">Luminous Intensity</rdfs:label>
        <rdfs:isDefinedBy rdf:resource="http://purl.org/iot/vocab/m3-lite#"/>
    </owl:Class>



    <!-- http://purl.org/iot/vocab/iot-taxonomy-lite#Lux -->

    <owl:Class rdf:about="&iottaxolite;Lux">
        <rdfs:subClassOf rdf:resource="&qu;Unit"/>
        <rdfs:comment xml:lang="en">The SI unit of illuminance, equal to one lumen per square metre.</rdfs:comment>
        <rdfs:label xml:lang="en">Lux (lx)</rdfs:label>
        <rdfs:seeAlso rdf:resource="&qudt;Lux"/>
        <rdfs:seeAlso rdf:resource="http://sweet.jpl.nasa.gov/ontology/units.owl#lux"/>
        <rdfs:seeAlso>http://purl.oclc.org/NET/ssnx/qu/unit#lux</rdfs:seeAlso>
        <rdfs:isDefinedBy rdf:resource="http://purl.org/iot/vocab/m3-lite#"/>
    </owl:Class>



    <!-- http://purl.org/iot/vocab/iot-taxonomy-lite#MagneticField -->

    <owl:Class rdf:about="&iottaxolite;MagneticField">
        <rdfs:subClassOf rdf:resource="&sosa;ObservableProperty"/>
        <rdfs:comment xml:lang="en">A region around a magnetic material or a moving electric charge within which the force of magnetism acts.</rdfs:comment>
        <rdfs:label xml:lang="en">Magnetic Field</rdfs:label>
        <rdfs:isDefinedBy rdf:resource="http://purl.org/iot/vocab/m3-lite#"/>
    </owl:Class>



    <!-- http://purl.org/iot/vocab/iot-taxonomy-lite#MagneticFluxDensity -->

    <owl:Class rdf:about="&iottaxolite;MagneticFluxDensity">
        <rdfs:subClassOf rdf:resource="&sosa;ObservableProperty"/>
        <rdfs:comment xml:lang="en">It is the magnetic flux  through a surface is the surface integral of the normal component of the magnetic field (B) passing through that surface. The SI unit of magnetic flux is the weber (Wb). (Source Wikipedia).</rdfs:comment>
        <rdfs:label xml:lang="en">Magnetic Flux Density</rdfs:label>
        <rdfs:isDefinedBy rdf:resource="http://purl.org/iot/vocab/m3-lite#"/>
    </owl:Class>



    <!-- http://purl.org/iot/vocab/iot-taxonomy-lite#Magnetometer -->

    <owl:Class rdf:about="&iottaxolite;Magnetometer">
        <rdfs:subClassOf rdf:resource="&sosa;Sensor"/>
        <rdfs:comment xml:lang="en">A magnetometer is an device that measures magnetism—either magnetization of magnetic material like a ferromagnet, or the strength and, in some cases, direction of the magnetic field at a point in space. (Source Wikipedia).</rdfs:comment>
        <rdfs:label xml:lang="en">Magnetometer</rdfs:label>
        <rdfs:isDefinedBy rdf:resource="http://purl.org/iot/vocab/m3-lite#"/>
    </owl:Class>



    <!-- http://purl.org/iot/vocab/iot-taxonomy-lite#Manual -->

    <owl:Class rdf:about="&iottaxolite;Manual">
        <rdfs:subClassOf rdf:resource="&iottaxolite;MeasurementType"/>
        <rdfs:comment xml:lang="en">If the measurement was taken when human effort was involved.</rdfs:comment>
        <rdfs:label xml:lang="en">Manual Measurement Type</rdfs:label>
        <rdfs:isDefinedBy rdf:resource="http://purl.org/iot/vocab/m3-lite#"/>
    </owl:Class>



    <!-- http://purl.org/iot/vocab/iot-taxonomy-lite#Mass -->

    <owl:Class rdf:about="&iottaxolite;Mass">
        <rdfs:subClassOf rdf:resource="&sosa;ObservableProperty"/>
        <rdfs:comment xml:lang="en">Mass is a property of a physical body. It is the measure of an object's resistance to acceleration when a net force is applied.</rdfs:comment>
        <rdfs:label xml:lang="en">Mass</rdfs:label>
        <rdfs:seeAlso>http://purl.oclc.org/NET/ssnx/qu/quantity#mass</rdfs:seeAlso>
        <rdfs:isDefinedBy rdf:resource="http://purl.org/iot/vocab/m3-lite#"/>
    </owl:Class>



    <!-- http://purl.org/iot/vocab/iot-taxonomy-lite#MeasurementType -->

    <owl:Class rdf:about="&iottaxolite;MeasurementType">
        <rdfs:comment xml:lang="en">Type of Measurement done using a device.</rdfs:comment>
        <rdfs:label xml:lang="en">Measurement Type</rdfs:label>
        <rdfs:isDefinedBy rdf:resource="http://purl.org/iot/vocab/m3-lite#"/>
    </owl:Class>



    <!-- http://purl.org/iot/vocab/iot-taxonomy-lite#Metre -->

    <owl:Class rdf:about="&iottaxolite;Metre">
        <rdfs:subClassOf rdf:resource="&qu;Unit"/>
        <rdfs:comment xml:lang="en">It is the unit of length.</rdfs:comment>
        <rdfs:label xml:lang="en">Metre, Meter</rdfs:label>
        <rdfs:seeAlso rdf:resource="&qudt;Meter"/>
        <rdfs:seeAlso rdf:resource="http://sweet.jpl.nasa.gov/ontology/units.owl#meter"/>
        <rdfs:isDefinedBy rdf:resource="http://purl.org/iot/vocab/m3-lite#"/>
    </owl:Class>



    <!-- http://purl.org/iot/vocab/iot-taxonomy-lite#MetrePerSecond -->

    <owl:Class rdf:about="&iottaxolite;MetrePerSecond">
        <rdfs:subClassOf rdf:resource="&qu;Unit"/>
        <rdfs:comment xml:lang="en">A speed/velocity unit which is equal to the speed of an object traveling 1 metre distance in one second.</rdfs:comment>
        <rdfs:label xml:lang="en">Metre Per Second, Meter Per Second  (m/s)</rdfs:label>
        <rdfs:seeAlso rdf:resource="&qudt;MeterPerSecond"/>
        <rdfs:seeAlso>http://purl.oclc.org/NET/ssnx/qu/unit#metrePerSecond</rdfs:seeAlso>
        <rdfs:isDefinedBy rdf:resource="http://purl.org/iot/vocab/m3-lite#"/>
    </owl:Class>



    <!-- http://purl.org/iot/vocab/iot-taxonomy-lite#MetrePerSecondSquare -->

    <owl:Class rdf:about="&iottaxolite;MetrePerSecondSquare">
        <rdfs:subClassOf rdf:resource="&qu;Unit"/>
        <rdfs:comment xml:lang="en">It is the unit of acceleration (Metre Per Second Square, Meter Per Second Square)</rdfs:comment>
        <rdfs:label xml:lang="en">Metre Per Second Square, Meter Per Second Square</rdfs:label>
        <rdfs:seeAlso rdf:resource="http://purl.oclc.org/NET/ssnx/qu/unit#metrePerSecondSquared"/>
        <rdfs:isDefinedBy rdf:resource="http://purl.org/iot/vocab/m3-lite#"/>
    </owl:Class>



    <!-- http://purl.org/iot/vocab/iot-taxonomy-lite#MethaneSensor -->

    <owl:Class rdf:about="&iottaxolite;MethaneSensor">
        <rdfs:subClassOf rdf:resource="&iottaxolite;GaseousPollutantSensor"/>
        <rdfs:comment xml:lang="en">Device used to detect Methane in the environment.</rdfs:comment>
        <rdfs:label xml:lang="en">Methane (CH4) Sensor</rdfs:label>
        <rdfs:isDefinedBy rdf:resource="http://purl.org/iot/vocab/m3-lite#"/>
    </owl:Class>



    <!-- http://purl.org/iot/vocab/iot-taxonomy-lite#Microampere -->

    <owl:Class rdf:about="&iottaxolite;Microampere">
        <rdfs:subClassOf rdf:resource="&iottaxolite;Ampere"/>
        <rdfs:label xml:lang="en">Microampere (uA)</rdfs:label>
        <rdfs:comment xml:lang="en">It is a unit of electric current, or amount of electric charge per second.</rdfs:comment>
        <rdfs:isDefinedBy rdf:resource="http://purl.org/iot/vocab/m3-lite#"/>
    </owl:Class>



    <!-- http://purl.org/iot/vocab/iot-taxonomy-lite#Microgram -->

    <owl:Class rdf:about="&iottaxolite;Microgram">
        <rdfs:subClassOf rdf:resource="&iottaxolite;Gram"/>
        <rdfs:label xml:lang="en">Microgram (ug)</rdfs:label>
        <rdfs:comment xml:lang="en">It is a unit of mass equal to one billionth (1×10^−9) of a kilogram.</rdfs:comment>
        <rdfs:isDefinedBy rdf:resource="http://purl.org/iot/vocab/m3-lite#"/>
    </owl:Class>



    <!-- http://purl.org/iot/vocab/iot-taxonomy-lite#MicrogramPerCubicMetre -->

    <owl:Class rdf:about="&iottaxolite;MicrogramPerCubicMetre">
        <rdfs:subClassOf rdf:resource="&iottaxolite;GramPerCubicMetre"/>
        <rdfs:comment xml:lang="en">Microgram per cubic metre is a unit of density defined as microgram divided by cubic metre. Milligram per cubic metre is a derived unit in the International System of Units.</rdfs:comment>
        <rdfs:label xml:lang="en">Microgram Per Cubic Metre, Microgram Per Cubic Meter</rdfs:label>
        <rdfs:seeAlso>http://purl.oclc.org/NET/ssnx/qu/unit#microgramPerCubicMetre</rdfs:seeAlso>
        <rdfs:isDefinedBy rdf:resource="http://purl.org/iot/vocab/m3-lite#"/>
    </owl:Class>



    <!-- http://purl.org/iot/vocab/iot-taxonomy-lite#Microvolt -->

    <owl:Class rdf:about="&iottaxolite;Microvolt">
        <rdfs:subClassOf rdf:resource="&iottaxolite;Volt"/>
        <rdfs:label xml:lang="en">Microvolt (uV)</rdfs:label>
        <rdfs:comment xml:lang="en">It is a unit of electromotive force or potential difference equal to one millionth of a volt. </rdfs:comment>
        <rdfs:isDefinedBy rdf:resource="http://purl.org/iot/vocab/m3-lite#"/>
    </owl:Class>



    <!-- http://purl.org/iot/vocab/iot-taxonomy-lite#Microwatt -->

    <owl:Class rdf:about="&iottaxolite;Microwatt">
        <rdfs:subClassOf rdf:resource="&iottaxolite;Watt"/>
        <rdfs:label xml:lang="en">Microwatt (uW)</rdfs:label>
        <rdfs:comment xml:lang="en">It is a unit of power.</rdfs:comment>
        <rdfs:isDefinedBy rdf:resource="http://purl.org/iot/vocab/m3-lite#"/>
    </owl:Class>



    <!-- http://purl.org/iot/vocab/iot-taxonomy-lite#Microwave -->

    <owl:Class rdf:about="&iottaxolite;Microwave">
        <rdfs:subClassOf rdf:resource="&sosa;Actuator"/>
        <rdfs:comment xml:lang="en">An actuator to automatically switch on/off the Microwave.</rdfs:comment>
        <rdfs:label xml:lang="en">Microwave Actuating Device</rdfs:label>
        <rdfs:isDefinedBy rdf:resource="http://purl.org/iot/vocab/m3-lite#"/>
    </owl:Class>



    <!-- http://purl.org/iot/vocab/iot-taxonomy-lite#Mileage -->

    <owl:Class rdf:about="&iottaxolite;Mileage">
        <rdfs:subClassOf rdf:resource="&sosa;ObservableProperty"/>
        <rdfs:label xml:lang="en">Mileage</rdfs:label>
        <rdfs:comment xml:lang="en">Measure of the number of miles or the average distance that a vehicle can travel on a specified quantity of fuel</rdfs:comment>
        <rdfs:isDefinedBy rdf:resource="http://purl.org/iot/vocab/m3-lite#"/>
    </owl:Class>



    <!-- http://purl.org/iot/vocab/iot-taxonomy-lite#MileageDistanceToService -->

    <owl:Class rdf:about="&iottaxolite;MileageDistanceToService">
        <rdfs:subClassOf rdf:resource="&iottaxolite;Mileage"/>
        <rdfs:comment xml:lang="en">The distance which can be travelled by the vehicle before the next service inspection is required.  A negative distance is transmitted if the service inspection has been passed.</rdfs:comment>
        <rdfs:label xml:lang="en">Mileage Distance To Service</rdfs:label>
        <rdfs:isDefinedBy rdf:resource="http://purl.org/iot/vocab/m3-lite#"/>
    </owl:Class>



    <!-- http://purl.org/iot/vocab/iot-taxonomy-lite#MileageTotal -->

    <owl:Class rdf:about="&iottaxolite;MileageTotal">
        <rdfs:subClassOf rdf:resource="&iottaxolite;Mileage"/>
        <rdfs:comment xml:lang="en">The total distance travelled by the particular vehicle since its initial production.</rdfs:comment>
        <rdfs:label xml:lang="en">Mileage Total</rdfs:label>
        <rdfs:isDefinedBy rdf:resource="http://purl.org/iot/vocab/m3-lite#"/>
    </owl:Class>



    <!-- http://purl.org/iot/vocab/iot-taxonomy-lite#Miles -->

    <owl:Class rdf:about="&iottaxolite;Miles">
        <rdfs:subClassOf rdf:resource="&iottaxolite;Metre"/>
        <rdfs:comment xml:lang="en">It is a unit of length that is equal to 1,760 yards (approx. 1.609 kilometres).</rdfs:comment>
        <rdfs:label xml:lang="en">Miles</rdfs:label>
        <rdfs:isDefinedBy rdf:resource="http://purl.org/iot/vocab/m3-lite#"/>
    </owl:Class>



    <!-- http://purl.org/iot/vocab/iot-taxonomy-lite#Millisecond -->

    <owl:Class rdf:about="&iottaxolite;Millisecond">
        <rdfs:subClassOf rdf:resource="&iottaxolite;SecondTime"/>
        <rdfs:comment xml:lang="en">One thousandth of a second.</rdfs:comment>
        <rdfs:label xml:lang="en">Millisecond</rdfs:label>
        <rdfs:isDefinedBy rdf:resource="http://purl.org/iot/vocab/m3-lite#"/>
    </owl:Class>



    <!-- http://purl.org/iot/vocab/iot-taxonomy-lite#Milliampere -->

    <owl:Class rdf:about="&iottaxolite;Milliampere">
        <rdfs:subClassOf rdf:resource="&iottaxolite;Ampere"/>
        <rdfs:label xml:lang="en">Milliampere (mA)</rdfs:label>
        <rdfs:comment xml:lang="en">One thousandth of an ampere.</rdfs:comment>
        <rdfs:isDefinedBy rdf:resource="http://purl.org/iot/vocab/m3-lite#"/>
    </owl:Class>



    <!-- http://purl.org/iot/vocab/iot-taxonomy-lite#Millibar -->

    <owl:Class rdf:about="&iottaxolite;Millibar">
        <rdfs:subClassOf rdf:resource="&iottaxolite;Bar"/>
        <rdfs:label xml:lang="en">Millibar</rdfs:label>
        <rdfs:comment xml:lang="en">One thousandth of a bar.</rdfs:comment>
        <rdfs:isDefinedBy rdf:resource="http://purl.org/iot/vocab/m3-lite#"/>
    </owl:Class>



    <!-- http://purl.org/iot/vocab/iot-taxonomy-lite#Milligram -->

    <owl:Class rdf:about="&iottaxolite;Milligram">
        <rdfs:subClassOf rdf:resource="&iottaxolite;Gram"/>
        <rdfs:label xml:lang="en">Milligram (mg)</rdfs:label>
        <rdfs:comment xml:lang="en">One thousandth of a gram.</rdfs:comment>
        <rdfs:isDefinedBy rdf:resource="http://purl.org/iot/vocab/m3-lite#"/>
    </owl:Class>



    <!-- http://purl.org/iot/vocab/iot-taxonomy-lite#MilligramPerCubicMetre -->

    <owl:Class rdf:about="&iottaxolite;MilligramPerCubicMetre">
        <rdfs:subClassOf rdf:resource="&iottaxolite;GramPerCubicMetre"/>
        <rdfs:label xml:lang="en">Milligram Per Cubic Metre, Milligram Per Cubic Meter</rdfs:label>
        <rdfs:comment xml:lang="en">It is a density measurement unit.</rdfs:comment>
        <rdfs:isDefinedBy rdf:resource="http://purl.org/iot/vocab/m3-lite#"/>
    </owl:Class>



    <!-- http://purl.org/iot/vocab/iot-taxonomy-lite#MilligramPerSquareMetre -->

    <owl:Class rdf:about="&iottaxolite;MilligramPerSquareMetre">
        <rdfs:subClassOf rdf:resource="&qu;Unit"/>
        <rdfs:comment xml:lang="en">A dose unit which is equal to 1 milligram of a substance per square metre of surface area of the recipient subject.</rdfs:comment>
        <rdfs:label xml:lang="en">Milligram Per Square Metre, Milligram Per Square Meter</rdfs:label>
        <rdfs:seeAlso>http://purl.oclc.org/NET/ssnx/qu/unit#milligramPerSquareMetre</rdfs:seeAlso>
        <rdfs:isDefinedBy rdf:resource="http://purl.org/iot/vocab/m3-lite#"/>
    </owl:Class>



    <!-- http://purl.org/iot/vocab/iot-taxonomy-lite#Millilitre -->

    <owl:Class rdf:about="&iottaxolite;Millilitre">
        <rdfs:subClassOf rdf:resource="&iottaxolite;Litre"/>
        <rdfs:comment xml:lang="en">One thousandth of a litre (0.002 pint).</rdfs:comment>
        <rdfs:label xml:lang="en">Millilitre, Milliliter</rdfs:label>
        <rdfs:isDefinedBy rdf:resource="http://purl.org/iot/vocab/m3-lite#"/>
    </owl:Class>



    <!-- http://purl.org/iot/vocab/iot-taxonomy-lite#MillimetrePerHour -->

    <owl:Class rdf:about="&iottaxolite;MillimetrePerHour">
        <rdfs:subClassOf rdf:resource="&qu;Unit"/>
        <rdfs:comment xml:lang="en">A unit of both speed (scalar) and velocity (vector), defined as the distance of one millimetre travelled per unit hour.</rdfs:comment>
        <rdfs:label xml:lang="en">Millimetre Per Hour, Millimeter Per Hour</rdfs:label>
        <rdfs:seeAlso>http://purl.oclc.org/NET/ssnx/qu/unit#millimetrePerHour</rdfs:seeAlso>
        <rdfs:isDefinedBy rdf:resource="http://purl.org/iot/vocab/m3-lite#"/>
    </owl:Class>



    <!-- http://purl.org/iot/vocab/iot-taxonomy-lite#Millimetre -->

    <owl:Class rdf:about="&iottaxolite;Millimetre">
        <rdfs:subClassOf rdf:resource="&iottaxolite;Metre"/>
        <rdfs:label xml:lang="en">Millimetre, Millimeter</rdfs:label>
        <rdfs:comment xml:lang="en">One thousandth of a metre (0.039 in).</rdfs:comment>
        <rdfs:isDefinedBy rdf:resource="http://purl.org/iot/vocab/m3-lite#"/>
    </owl:Class>



    <!-- http://purl.org/iot/vocab/iot-taxonomy-lite#Millivolt -->

    <owl:Class rdf:about="&iottaxolite;Millivolt">
        <rdfs:subClassOf rdf:resource="&iottaxolite;Volt"/>
        <rdfs:label xml:lang="en">Millivolt (mV)</rdfs:label>
        <rdfs:comment xml:lang="en">One thousandth of a volt.</rdfs:comment>
        <rdfs:isDefinedBy rdf:resource="http://purl.org/iot/vocab/m3-lite#"/>
    </owl:Class>



    <!-- http://purl.org/iot/vocab/iot-taxonomy-lite#MillivoltPerMetre -->

    <owl:Class rdf:about="&iottaxolite;MillivoltPerMetre">
        <rdfs:subClassOf rdf:resource="&qu;Unit"/>
        <rdfs:label xml:lang="en">Millivolt Per Metre, Millivolt Per Meter</rdfs:label>
        <rdfs:comment xml:lang="en">It is a measure of the intensity of the signal of a radio transmitter.</rdfs:comment>
        <rdfs:isDefinedBy rdf:resource="http://purl.org/iot/vocab/m3-lite#"/>
    </owl:Class>



    <!-- http://purl.org/iot/vocab/iot-taxonomy-lite#Milliwatt -->

    <owl:Class rdf:about="&iottaxolite;Milliwatt">
        <rdfs:subClassOf rdf:resource="&iottaxolite;Watt"/>
        <rdfs:label xml:lang="en">Milliwatt (mW)</rdfs:label>
        <rdfs:comment xml:lang="en">A unit of power equal to one thousandth of a watt.</rdfs:comment>
        <rdfs:isDefinedBy rdf:resource="http://purl.org/iot/vocab/m3-lite#"/>
    </owl:Class>



    <!-- http://purl.org/iot/vocab/iot-taxonomy-lite#MinuteAngle -->

    <owl:Class rdf:about="&iottaxolite;MinuteAngle">
        <rdfs:subClassOf rdf:resource="&qu;Unit"/>
        <rdfs:comment xml:lang="en">A Minute of Angle (MOA) is an angular measurement. A MOA is 1/60th of a degree.</rdfs:comment>
        <rdfs:label xml:lang="en">Minute Angle</rdfs:label>
        <rdfs:isDefinedBy rdf:resource="http://purl.org/iot/vocab/m3-lite#"/>
    </owl:Class>



    <!-- http://purl.org/iot/vocab/iot-taxonomy-lite#MinuteTime -->

    <owl:Class rdf:about="&iottaxolite;MinuteTime">
        <rdfs:subClassOf rdf:resource="&iottaxolite;SecondTime"/>
        <rdfs:comment xml:lang="en">A unit of time equal to 60 seconds or 1/60th of an hour.</rdfs:comment>
        <rdfs:label xml:lang="en">Minute Time</rdfs:label>
        <rdfs:isDefinedBy rdf:resource="http://purl.org/iot/vocab/m3-lite#"/>
    </owl:Class>



    <!-- http://purl.org/iot/vocab/iot-taxonomy-lite#MmHg -->

    <owl:Class rdf:about="&iottaxolite;MmHg">
        <rdfs:subClassOf rdf:resource="&qu;Unit"/>
        <rdfs:comment xml:lang="en">A millimetre of mercury is a manometric unit of pressure, formerly defined as the extra pressure generated by a column of mercury one millimetre high and now defined as precisely 133.322387415 pascals. It is denoted by the symbol mmHg. It  is used to measure blood pressure measurements (systolic and diastolic).</rdfs:comment>
        <rdfs:label xml:lang="en">MmHg</rdfs:label>
        <rdfs:isDefinedBy rdf:resource="http://purl.org/iot/vocab/m3-lite#"/>
    </owl:Class>



    <!-- http://purl.org/iot/vocab/iot-taxonomy-lite#MmolPerLitre -->

    <owl:Class rdf:about="&iottaxolite;MmolPerLitre">
        <rdfs:subClassOf rdf:resource="&qu;Unit"/>
        <rdfs:comment xml:lang="en">It is the amount of a substance that corresponds to its formula mass in milligrams. MmolPerLitre is used to measure cholesterol.</rdfs:comment>
        <rdfs:label xml:lang="en">Mmol Per Litre, Mmol Per Liter</rdfs:label>
        <rdfs:isDefinedBy rdf:resource="http://purl.org/iot/vocab/m3-lite#"/>
    </owl:Class>



    <!-- http://purl.org/iot/vocab/iot-taxonomy-lite#MobHoExecSuccRate -->

    <owl:Class rdf:about="&iottaxolite;MobHoExecSuccRate">
        <rdfs:subClassOf rdf:resource="&iottaxolite;Communication"/>
        <rdfs:comment xml:lang="en">Handover Execution.</rdfs:comment>
        <rdfs:label xml:lang="en">Handover Execution</rdfs:label>
        <rdfs:isDefinedBy rdf:resource="http://purl.org/iot/vocab/m3-lite#"/>
    </owl:Class>



    <!-- http://purl.org/iot/vocab/iot-taxonomy-lite#MobHoPrepSuccRate -->

    <owl:Class rdf:about="&iottaxolite;MobHoPrepSuccRate">
        <rdfs:subClassOf rdf:resource="&iottaxolite;Communication"/>
        <rdfs:comment xml:lang="en">Handover Preparation Success Rate.</rdfs:comment>
        <rdfs:label xml:lang="en">Handover Preparation Success Rate</rdfs:label>
        <rdfs:isDefinedBy rdf:resource="http://purl.org/iot/vocab/m3-lite#"/>
    </owl:Class>



    <!-- http://purl.org/iot/vocab/iot-taxonomy-lite#MobMobilitySuccRate -->

    <owl:Class rdf:about="&iottaxolite;MobMobilitySuccRate">
        <rdfs:subClassOf rdf:resource="&iottaxolite;Communication"/>
        <rdfs:comment xml:lang="en">Handover Mobility Success Rate.</rdfs:comment>
        <rdfs:label xml:lang="en">Handover Mobility Success Rate</rdfs:label>
        <rdfs:isDefinedBy rdf:resource="http://purl.org/iot/vocab/m3-lite#"/>
    </owl:Class>



    <!-- http://purl.org/iot/vocab/iot-taxonomy-lite#Motion -->

    <owl:Class rdf:about="&iottaxolite;Motion">
        <rdfs:subClassOf rdf:resource="&sosa;ObservableProperty"/>
        <rdfs:comment xml:lang="en">It is the action or process of moving or being moved.</rdfs:comment>
        <rdfs:label xml:lang="en">Motion</rdfs:label>
        <rdfs:seeAlso rdf:resource="http://spitfire-project.eu/ontology/ns/Motion"/>
        <rdfs:isDefinedBy rdf:resource="http://purl.org/iot/vocab/m3-lite#"/>
    </owl:Class>


    <!-- http://purl.org/iot/vocab/iot-taxonomy-lite#MotionState -->

    <owl:Class rdf:about="&iottaxolite;MotionState">
        <rdfs:subClassOf rdf:resource="&sosa;ObservableProperty"/>
        <rdfs:label xml:lang="en">Motion State</rdfs:label>
        <rdfs:comment xml:lang="en">Indicator of whether a person (or object) is detected upon his/her/its movement.</rdfs:comment>
        <rdfs:isDefinedBy rdf:resource="http://purl.org/iot/vocab/m3-lite#"/>
    </owl:Class>



    <!-- http://purl.org/iot/vocab/iot-taxonomy-lite#MotionStateVehicle -->

    <owl:Class rdf:about="&iottaxolite;MotionStateVehicle">
        <rdfs:subClassOf rdf:resource="&iottaxolite;MotionState"/>
        <rdfs:comment xml:lang="en">Indicates whether motion of the vehicle is detected or not.</rdfs:comment>
        <rdfs:label xml:lang="en">Motion State Vehicle</rdfs:label>
        <rdfs:isDefinedBy rdf:resource="http://purl.org/iot/vocab/m3-lite#"/>
    </owl:Class>



    <!-- http://purl.org/iot/vocab/iot-taxonomy-lite#NFC -->

    <owl:Class rdf:about="&iottaxolite;NFC">
        <rdfs:subClassOf rdf:resource="&iot-lite;Tag"/>
        <rdfs:comment xml:lang="en">A tagging device can be NFC (Near Field Communication).</rdfs:comment>
        <rdfs:label xml:lang="en">NFC Tagging Device</rdfs:label>
        <rdfs:isDefinedBy rdf:resource="http://purl.org/iot/vocab/m3-lite#"/>
    </owl:Class>



    <!-- http://purl.org/iot/vocab/iot-taxonomy-lite#NH3Sensor -->

    <owl:Class rdf:about="&iottaxolite;NH3Sensor">
        <rdfs:subClassOf rdf:resource="&iottaxolite;GaseousPollutantSensor"/>
        <rdfs:comment xml:lang="en">Device used to detect NH3 level in the environment.</rdfs:comment>
        <rdfs:label xml:lang="en">NH3 Sensor</rdfs:label>
        <rdfs:isDefinedBy rdf:resource="http://purl.org/iot/vocab/m3-lite#"/>
    </owl:Class>



    <!-- http://purl.org/iot/vocab/iot-taxonomy-lite#NO2Sensor -->

    <owl:Class rdf:about="&iottaxolite;NO2Sensor">
        <rdfs:subClassOf rdf:resource="&iottaxolite;GaseousPollutantSensor"/>
        <rdfs:comment xml:lang="en">Sensor detecting levels of Nitrogen Dioxide (NO2) in the environment.</rdfs:comment>
        <rdfs:label xml:lang="en">Nitrogen Dioxide (NO2) Sensor</rdfs:label>
        <rdfs:isDefinedBy rdf:resource="http://purl.org/iot/vocab/m3-lite#"/>
    </owl:Class>



    <!-- http://purl.org/iot/vocab/iot-taxonomy-lite#NOSensor -->

    <owl:Class rdf:about="&iottaxolite;NOSensor">
        <rdfs:subClassOf rdf:resource="&iottaxolite;GaseousPollutantSensor"/>
        <rdfs:comment xml:lang="en">Device used to detect Nitrogen Oxide (NO) in the environment.</rdfs:comment>
        <rdfs:label xml:lang="en">Nitrogen Oxide (NO) Sensor</rdfs:label>
        <rdfs:isDefinedBy rdf:resource="http://purl.org/iot/vocab/m3-lite#"/>
    </owl:Class>



    <!-- http://purl.org/iot/vocab/iot-taxonomy-lite#Neighbors -->

    <owl:Class rdf:about="&iottaxolite;Neighbours">
        <rdfs:subClassOf rdf:resource="&iottaxolite;SoundSource"/>
        <rdfs:comment xml:lang="en">When the source of the sound were noisy neighbours.</rdfs:comment>
        <rdfs:label xml:lang="en">Neighbours Sound Source</rdfs:label>
        <rdfs:isDefinedBy rdf:resource="http://purl.org/iot/vocab/m3-lite#"/>
    </owl:Class>



    <!-- http://purl.org/iot/vocab/iot-taxonomy-lite#Step -->

    <owl:Class rdf:about="&iottaxolite;Step">
        <rdfs:subClassOf rdf:resource="&qu;Unit"/>
        <rdfs:comment xml:lang="en">It is a measure of number of Step taken.</rdfs:comment>
        <rdfs:label xml:lang="en">Step</rdfs:label>
        <rdfs:isDefinedBy rdf:resource="http://purl.org/iot/vocab/m3-lite#"/>
    </owl:Class>



    <!-- http://purl.org/iot/vocab/iot-taxonomy-lite#O3Sensor -->

    <owl:Class rdf:about="&iottaxolite;O3Sensor">
        <rdfs:subClassOf rdf:resource="&iottaxolite;GaseousPollutantSensor"/>
        <rdfs:comment xml:lang="en">Device used to detect Ozone (O3) in the environment.</rdfs:comment>
        <rdfs:label xml:lang="en">Ozone (O3) Sensor</rdfs:label>
        <rdfs:isDefinedBy rdf:resource="http://purl.org/iot/vocab/m3-lite#"/>
    </owl:Class>



    <!-- http://purl.org/iot/vocab/iot-taxonomy-lite#PresenceDetector -->

    <owl:Class rdf:about="&iottaxolite;PresenceDetector">
        <rdfs:subClassOf rdf:resource="&sosa;Sensor"/>
        <rdfs:comment xml:lang="en">Device used to detect if on object is occupied or not.</rdfs:comment>
        <rdfs:label xml:lang="en">Presence Detector</rdfs:label>
        <rdfs:seeAlso rdf:resource="http://casas.wsu.edu/owl/cose.owl#PassiveInfraredSensor"/>
        <rdfs:isDefinedBy rdf:resource="http://purl.org/iot/vocab/m3-lite#"/>
    </owl:Class>



    <!-- http://purl.org/iot/vocab/iot-taxonomy-lite#Odometer -->

    <owl:Class rdf:about="&iottaxolite;Odometer">
        <rdfs:subClassOf rdf:resource="&sosa;Sensor"/>
        <rdfs:comment xml:lang="en">An odometer or odograph is an instrument that indicates distance travelled by a vehicle, such as bicycle or automobile.</rdfs:comment>
        <rdfs:label xml:lang="en">Odometer</rdfs:label>
        <rdfs:isDefinedBy rdf:resource="http://purl.org/iot/vocab/m3-lite#"/>
    </owl:Class>



    <!-- http://purl.org/iot/vocab/iot-taxonomy-lite#Ohm -->

    <owl:Class rdf:about="&iottaxolite;Ohm">
        <rdfs:subClassOf rdf:resource="&qu;Unit"/>
        <rdfs:comment xml:lang="en">Ohm is the unit of electrical resistance.</rdfs:comment>
        <rdfs:label xml:lang="en">Ohm</rdfs:label>
        <rdfs:seeAlso rdf:resource="http://sweet.jpl.nasa.gov/ontology/units.owl#ohm"/>
        <rdfs:isDefinedBy rdf:resource="http://purl.org/iot/vocab/m3-lite#"/>
    </owl:Class>



    <!-- http://purl.org/iot/vocab/iot-taxonomy-lite#Okta -->

    <owl:Class rdf:about="&iottaxolite;Okta">
        <rdfs:subClassOf rdf:resource="&qu;Unit"/>
        <rdfs:comment xml:lang="en">Okta is the unit to measure the cloud cover.</rdfs:comment>
        <rdfs:label xml:lang="en">Okta</rdfs:label>
        <rdfs:isDefinedBy rdf:resource="http://purl.org/iot/vocab/m3-lite#"/>
    </owl:Class>



    <!-- http://purl.org/iot/vocab/iot-taxonomy-lite#Others -->

    <owl:Class rdf:about="&iottaxolite;Others">
        <rdfs:subClassOf rdf:resource="&sosa;ObservableProperty"/>
        <rdfs:subClassOf rdf:resource="&qu;Unit"/>
        <rdfs:subClassOf rdf:resource="&iottaxolite;MeasurementType"/>
        <rdfs:subClassOf rdf:resource="&iottaxolite;SoundSource"/>
        <rdfs:subClassOf rdf:resource="&iottaxolite;Source"/>
        <rdfs:comment xml:lang="en">Relates to phenomenon and unit that are not available currently in the current version of Taxonomy.</rdfs:comment>
        <rdfs:label xml:lang="en">Others</rdfs:label>
        <rdfs:isDefinedBy rdf:resource="http://purl.org/iot/vocab/m3-lite#"/>
    </owl:Class>



    <!-- http://purl.org/iot/vocab/iot-taxonomy-lite#OxygenSensor -->

    <owl:Class rdf:about="&iottaxolite;OxygenSensor">
        <rdfs:subClassOf rdf:resource="&iottaxolite;GaseousPollutantSensor"/>
        <rdfs:comment xml:lang="en">Device used to detect Oxygen (O2) in the environment.</rdfs:comment>
        <rdfs:label xml:lang="en">Oxygen Sensor</rdfs:label>
        <rdfs:isDefinedBy rdf:resource="http://purl.org/iot/vocab/m3-lite#"/>
    </owl:Class>



    <!-- http://purl.org/iot/vocab/iot-taxonomy-lite#PH -->

    <owl:Class rdf:about="&iottaxolite;PH">
        <rdfs:subClassOf rdf:resource="&sosa;ObservableProperty"/>
        <rdfs:comment xml:lang="en">It is a numeric scale used to specify the acidity or basicity of an aqueous solution.</rdfs:comment>
        <rdfs:label xml:lang="en">PH</rdfs:label>
        <rdfs:isDefinedBy rdf:resource="http://purl.org/iot/vocab/m3-lite#"/>
    </owl:Class>



    <!-- http://purl.org/iot/vocab/iot-taxonomy-lite#PHSensor -->

    <owl:Class rdf:about="&iottaxolite;PHSensor">
        <rdfs:subClassOf rdf:resource="&sosa;Sensor"/>
        <rdfs:comment xml:lang="en">Device used to detect PH level.</rdfs:comment>
        <rdfs:label xml:lang="en">PH Sensor</rdfs:label>
        <rdfs:isDefinedBy rdf:resource="http://purl.org/iot/vocab/m3-lite#"/>
    </owl:Class>



    <!-- http://purl.org/iot/vocab/iot-taxonomy-lite#PPM -->

    <owl:Class rdf:about="&iottaxolite;PPM">
        <rdfs:subClassOf rdf:resource="&qu;Unit"/>
        <rdfs:comment xml:lang="en">It describes the concentration of something in water or soil.</rdfs:comment>
        <rdfs:label xml:lang="en">PPM (parts per million)</rdfs:label>
        <rdfs:isDefinedBy rdf:resource="http://purl.org/iot/vocab/m3-lite#"/>
    </owl:Class>





    <!-- http://purl.org/iot/vocab/iot-taxonomy-lite#Pascal -->

    <owl:Class rdf:about="&iottaxolite;Pascal">
        <rdfs:subClassOf rdf:resource="&qu;Unit"/>
        <rdfs:comment xml:lang="en">Unit for pressure (e.g., atmospheric pressure).</rdfs:comment>
        <rdfs:label xml:lang="en">Pascal</rdfs:label>
        <rdfs:isDefinedBy rdf:resource="http://purl.org/iot/vocab/m3-lite#"/>
    </owl:Class>




    <!-- http://purl.org/iot/vocab/iot-taxonomy-lite#Pedometer -->

    <owl:Class rdf:about="&iottaxolite;Pedometer">
        <rdfs:subClassOf rdf:resource="&sosa;Sensor"/>
        <rdfs:comment xml:lang="en">Pedometer is used to count the number of steps when walking, running, etc.</rdfs:comment>
        <rdfs:label xml:lang="en">Pedometer</rdfs:label>
        <rdfs:isDefinedBy rdf:resource="http://purl.org/iot/vocab/m3-lite#"/>
    </owl:Class>



    <!-- http://purl.org/iot/vocab/iot-taxonomy-lite#Percent -->

    <owl:Class rdf:about="&iottaxolite;Percent">
        <rdfs:subClassOf rdf:resource="&qu;Unit"/>
        <rdfs:comment xml:lang="en">It is the amount in or for every hundred.</rdfs:comment>
        <rdfs:label xml:lang="en">Percent</rdfs:label>
        <rdfs:seeAlso rdf:resource="&qudt;Percent"/>
        <rdfs:seeAlso rdf:resource="http://sweet.jpl.nasa.gov/ontology/units.owl#percent"/>
        <rdfs:isDefinedBy rdf:resource="http://purl.org/iot/vocab/m3-lite#"/>
    </owl:Class>



    <!-- http://purl.org/iot/vocab/iot-taxonomy-lite#Place -->

    <owl:Class rdf:about="&iottaxolite;Place">
        <rdfs:subClassOf rdf:resource="&iottaxolite;DomainOfInterest"/>
        <rdfs:comment xml:lang="en">Location, Place, GPS coordinates as an Internet of Things (IoT) applicative domain.</rdfs:comment>
        <rdfs:label xml:lang="en">Place DOI</rdfs:label>
        <rdfs:isDefinedBy rdf:resource="http://purl.org/iot/vocab/m3-lite#"/>
    </owl:Class>




    <!-- http://purl.org/iot/vocab/iot-taxonomy-lite#Potassium -->

    <owl:Class rdf:about="&iottaxolite;Potassium">
        <rdfs:subClassOf rdf:resource="&sosa;ObservableProperty"/>
        <rdfs:comment xml:lang="en">It is the measure of Blood Potassium Level.</rdfs:comment>
        <rdfs:label xml:lang="en">Potassium</rdfs:label>
        <rdfs:isDefinedBy rdf:resource="http://purl.org/iot/vocab/m3-lite#"/>
    </owl:Class>



    <!-- http://purl.org/iot/vocab/iot-taxonomy-lite#Pound -->

    <owl:Class rdf:about="&iottaxolite;Pound">
        <rdfs:subClassOf rdf:resource="&iottaxolite;Gram"/>
        <rdfs:comment xml:lang="en">A unit of weight equal to 16 oz. 1 pound= 453.592 grams</rdfs:comment>
        <rdfs:label xml:lang="en">Pound</rdfs:label>
        <rdfs:isDefinedBy rdf:resource="http://purl.org/iot/vocab/m3-lite#"/>
    </owl:Class>



    <!-- http://purl.org/iot/vocab/iot-taxonomy-lite#Power -->

    <owl:Class rdf:about="&iottaxolite;Power">
        <rdfs:subClassOf rdf:resource="&sosa;ObservableProperty"/>
        <rdfs:comment xml:lang="en">It is the rate, per unit time, at which electrical energy is transferred by an electric circuit.</rdfs:comment>
        <rdfs:label xml:lang="en">Power</rdfs:label>
        <rdfs:isDefinedBy rdf:resource="http://purl.org/iot/vocab/m3-lite#"/>
    </owl:Class>



    <!-- http://purl.org/iot/vocab/iot-taxonomy-lite#Precipitation -->

    <owl:Class rdf:about="&iottaxolite;Precipitation">
        <rdfs:subClassOf rdf:resource="&sosa;ObservableProperty"/>
        <rdfs:comment xml:lang="en">It is any product of the condensation of atmospheric water vapour that falls under gravity.</rdfs:comment>
        <rdfs:label xml:lang="en">Precipitation</rdfs:label>
        <rdfs:seeAlso rdf:resource="http://archive.knoesis.org/research/semsci/application_domain/sem_sensor/ont/sensor-observation.owlPrecipitatiowl:onProperty"/>
        <rdfs:seeAlso rdf:resource="http://paul.staroch.name/thesis/SmartHomeWeather.owl#Precipitation"/>
        <rdfs:isDefinedBy rdf:resource="http://purl.org/iot/vocab/m3-lite#"/>
    </owl:Class>



    <!-- http://purl.org/iot/vocab/iot-taxonomy-lite#PrecipitationSensor -->

    <owl:Class rdf:about="&iottaxolite;PrecipitationSensor">
        <rdfs:subClassOf rdf:resource="&sosa;Sensor"/>
        <rdfs:comment xml:lang="en">It is a device measuring the amount of precipitation.</rdfs:comment>
        <rdfs:label xml:lang="en">Precipitation Sensor</rdfs:label>
        <rdfs:seeAlso rdf:resource="http://purl.oclc.org/NET/ssnx/meteo/aws#PrecipitationSensor"/>
        <rdfs:isDefinedBy rdf:resource="http://purl.org/iot/vocab/m3-lite#"/>
    </owl:Class>



    <!-- http://purl.org/iot/vocab/iot-taxonomy-lite#Presence -->

    <owl:Class rdf:about="&iottaxolite;Presence">
        <rdfs:subClassOf rdf:resource="&sosa;ObservableProperty"/>
        <rdfs:label xml:lang="en">Presence</rdfs:label>
        <rdfs:comment xml:lang="en">Measure to know if an object is present. It is usually boolean.</rdfs:comment>
        <rdfs:isDefinedBy rdf:resource="http://purl.org/iot/vocab/m3-lite#"/>
    </owl:Class>



    <!-- http://purl.org/iot/vocab/iot-taxonomy-lite#PresenceStateDriverCard -->

    <owl:Class rdf:about="&iottaxolite;PresenceStateDriverCard">
        <rdfs:subClassOf rdf:resource="&iottaxolite;Presence"/>
        <rdfs:label xml:lang="en">Presence State Driver Card</rdfs:label>
        <rdfs:comment xml:lang="en">Indicates the presence of the first driver card.</rdfs:comment>
        <rdfs:isDefinedBy rdf:resource="http://purl.org/iot/vocab/m3-lite#"/>
    </owl:Class>



    <!-- http://purl.org/iot/vocab/iot-taxonomy-lite#PresenceStateDriverCardOne -->

    <owl:Class rdf:about="&iottaxolite;PresenceStateDriverCardOne">
        <rdfs:subClassOf rdf:resource="&iottaxolite;PresenceStateDriverCard"/>
        <rdfs:comment xml:lang="en">Indicates the presence of the first driver card.</rdfs:comment>
        <rdfs:label xml:lang="en">Presence State Driver Card 1</rdfs:label>
        <rdfs:isDefinedBy rdf:resource="http://purl.org/iot/vocab/m3-lite#"/>
    </owl:Class>



    <!-- http://purl.org/iot/vocab/iot-taxonomy-lite#PresenceStateDriverCardTwo -->

    <owl:Class rdf:about="&iottaxolite;PresenceStateDriverCardTwo">
        <rdfs:subClassOf rdf:resource="&iottaxolite;PresenceStateDriverCard"/>
        <rdfs:comment xml:lang="en">Indicates the presence of the second driver card.</rdfs:comment>
        <rdfs:label xml:lang="en">Presence State Driver Card 2</rdfs:label>
        <rdfs:isDefinedBy rdf:resource="http://purl.org/iot/vocab/m3-lite#"/>
    </owl:Class>



    <!-- http://purl.org/iot/vocab/iot-taxonomy-lite#PresenceStateEmergencyVehicle -->

    <owl:Class rdf:about="&iottaxolite;PresenceStateEmergencyVehicle">
        <rdfs:subClassOf rdf:resource="&iottaxolite;Presence"/>
        <rdfs:comment xml:lang="en">The presence or absence of an emergency vehicle (ambulance, fire fighters, etc.).</rdfs:comment>
        <rdfs:label xml:lang="en">Presence State Emergency Vehicle</rdfs:label>
        <rdfs:isDefinedBy rdf:resource="http://purl.org/iot/vocab/m3-lite#"/>
    </owl:Class>



    <!-- http://purl.org/iot/vocab/iot-taxonomy-lite#PresenceStateParking -->

    <owl:Class rdf:about="&iottaxolite;PresenceStateParking">
        <rdfs:subClassOf rdf:resource="&iottaxolite;Presence"/>
        <rdfs:comment xml:lang="en">The presence or absence of a vehicle parked.</rdfs:comment>
        <rdfs:label xml:lang="en">Presence State Parking</rdfs:label>
        <rdfs:isDefinedBy rdf:resource="http://purl.org/iot/vocab/m3-lite#"/>
    </owl:Class>



    <!-- http://purl.org/iot/vocab/iot-taxonomy-lite#PresenceStatePeople -->

    <owl:Class rdf:about="&iottaxolite;PresenceStatePeople">
        <rdfs:subClassOf rdf:resource="&iottaxolite;Presence"/>
        <rdfs:comment xml:lang="en">The presence or absence of people passing.</rdfs:comment>
        <rdfs:label xml:lang="en">Presence State People</rdfs:label>
        <rdfs:isDefinedBy rdf:resource="http://purl.org/iot/vocab/m3-lite#"/>
    </owl:Class>



    <!-- http://purl.org/iot/vocab/iot-taxonomy-lite#Pressure -->

    <owl:Class rdf:about="&iottaxolite;Pressure">
        <rdfs:subClassOf rdf:resource="&sosa;ObservableProperty"/>
        <rdfs:comment xml:lang="en">It is the physical force exerted on or against an object by something in contact with it.</rdfs:comment>
        <rdfs:label xml:lang="en">Pressure</rdfs:label>
        <rdfs:seeAlso rdf:resource="http://archive.knoesis.org/research/semsci/application_domain/sem_sensor/ont/sensor-observation.owlPressureProperty"/>
        <rdfs:isDefinedBy rdf:resource="http://purl.org/iot/vocab/m3-lite#"/>
    </owl:Class>



    <!-- http://purl.org/iot/vocab/iot-taxonomy-lite#PressureSensor -->

    <owl:Class rdf:about="&iottaxolite;PressureSensor">
        <rdfs:subClassOf rdf:resource="&sosa;Sensor"/>
        <rdfs:comment xml:lang="en">A device used to detect pressure. For example, it can be attached on the bed to infer if the user is lying, sleeping, sitting, bed occupancy, etc.</rdfs:comment>
        <rdfs:label xml:lang="en">Pressure Sensor</rdfs:label>
        <rdfs:isDefinedBy rdf:resource="http://purl.org/iot/vocab/m3-lite#"/>
    </owl:Class>



    <!-- http://purl.org/iot/vocab/iot-taxonomy-lite#Proximity -->

    <owl:Class rdf:about="&iottaxolite;Proximity">
        <rdfs:subClassOf rdf:resource="&sosa;ObservableProperty"/>
        <rdfs:comment xml:lang="en">Measure to detect proximity.</rdfs:comment>
        <rdfs:label xml:lang="en">Proximity</rdfs:label>
        <rdfs:isDefinedBy rdf:resource="http://purl.org/iot/vocab/m3-lite#"/>
    </owl:Class>



    <!-- http://purl.org/iot/vocab/iot-taxonomy-lite#ProximitySensor -->

    <owl:Class rdf:about="&iottaxolite;ProximitySensor">
        <rdfs:subClassOf rdf:resource="&sosa;Sensor"/>
        <rdfs:comment xml:lang="en">Detect if something is within proximity of a sensor.</rdfs:comment>
        <rdfs:label xml:lang="en">Proximity Sensor</rdfs:label>
        <rdfs:isDefinedBy rdf:resource="http://purl.org/iot/vocab/m3-lite#"/>
    </owl:Class>



    <!-- http://purl.org/iot/vocab/iot-taxonomy-lite#PublicTransit -->

    <owl:Class rdf:about="&iottaxolite;PublicTransit">
        <rdfs:subClassOf rdf:resource="&iottaxolite;SoundSource"/>
        <rdfs:comment xml:lang="en">When the source of the sound was public transit.</rdfs:comment>
        <rdfs:label xml:lang="en">Public Transit Sound Source</rdfs:label>
        <rdfs:isDefinedBy rdf:resource="http://purl.org/iot/vocab/m3-lite#"/>
    </owl:Class>



    <!-- http://purl.org/iot/vocab/iot-taxonomy-lite#PulseOxymeter -->

    <owl:Class rdf:about="&iottaxolite;PulseOxymeter">
        <rdfs:subClassOf rdf:resource="&sosa;Sensor"/>
        <rdfs:comment xml:lang="en">Pulse Oxymeter, SpO2, Blood Oxygen Saturation Sensor are used to measure the concentration of oxygen in the blood.</rdfs:comment>
        <rdfs:label xml:lang="en">Pulse Oxymeter</rdfs:label>
        <rdfs:isDefinedBy rdf:resource="http://purl.org/iot/vocab/m3-lite#"/>
    </owl:Class>



    <!-- http://purl.org/iot/vocab/iot-taxonomy-lite#QRCode -->

    <owl:Class rdf:about="&iottaxolite;QRCode">
        <rdfs:subClassOf rdf:resource="&iot-lite;Tag"/>
        <rdfs:comment xml:lang="en">A tagging device can be QRCode.</rdfs:comment>
        <rdfs:label xml:lang="en">QR Code tagging Device</rdfs:label>
        <rdfs:isDefinedBy rdf:resource="http://purl.org/iot/vocab/m3-lite#"/>
    </owl:Class>



    <!-- http://purl.org/iot/vocab/iot-taxonomy-lite#RFID -->

    <owl:Class rdf:about="&iottaxolite;RFID">
        <rdfs:subClassOf rdf:resource="&iot-lite;Tag"/>
        <rdfs:comment xml:lang="en">A tagging device can be RFID.</rdfs:comment>
        <rdfs:label xml:lang="en">RFID Tagging Device</rdfs:label>
        <rdfs:isDefinedBy rdf:resource="http://purl.org/iot/vocab/m3-lite#"/>
    </owl:Class>



    <!-- http://purl.org/iot/vocab/iot-taxonomy-lite#Radian -->

    <owl:Class rdf:about="&iottaxolite;Radian">
        <rdfs:subClassOf rdf:resource="&qu;Unit"/>
        <rdfs:comment xml:lang="en">The radian is a unit of angular measure defined such that an angle of one radian subtended from the centre of a unit circle produces an arc with arc length 1.</rdfs:comment>
        <rdfs:label xml:lang="en">Radian</rdfs:label>
        <rdfs:seeAlso rdf:resource="http://sweet.jpl.nasa.gov/ontology/units.owl#radian"/>
        <rdfs:isDefinedBy rdf:resource="http://purl.org/iot/vocab/m3-lite#"/>
    </owl:Class>



    <!-- http://purl.org/iot/vocab/iot-taxonomy-lite#RadianPerSecond -->

    <owl:Class rdf:about="&iottaxolite;RadianPerSecond">
        <rdfs:subClassOf rdf:resource="&qu;Unit"/>
        <rdfs:comment xml:lang="en">The radian per second is defined as the change in the orientation of an object, in radians, every second. The radian per second is the SI unit of angular (rotational) speed.</rdfs:comment>
        <rdfs:label xml:lang="en">Radian Per Second</rdfs:label>
        <rdfs:seeAlso>http://purl.oclc.org/NET/ssnx/qu/unit#radianPerSecond</rdfs:seeAlso>
        <rdfs:isDefinedBy rdf:resource="http://purl.org/iot/vocab/m3-lite#"/>
    </owl:Class>



    <!-- http://purl.org/iot/vocab/iot-taxonomy-lite#Rainfall -->

    <owl:Class rdf:about="&iottaxolite;Rainfall">
        <rdfs:subClassOf rdf:resource="&sosa;ObservableProperty"/>
        <rdfs:comment xml:lang="en">The depth of precipitation (water-equivalent) that accumulated over a measurement time quantity.</rdfs:comment>
        <rdfs:label xml:lang="en">Rainfall</rdfs:label>
        <rdfs:seeAlso>http://sweet.jpl.nasa.gov/ontology/property.owl#Rainfall</rdfs:seeAlso>
        <rdfs:isDefinedBy rdf:resource="http://purl.org/iot/vocab/m3-lite#"/>
    </owl:Class>



    <!-- http://purl.org/iot/vocab/iot-taxonomy-lite#ReactivePower -->

    <owl:Class rdf:about="&iottaxolite;ReactivePower">
        <rdfs:subClassOf rdf:resource="&iottaxolite;Power"/>
        <rdfs:comment xml:lang="en">The portion of electricity that establishes and sustains the electric and magnetic fields of alternating-current equipment.</rdfs:comment>
        <rdfs:label xml:lang="en">Reactive Power</rdfs:label>
        <rdfs:seeAlso>http://purl.oclc.org/NET/ssnx/qu/dim#ReactivePower</rdfs:seeAlso>
        <rdfs:isDefinedBy rdf:resource="http://purl.org/iot/vocab/m3-lite#"/>
    </owl:Class>



    <!-- http://purl.org/iot/vocab/iot-taxonomy-lite#RecognizedActivity -->

    <owl:Class rdf:about="&iottaxolite;RecognizedActivity">
        <rdfs:subClassOf rdf:resource="&sosa;ObservableProperty"/>
        <rdfs:comment xml:lang="en">Activity Recognized. This is usually made available as a part of analysis done by Google. The available activities recognized are IN_VEHICLE, ON_BICYCLE, ON_FOOT, RUNNING, STILL, TILTING, UNKNOWN, and WALKING.</rdfs:comment>
        <rdfs:label xml:lang="en">Recognized Activity</rdfs:label>
        <rdfs:isDefinedBy rdf:resource="http://purl.org/iot/vocab/m3-lite#"/>
    </owl:Class>



    <!-- http://purl.org/iot/vocab/iot-taxonomy-lite#RelativeHumidity -->

    <owl:Class rdf:about="&iottaxolite;RelativeHumidity">
        <rdfs:subClassOf rdf:resource="&sosa;ObservableProperty"/>
        <rdfs:comment xml:lang="en">The ratio of vapour pressure to saturation vapour pressure, where vapour pressure is the pressure exerted by the molecules of water vapour and saturation vapour pressure is the pressure exerted by molecules of water vapour in AIR that has attained saturation.</rdfs:comment>
        <rdfs:label xml:lang="en">Relative Humidity</rdfs:label>
        <rdfs:seeAlso>http://sweet.jpl.nasa.gov/ontology/property.owl#RelativeHumidity</rdfs:seeAlso>
        <rdfs:isDefinedBy rdf:resource="http://purl.org/iot/vocab/m3-lite#"/>
    </owl:Class>



    <!-- http://purl.org/iot/vocab/iot-taxonomy-lite#ResAverageLicConnectedUsers -->

    <owl:Class rdf:about="&iottaxolite;ResAverageLicConnectedUsers">
        <rdfs:subClassOf rdf:resource="&iottaxolite;Communication"/>
        <rdfs:comment xml:lang="en">Connected Users to a communication channel/platform</rdfs:comment>
        <rdfs:label xml:lang="en">Connected Users</rdfs:label>
        <rdfs:isDefinedBy rdf:resource="http://purl.org/iot/vocab/m3-lite#"/>
    </owl:Class>




    <!-- http://purl.org/iot/vocab/iot-taxonomy-lite#RetERabDrop -->

    <owl:Class rdf:about="&iottaxolite;RetERabDrop">
        <rdfs:subClassOf rdf:resource="&iottaxolite;Communication"/>
        <rdfs:comment xml:lang="en">ERAB Drop.</rdfs:comment>
        <rdfs:label xml:lang="en">ERAB Drop</rdfs:label>
        <rdfs:isDefinedBy rdf:resource="http://purl.org/iot/vocab/m3-lite#"/>
    </owl:Class>



    <!-- http://purl.org/iot/vocab/iot-taxonomy-lite#RevolutionsPerMinute -->

    <owl:Class rdf:about="&iottaxolite;RevolutionsPerMinute">
        <rdfs:subClassOf rdf:resource="&qu;Unit"/>
        <rdfs:comment xml:lang="en">Revolutions per minute (abbreviated rpm, RPM, rev/min, r/min) is a measure of the frequency of rotation, specifically the number of rotations around a fixed axis in one minute. It is used as a measure of rotational speed of a mechanical component.</rdfs:comment>
        <rdfs:label xml:lang="en">Revolutions Per Minute</rdfs:label>
        <rdfs:isDefinedBy rdf:resource="http://purl.org/iot/vocab/m3-lite#"/>
    </owl:Class>



    <!-- http://purl.org/iot/vocab/iot-taxonomy-lite#RoadOccupancy -->

    <owl:Class rdf:about="&iottaxolite;RoadOccupancy">
        <rdfs:subClassOf rdf:resource="&sosa;ObservableProperty"/>
        <rdfs:comment xml:lang="en">Ratio of time on which a road lane section is occupied by vehicles within a given period of time.</rdfs:comment>
        <rdfs:label xml:lang="en">Road Occupancy</rdfs:label>
        <rdfs:isDefinedBy rdf:resource="http://purl.org/iot/vocab/m3-lite#"/>
    </owl:Class>



    <!-- http://purl.org/iot/vocab/iot-taxonomy-lite#RoadSurfaceThermometer -->

    <owl:Class rdf:about="&iottaxolite;RoadSurfaceThermometer">
        <rdfs:subClassOf rdf:resource="&iottaxolite;Thermometer"/>
        <rdfs:comment xml:lang="en">Device used to measure the road Surface temperature.</rdfs:comment>
        <rdfs:label xml:lang="en">Road Surface Thermometer</rdfs:label>
        <rdfs:isDefinedBy rdf:resource="http://purl.org/iot/vocab/m3-lite#"/>
    </owl:Class>



    <!-- http://purl.org/iot/vocab/iot-taxonomy-lite#RoadTemperature -->

    <owl:Class rdf:about="&iottaxolite;RoadTemperature">
        <rdfs:subClassOf rdf:resource="&iottaxolite;Temperature"/>
        <rdfs:comment xml:lang="en">Temperature of the road.</rdfs:comment>
        <rdfs:label xml:lang="en">Road Temperature</rdfs:label>
        <rdfs:isDefinedBy rdf:resource="http://purl.org/iot/vocab/m3-lite#"/>
    </owl:Class>



    <!-- http://purl.org/iot/vocab/iot-taxonomy-lite#RoomTemperature -->

    <owl:Class rdf:about="&iottaxolite;RoomTemperature">
        <rdfs:subClassOf rdf:resource="&iottaxolite;BuildingTemperature"/>
        <rdfs:comment xml:lang="en">Temperature of a room.</rdfs:comment>
        <rdfs:label xml:lang="en">Room Temperature</rdfs:label>
        <rdfs:seeAlso rdf:resource="http://elite.polito.it/ontologies/dogont.owl#TemperatureMeasurementMNotification"/>
        <rdfs:seeAlso rdf:resource="http://sensormeasurement.appspot.com/home#RoomTemperature"/>
        <rdfs:isDefinedBy rdf:resource="http://purl.org/iot/vocab/m3-lite#"/>
    </owl:Class>



    <!-- http://purl.org/iot/vocab/iot-taxonomy-lite#RotationalSpeed -->

    <owl:Class rdf:about="&iottaxolite;RotationalSpeed">
        <rdfs:subClassOf rdf:resource="&sosa;ObservableProperty"/>
        <rdfs:label xml:lang="en">Rotational Speed</rdfs:label>
        <rdfs:comment xml:lang="en">Rotational speed (or speed of revolution) of an object rotating around an axis is the number of turns of the object divided by time, specified as revolutions per minute (rpm), revolutions per second (rev/s), or radians per second (rad/s). (Source Wikipedia)</rdfs:comment>
        <rdfs:isDefinedBy rdf:resource="http://purl.org/iot/vocab/m3-lite#"/>
    </owl:Class>



    <!-- http://purl.org/iot/vocab/iot-taxonomy-lite#RotationalSpeedEngine -->

    <owl:Class rdf:about="&iottaxolite;RotationalSpeedEngine">
        <rdfs:subClassOf rdf:resource="&iottaxolite;RotationalSpeed"/>
        <rdfs:comment xml:lang="en">Rotational speed is a property that is the rate of rotation of a material around an axis, in this case the engine cylinders.</rdfs:comment>
        <rdfs:label xml:lang="en">Rotational Speed Engine</rdfs:label>
        <rdfs:seeAlso>http://purl.oclc.org/NET/ssnx/qu/quantity#rotationalSpeed</rdfs:seeAlso>
        <rdfs:isDefinedBy rdf:resource="http://purl.org/iot/vocab/m3-lite#"/>
    </owl:Class>



    <!-- http://purl.org/iot/vocab/iot-taxonomy-lite#SO2Sensor -->

    <owl:Class rdf:about="&iottaxolite;SO2Sensor">
        <rdfs:subClassOf rdf:resource="&iottaxolite;GaseousPollutantSensor"/>
        <rdfs:comment xml:lang="en">Device use to detect Sulphur Dioxide (SO2) level in the environment.</rdfs:comment>
        <rdfs:label xml:lang="en">Sulphur Dioxide (SO2) Sensor</rdfs:label>
        <rdfs:isDefinedBy rdf:resource="http://purl.org/iot/vocab/m3-lite#"/>
    </owl:Class>



    <!-- http://purl.org/iot/vocab/iot-taxonomy-lite#SPO2 -->

    <owl:Class rdf:about="&iottaxolite;SPO2">
        <rdfs:subClassOf rdf:resource="&sosa;ObservableProperty"/>
        <rdfs:comment xml:lang="en">It is a measure of the amount of oxygenated haemoglobin in the blood.</rdfs:comment>
        <rdfs:label xml:lang="en">SPO2</rdfs:label>
        <rdfs:isDefinedBy rdf:resource="http://purl.org/iot/vocab/m3-lite#"/>
    </owl:Class>



    <!-- http://purl.org/iot/vocab/iot-taxonomy-lite#Salinity -->

    <owl:Class rdf:about="&iottaxolite;Salinity">
        <rdfs:subClassOf rdf:resource="&sosa;ObservableProperty"/>
        <rdfs:comment xml:lang="en">It is the measure of all the salts dissolved in water.</rdfs:comment>
        <rdfs:label xml:lang="en">Salinity</rdfs:label>
        <rdfs:isDefinedBy rdf:resource="http://purl.org/iot/vocab/m3-lite#"/>
    </owl:Class>



    <!-- http://purl.org/iot/vocab/iot-taxonomy-lite#SaltMeter -->

    <owl:Class rdf:about="&iottaxolite;SaltMeter">
        <rdfs:subClassOf rdf:resource="&sosa;Sensor"/>
        <rdfs:comment xml:lang="en">Device use to detect salinity of water.</rdfs:comment>
        <rdfs:label xml:lang="en">Salt Meter</rdfs:label>
        <rdfs:isDefinedBy rdf:resource="http://purl.org/iot/vocab/m3-lite#"/>
    </owl:Class>



    <!-- http://purl.org/iot/vocab/iot-taxonomy-lite#Scale -->

    <owl:Class rdf:about="&iottaxolite;Scale">
        <rdfs:subClassOf rdf:resource="&qu;Unit"/>
        <rdfs:comment xml:lang="en">Arbitrary indirect reference which should be translated into meaningful measurements by using the corresponding decoding algorithm detailed in the resource description. In this case the returned values are part of a continuous variable which can take any numeric value.</rdfs:comment>
        <rdfs:label xml:lang="en">Scale</rdfs:label>
        <rdfs:isDefinedBy rdf:resource="http://purl.org/iot/vocab/m3-lite#"/>
    </owl:Class>



    <!-- http://purl.org/iot/vocab/iot-taxonomy-lite#SeatBeltTensionSensor -->

    <owl:Class rdf:about="&iottaxolite;SeatBeltTensionSensor">
        <rdfs:subClassOf rdf:resource="&sosa;Actuator"/>
        <rdfs:comment xml:lang="en"> Actuator used to turn Seat Belt Tension Actuator on or off. </rdfs:comment>
        <rdfs:label xml:lang="en">Seat Belt Tension Actuating Device</rdfs:label>
        <rdfs:isDefinedBy rdf:resource="http://purl.org/iot/vocab/m3-lite#"/>
    </owl:Class>



    <!-- http://purl.org/iot/vocab/iot-taxonomy-lite#SecondAngle -->

    <owl:Class rdf:about="&iottaxolite;SecondAngle">
        <rdfs:subClassOf rdf:resource="&qu;Unit"/>
        <rdfs:comment xml:lang="en">It is a unit of angular measurement equal to 1/60 of one degree.</rdfs:comment>
        <rdfs:label xml:lang="en">Second Angle</rdfs:label>
        <rdfs:isDefinedBy rdf:resource="http://purl.org/iot/vocab/m3-lite#"/>
    </owl:Class>


    <!-- NOT SURE -->
    <!-- http://purl.org/iot/vocab/iot-taxonomy-lite#SecondTime -->

    <owl:Class rdf:about="&iottaxolite;SecondTime">
        <rdfs:subClassOf rdf:resource="&qu;Unit"/>
        <rdfs:comment xml:lang="en">Qualitatively defined as the second division of the hour by sixty, the first division by sixty being the minute. SI definition of second is "the duration of 9 192 631 770 periods of the radiation corresponding to the transition between the two hyperfine levels of the ground state of the cesium 133 atom.</rdfs:comment>
        <rdfs:label xml:lang="en">Second Time</rdfs:label>
        <rdfs:isDefinedBy rdf:resource="http://purl.org/iot/vocab/m3-lite#"/>
    </owl:Class>



    <!-- http://purl.org/iot/vocab/iot-taxonomy-lite#Seismometer -->

    <owl:Class rdf:about="&iottaxolite;Seismometer">
        <rdfs:subClassOf rdf:resource="&sosa;Sensor"/>
        <rdfs:comment xml:lang="en">Seismometers are instruments that measure motions of the ground, including those of seismic waves generated by earthquakes, volcanic eruptions, and other seismic sources.</rdfs:comment>
        <rdfs:label xml:lang="en">Seismometer</rdfs:label>
        <rdfs:isDefinedBy rdf:resource="http://purl.org/iot/vocab/m3-lite#"/>
    </owl:Class>



    <!-- http://purl.org/iot/vocab/iot-taxonomy-lite#ShakeSensor -->

    <owl:Class rdf:about="&iottaxolite;ShakeSensor">
        <rdfs:subClassOf rdf:resource="&sosa;Sensor"/>
        <rdfs:comment xml:lang="en">Shake sensor is used to deduce the quality of the road, earthquakes.</rdfs:comment>
        <rdfs:label xml:lang="en">Shake Sensor</rdfs:label>
        <rdfs:seeAlso rdf:resource="http://casas.wsu.edu/owl/cose.owl#ShakeSensor"/>
        <rdfs:isDefinedBy rdf:resource="http://purl.org/iot/vocab/m3-lite#"/>
    </owl:Class>



    <!-- http://purl.org/iot/vocab/iot-taxonomy-lite#Shower -->

    <owl:Class rdf:about="&iottaxolite;Shower">
        <rdfs:subClassOf rdf:resource="&sosa;Actuator"/>
        <rdfs:comment xml:lang="en">An actuator to automatically switch on/off the shower.</rdfs:comment>
        <rdfs:label xml:lang="en">Shower Actuating Device</rdfs:label>
        <rdfs:isDefinedBy rdf:resource="http://purl.org/iot/vocab/m3-lite#"/>
    </owl:Class>



    <!-- http://purl.org/iot/vocab/iot-taxonomy-lite#Sink -->

    <owl:Class rdf:about="&iottaxolite;Sink">
        <rdfs:subClassOf rdf:resource="&sosa;Actuator"/>
        <rdfs:comment xml:lang="en">An actuator to automatically switch on/off the sink.</rdfs:comment>
        <rdfs:label xml:lang="en">Sink Actuating Device</rdfs:label>
        <rdfs:isDefinedBy rdf:resource="http://purl.org/iot/vocab/m3-lite#"/>
    </owl:Class>



    <!-- http://purl.org/iot/vocab/iot-taxonomy-lite#Sirens -->

    <owl:Class rdf:about="&iottaxolite;Sirens">
        <rdfs:subClassOf rdf:resource="&iottaxolite;SoundSource"/>
        <rdfs:comment xml:lang="en">When source of the sound were sirens either from ambulance, police car or factory etc.</rdfs:comment>
        <rdfs:label xml:lang="en">Sirens Sound Source</rdfs:label>
        <rdfs:isDefinedBy rdf:resource="http://purl.org/iot/vocab/m3-lite#"/>
    </owl:Class>



    <!-- http://purl.org/iot/vocab/iot-taxonomy-lite#SkinConductance -->

    <owl:Class rdf:about="&iottaxolite;SkinConductance">
        <rdfs:subClassOf rdf:resource="&sosa;ObservableProperty"/>
        <rdfs:comment xml:lang="en">Electroderal activity (also known as skin conductance or galvanic skin response) directly correlates to the sympathetic nervous system activity and thus provides a powerful tool for monitoring arousal and certain aspects of autonomic regulation.</rdfs:comment>
        <rdfs:label xml:lang="en">Skin conductance, GSR</rdfs:label>
        <rdfs:isDefinedBy rdf:resource="http://purl.org/iot/vocab/m3-lite#"/>
    </owl:Class>



    <!-- http://purl.org/iot/vocab/iot-taxonomy-lite#SkinConductanceSensor -->

    <owl:Class rdf:about="&iottaxolite;SkinConductanceSensor">
        <rdfs:subClassOf rdf:resource="&sosa;Sensor"/>
        <rdfs:comment xml:lang="en">Device used to detect Skin Conductance.</rdfs:comment>
        <rdfs:label xml:lang="en">Skin Conductance Sensor</rdfs:label>
        <rdfs:isDefinedBy rdf:resource="http://purl.org/iot/vocab/m3-lite#"/>
    </owl:Class>



    <!-- http://purl.org/iot/vocab/iot-taxonomy-lite#SmokeDetector -->

    <owl:Class rdf:about="&iottaxolite;SmokeDetector">
        <rdfs:subClassOf rdf:resource="&sosa;Sensor"/>
        <rdfs:comment xml:lang="en">Device used to detect if there is a fire or the smoke.</rdfs:comment>
        <rdfs:label xml:lang="en">Smoke Detector</rdfs:label>
        <rdfs:seeAlso rdf:resource="http://casas.wsu.edu/owl/cose.owl#SmokeAlarm"/>
        <rdfs:isDefinedBy rdf:resource="http://purl.org/iot/vocab/m3-lite#"/>
    </owl:Class>



    <!-- http://purl.org/iot/vocab/iot-taxonomy-lite#SnowChains -->

    <owl:Class rdf:about="&iottaxolite;SnowChains">
        <rdfs:subClassOf rdf:resource="&sosa;Actuator"/>
        <rdfs:comment xml:lang="en">The actuator that turn Snow chains on/off.</rdfs:comment>
        <rdfs:label xml:lang="en">Snow Chains Actuating Device</rdfs:label>
        <rdfs:isDefinedBy rdf:resource="http://purl.org/iot/vocab/m3-lite#"/>
    </owl:Class>



    <!-- http://purl.org/iot/vocab/iot-taxonomy-lite#Sodium -->

    <owl:Class rdf:about="&iottaxolite;Sodium">
        <rdfs:subClassOf rdf:resource="&sosa;ObservableProperty"/>
        <rdfs:comment xml:lang="en">Measure of Blood Sodium level.</rdfs:comment>
        <rdfs:label xml:lang="en">Sodium</rdfs:label>
        <rdfs:isDefinedBy rdf:resource="http://purl.org/iot/vocab/m3-lite#"/>
    </owl:Class>




    <!-- http://purl.org/iot/vocab/iot-taxonomy-lite#SoilHumidity -->

    <owl:Class rdf:about="&iottaxolite;SoilHumidity">
        <rdfs:subClassOf rdf:resource="&sosa;ObservableProperty"/>
        <rdfs:comment xml:lang="en">It is the quantity of water contained in a material, such as soil. </rdfs:comment>
        <rdfs:label xml:lang="en">Soil Humidity</rdfs:label>
        <rdfs:isDefinedBy rdf:resource="http://purl.org/iot/vocab/m3-lite#"/>
    </owl:Class>



    <!-- http://purl.org/iot/vocab/iot-taxonomy-lite#SoilHumiditySensor -->

    <owl:Class rdf:about="&iottaxolite;SoilHumiditySensor">
        <rdfs:subClassOf rdf:resource="&iottaxolite;HumiditySensor"/>
        <rdfs:comment xml:lang="en">Soil Humidity sensor, Soil moisture, Hygrometer are an instrument used for measuring the soil moisture or soil humidity.</rdfs:comment>
        <rdfs:label xml:lang="en">Soil Humidity Sensor</rdfs:label>
        <rdfs:isDefinedBy rdf:resource="http://purl.org/iot/vocab/m3-lite#"/>
    </owl:Class>



    <!-- http://purl.org/iot/vocab/iot-taxonomy-lite#SoilMoistureTension -->

    <owl:Class rdf:about="&iottaxolite;SoilMoistureTension">
        <rdfs:subClassOf rdf:resource="&sosa;ObservableProperty"/>
        <rdfs:comment xml:lang="en">The force per unit area required to remove film water from soil.</rdfs:comment>
        <rdfs:label xml:lang="en">Soil Moisture Tension</rdfs:label>
        <rdfs:isDefinedBy rdf:resource="http://purl.org/iot/vocab/m3-lite#"/>
    </owl:Class>



    <!-- http://purl.org/iot/vocab/iot-taxonomy-lite#SoilTemperature -->

    <owl:Class rdf:about="&iottaxolite;SoilTemperature">
        <rdfs:subClassOf rdf:resource="&iottaxolite;Temperature"/>
        <rdfs:comment xml:lang="en">Soil temperature is the bulk temperature of the soil, not the surface (skin) temperature.</rdfs:comment>
        <rdfs:label xml:lang="en">Soil Temperature</rdfs:label>
        <rdfs:isDefinedBy rdf:resource="http://purl.org/iot/vocab/m3-lite#"/>
    </owl:Class>



    <!-- http://purl.org/iot/vocab/iot-taxonomy-lite#SolarRadiation -->

    <owl:Class rdf:about="&iottaxolite;SolarRadiation">
        <rdfs:subClassOf rdf:resource="&sosa;ObservableProperty"/>
        <rdfs:comment xml:lang="en">It is the power per unit area received from the Sun in the form of electromagnetic radiation in the wavelength range of the measuring instrument. (Source Wikipedia).</rdfs:comment>
        <rdfs:label xml:lang="en">Solar Radiation Measurement, PAR Measurement (Photosynthetically Active Radiation)</rdfs:label>
        <rdfs:isDefinedBy rdf:resource="http://purl.org/iot/vocab/m3-lite#"/>
    </owl:Class>



    <!-- http://purl.org/iot/vocab/iot-taxonomy-lite#SolarRadiationSensor -->

    <owl:Class rdf:about="&iottaxolite;SolarRadiationSensor">
        <rdfs:subClassOf rdf:resource="&sosa;Sensor"/>
        <rdfs:comment xml:lang="en">Device used to detect Solar Radiation.</rdfs:comment>
        <rdfs:label xml:lang="en">Solar Radiation Sensor</rdfs:label>
        <rdfs:seeAlso rdf:resource="http://purl.oclc.org/NET/ssnx/meteo/aws#RadiationSensor"/>
        <rdfs:seeAlso rdf:resource="http://spitfire-project.eu/ontology/ns/Light"/>
        <rdfs:isDefinedBy rdf:resource="http://purl.org/iot/vocab/m3-lite#"/>
    </owl:Class>



    <!-- http://purl.org/iot/vocab/iot-taxonomy-lite#Sound -->

    <owl:Class rdf:about="&iottaxolite;Sound">
        <rdfs:subClassOf rdf:resource="&sosa;ObservableProperty"/>
        <rdfs:comment xml:lang="en">Measure of noise level in the environment</rdfs:comment>
        <rdfs:label xml:lang="en">Sound, Noise Level</rdfs:label>
        <rdfs:isDefinedBy rdf:resource="http://purl.org/iot/vocab/m3-lite#"/>
    </owl:Class>



    <!-- http://purl.org/iot/vocab/iot-taxonomy-lite#SoundPressureLevel -->

    <owl:Class rdf:about="&iottaxolite;SoundPressureLevel">
        <rdfs:subClassOf rdf:resource="&sosa;ObservableProperty"/>
        <rdfs:comment xml:lang="en">Sound pressure level is a logarithmic measure of the RMS sound pressure of a sound relative to a reference value, the threshold of hearing. The reference sound pressure was chosen conventionally to correspond to the quietest sound at 1000 Hz that the human ear can detect (20 uPa). In this case, the specific parameter is measured in an open environment.</rdfs:comment>
        <rdfs:label xml:lang="en">Sound Pressure Level</rdfs:label>
        <rdfs:seeAlso>http://purl.oclc.org/NET/ssnx/qu/quantity#soundPressure</rdfs:seeAlso>
        <rdfs:isDefinedBy rdf:resource="http://purl.org/iot/vocab/m3-lite#"/>
    </owl:Class>



    <!-- http://purl.org/iot/vocab/iot-taxonomy-lite#SoundPressureLevelAmbient -->

    <owl:Class rdf:about="&iottaxolite;SoundPressureLevelAmbient">
        <rdfs:subClassOf rdf:resource="&iottaxolite;SoundPressureLevel"/>
        <rdfs:label xml:lang="en">Sound Pressure Level Ambient</rdfs:label>
        <rdfs:comment xml:lang="en">Similar to Sound.</rdfs:comment>
        <rdfs:isDefinedBy rdf:resource="http://purl.org/iot/vocab/m3-lite#"/>
    </owl:Class>



    <!-- http://purl.org/iot/vocab/iot-taxonomy-lite#SoundSensor -->

    <owl:Class rdf:about="&iottaxolite;SoundSensor">
        <rdfs:subClassOf rdf:resource="&sosa;Sensor"/>
        <rdfs:comment xml:lang="en">Sensor used to detect Noise level. It can be Sound Sensor, Noise level Sensor, Volume sensor, Microphone</rdfs:comment>
        <rdfs:label xml:lang="en">Sound Sensor</rdfs:label>
        <rdfs:seeAlso rdf:resource="http://casas.wsu.edu/owl/cose.owl#Microphone"/>
        <rdfs:isDefinedBy rdf:resource="http://purl.org/iot/vocab/m3-lite#"/>
    </owl:Class>



    <!-- http://purl.org/iot/vocab/iot-taxonomy-lite#SoundSource -->

    <owl:Class rdf:about="&iottaxolite;SoundSource">
        <rdfs:subClassOf rdf:resource="&iottaxolite;Source"/>
        <rdfs:comment xml:lang="en">Source where the sound originated.</rdfs:comment>
        <rdfs:label xml:lang="en">Sound Source</rdfs:label>
        <rdfs:isDefinedBy rdf:resource="http://purl.org/iot/vocab/m3-lite#"/>
    </owl:Class>



    <!-- http://purl.org/iot/vocab/iot-taxonomy-lite#Source -->

    <owl:Class rdf:about="&iottaxolite;Source">
        <rdfs:comment xml:lang="en">Environmental Origin of a particular observation. With respect to one kind of Source (Sound source), it can be coming from traffic, siren of a police car, etc.</rdfs:comment>
        <rdfs:label xml:lang="en">Source</rdfs:label>
        <rdfs:isDefinedBy rdf:resource="http://purl.org/iot/vocab/m3-lite#"/>
    </owl:Class>



    <!-- http://purl.org/iot/vocab/iot-taxonomy-lite#Speed -->

    <owl:Class rdf:about="&iottaxolite;Speed">
        <rdfs:subClassOf rdf:resource="&sosa;ObservableProperty"/>
        <rdfs:comment xml:lang="en">The rate at which someone or something moves or operates or is able to move or operate.</rdfs:comment>
        <rdfs:label xml:lang="en">Speed</rdfs:label>
        <rdfs:seeAlso>http://purl.oclc.org/NET/ssnx/qu/quantity#speed</rdfs:seeAlso>
        <rdfs:isDefinedBy rdf:resource="http://purl.org/iot/vocab/m3-lite#"/>
    </owl:Class>



    <!-- http://purl.org/iot/vocab/iot-taxonomy-lite#SpeedAverage -->

    <owl:Class rdf:about="&iottaxolite;SpeedAverage">
        <rdfs:subClassOf rdf:resource="&iottaxolite;Speed"/>
        <rdfs:comment xml:lang="en">A measure of the average rate of motion of an object.</rdfs:comment>
        <rdfs:label xml:lang="en">Speed Average</rdfs:label>
        <rdfs:isDefinedBy rdf:resource="http://purl.org/iot/vocab/m3-lite#"/>
    </owl:Class>



    <!-- http://purl.org/iot/vocab/iot-taxonomy-lite#SpeedInstantaneous -->

    <owl:Class rdf:about="&iottaxolite;SpeedInstantaneous">
        <rdfs:subClassOf rdf:resource="&iottaxolite;Speed"/>
        <rdfs:comment xml:lang="en">A measure of the instantaneous rate of motion of an object.</rdfs:comment>
        <rdfs:label xml:lang="en">Speed Instantaneous</rdfs:label>
        <rdfs:isDefinedBy rdf:resource="http://purl.org/iot/vocab/m3-lite#"/>
    </owl:Class>



    <!-- http://purl.org/iot/vocab/iot-taxonomy-lite#SpeedMedian -->

    <owl:Class rdf:about="&iottaxolite;SpeedMedian">
        <rdfs:subClassOf rdf:resource="&iottaxolite;Speed"/>
        <rdfs:comment xml:lang="en">A measure of the median rate of motion of an object.</rdfs:comment>
        <rdfs:label xml:lang="en">Speed Median</rdfs:label>
        <rdfs:isDefinedBy rdf:resource="http://purl.org/iot/vocab/m3-lite#"/>
    </owl:Class>



    <!-- http://purl.org/iot/vocab/iot-taxonomy-lite#SpeedSensor -->

    <owl:Class rdf:about="&iottaxolite;SpeedSensor">
        <rdfs:subClassOf rdf:resource="&sosa;Sensor"/>
        <rdfs:comment xml:lang="en">Sensor used to detect speed.</rdfs:comment>
        <rdfs:label xml:lang="en">Speed Sensor</rdfs:label>
        <rdfs:isDefinedBy rdf:resource="http://purl.org/iot/vocab/m3-lite#"/>
    </owl:Class>



    <!-- http://purl.org/iot/vocab/iot-taxonomy-lite#SunPositionDirection -->

    <owl:Class rdf:about="&iottaxolite;SunPositionDirection">
        <rdfs:subClassOf rdf:resource="&sosa;ObservableProperty"/>
        <rdfs:comment xml:lang="en">The position of the Sun in the sky is a function of both time and the geographic coordinates of the observer on the surface of the Earth. (Source Wikipedia).</rdfs:comment>
        <rdfs:label xml:lang="en">Sun Position Direction</rdfs:label>
        <rdfs:isDefinedBy rdf:resource="http://purl.org/iot/vocab/m3-lite#"/>
    </owl:Class>



    <!-- http://purl.org/iot/vocab/iot-taxonomy-lite#SunPositionDirectionSensor -->

    <owl:Class rdf:about="&iottaxolite;SunPositionDirectionSensor">
        <rdfs:subClassOf rdf:resource="&sosa;Sensor"/>
        <rdfs:comment xml:lang="en">Sensor used to detect sun position.</rdfs:comment>
        <rdfs:label xml:lang="en">Sun Position Direction Sensor</rdfs:label>
        <rdfs:isDefinedBy rdf:resource="http://purl.org/iot/vocab/m3-lite#"/>
    </owl:Class>



    <!-- http://purl.org/iot/vocab/iot-taxonomy-lite#SunPositionElevation -->

    <owl:Class rdf:about="&iottaxolite;SunPositionElevation">
        <rdfs:subClassOf rdf:resource="&sosa;ObservableProperty"/>
        <rdfs:comment xml:lang="en">It is the altitude of the sun, the angle between the horizon and the centre of the sun's disc.</rdfs:comment>
        <rdfs:label xml:lang="en">Sun Position Elevation</rdfs:label>
        <rdfs:isDefinedBy rdf:resource="http://purl.org/iot/vocab/m3-lite#"/>
    </owl:Class>



    <!-- http://purl.org/iot/vocab/iot-taxonomy-lite#SunPositionElevationSensor -->

    <owl:Class rdf:about="&iottaxolite;SunPositionElevationSensor">
        <rdfs:subClassOf rdf:resource="&sosa;Sensor"/>
        <rdfs:comment xml:lang="en">Device used to detect sun elevation.</rdfs:comment>
        <rdfs:label xml:lang="en">Sun Position Elevation Sensor</rdfs:label>
        <rdfs:isDefinedBy rdf:resource="http://purl.org/iot/vocab/m3-lite#"/>
    </owl:Class>



    <!-- http://purl.org/iot/vocab/iot-taxonomy-lite#SystolicBloodPressure -->

    <owl:Class rdf:about="&iottaxolite;SystolicBloodPressure">
        <rdfs:subClassOf rdf:resource="&iottaxolite;BloodPressure"/>
        <rdfs:comment xml:lang="en">It is the pressure when the heart beats while pumping blood.</rdfs:comment>
        <rdfs:label xml:lang="en">Systolic Blood Pressure</rdfs:label>
        <rdfs:isDefinedBy rdf:resource="http://purl.org/iot/vocab/m3-lite#"/>
    </owl:Class>



    <!-- http://purl.org/iot/vocab/iot-taxonomy-lite#TV -->

    <owl:Class rdf:about="&iottaxolite;TV">
        <rdfs:subClassOf rdf:resource="&sosa;Actuator"/>
        <rdfs:comment xml:lang="en">An actuator to automatically switch on/off the television.</rdfs:comment>
        <rdfs:label xml:lang="en">TV Actuating Device</rdfs:label>
        <rdfs:isDefinedBy rdf:resource="http://purl.org/iot/vocab/m3-lite#"/>
    </owl:Class>



    <!-- http://purl.org/iot/vocab/iot-taxonomy-lite#Telephone -->

    <owl:Class rdf:about="&iottaxolite;Telephone">
        <rdfs:subClassOf rdf:resource="&sosa;Actuator"/>
        <rdfs:comment xml:lang="en">An actuator to automatically switch on/off the Telephone.</rdfs:comment>
        <rdfs:label xml:lang="en">Telephone Actuating Device</rdfs:label>
        <rdfs:isDefinedBy rdf:resource="http://purl.org/iot/vocab/m3-lite#"/>
    </owl:Class>



    <!-- http://purl.org/iot/vocab/iot-taxonomy-lite#Temperature -->

    <owl:Class rdf:about="&iottaxolite;Temperature">
        <rdfs:subClassOf rdf:resource="&sosa;ObservableProperty"/>
        <rdfs:comment xml:lang="en">It is the air temperature.</rdfs:comment>
        <rdfs:label xml:lang="en">Temperature</rdfs:label>
        <rdfs:seeAlso rdf:resource="http://archive.knoesis.org/research/semsci/application_domain/sem_sensor/ont/sensor-observation.owlTemperatureProperty"/>
        <rdfs:seeAlso rdf:resource="http://openiot.eu/ontology/ns/Temperature"/>
        <rdfs:seeAlso rdf:resource="http://purl.oclc.org/NET/ssnx/meteo/aws#air_temperature"/>
        <rdfs:isDefinedBy rdf:resource="http://purl.org/iot/vocab/m3-lite#"/>
    </owl:Class>



    <!-- http://purl.org/iot/vocab/iot-taxonomy-lite#TemperatureEngine -->

    <owl:Class rdf:about="&iottaxolite;TemperatureEngine">
        <rdfs:subClassOf rdf:resource="&iottaxolite;Temperature"/>
        <rdfs:comment xml:lang="en">The temperature of a vehicle engine.</rdfs:comment>
        <rdfs:label xml:lang="en">Temperature Engine</rdfs:label>
        <rdfs:isDefinedBy rdf:resource="http://purl.org/iot/vocab/m3-lite#"/>
    </owl:Class>



    <!-- http://purl.org/iot/vocab/iot-taxonomy-lite#TemperatureWasteContainer -->

    <owl:Class rdf:about="&iottaxolite;TemperatureWasteContainer">
        <rdfs:subClassOf rdf:resource="&iottaxolite;Temperature"/>
        <rdfs:comment xml:lang="en">The temperature of the air that would be indicated by a thermometer exposed to the air inside a waste container.</rdfs:comment>
        <rdfs:label xml:lang="en">Temperature Waste Container</rdfs:label>
        <rdfs:isDefinedBy rdf:resource="http://purl.org/iot/vocab/m3-lite#"/>
    </owl:Class>



    <!-- http://purl.org/iot/vocab/iot-taxonomy-lite#Tesla -->

    <owl:Class rdf:about="&iottaxolite;Tesla">
        <rdfs:subClassOf rdf:resource="&qu;Unit"/>
        <rdfs:comment xml:lang="en">It is the SI unit of magnetic flux density.</rdfs:comment>
        <rdfs:label xml:lang="en">Tesla</rdfs:label>
        <rdfs:isDefinedBy rdf:resource="http://purl.org/iot/vocab/m3-lite#"/>
    </owl:Class>



    <!-- http://purl.org/iot/vocab/iot-taxonomy-lite#Thermometer -->

    <owl:Class rdf:about="&iottaxolite;Thermometer">
        <rdfs:subClassOf rdf:resource="&sosa;Sensor"/>
        <rdfs:comment xml:lang="en">A device to measure the temperature in a room or outside.</rdfs:comment>
        <rdfs:label xml:lang="en">Thermometer</rdfs:label>
        <rdfs:seeAlso rdf:resource="http://casas.wsu.edu/owl/cose.owl#TempuratureSensor"/>
        <rdfs:seeAlso rdf:resource="http://purl.oclc.org/NET/ssnx/meteo/aws#TemperatureSensor"/>
        <rdfs:isDefinedBy rdf:resource="http://purl.org/iot/vocab/m3-lite#"/>
    </owl:Class>



    <!-- http://purl.org/iot/vocab/iot-taxonomy-lite#ThrottleSensor -->

    <owl:Class rdf:about="&iottaxolite;ThrottleSensor">
        <rdfs:subClassOf rdf:resource="&sosa;Sensor"/>
        <rdfs:comment xml:lang="en">It is a device used to monitor the throttle position of a vehicle.</rdfs:comment>
        <rdfs:label xml:lang="en">Throttle Position Sensor</rdfs:label>
        <rdfs:isDefinedBy rdf:resource="http://purl.org/iot/vocab/m3-lite#"/>
    </owl:Class>



    <!-- http://purl.org/iot/vocab/iot-taxonomy-lite#TimeRelatedState -->

    <owl:Class rdf:about="&iottaxolite;TimeRelatedState">
        <rdfs:subClassOf rdf:resource="&sosa;ObservableProperty"/>
        <rdfs:label xml:lang="en">Time Related State</rdfs:label>
        <rdfs:comment xml:lang="en">Indicator of whether a person (or object) has overpassed a particular time threshold (e.g. maximum number of hours driving, etc.)</rdfs:comment>
        <rdfs:isDefinedBy rdf:resource="http://purl.org/iot/vocab/m3-lite#"/>
    </owl:Class>


    <!-- NOT SURE -->
    <!-- http://purl.org/iot/vocab/iot-taxonomy-lite#TimeRelatedStateDriver -->

    <owl:Class rdf:about="&iottaxolite;TimeRelatedStateDriver">
        <rdfs:subClassOf rdf:resource="&iottaxolite;TimeRelatedState"/>
        <rdfs:label xml:lang="en">Time Related State Driver</rdfs:label>
        <rdfs:comment xml:lang="en">Indicator of whether the driver of a vehicle approaches or exceeds his/her working time limits.</rdfs:comment>
        <rdfs:isDefinedBy rdf:resource="http://purl.org/iot/vocab/m3-lite#"/>
    </owl:Class>



    <!-- http://purl.org/iot/vocab/iot-taxonomy-lite#TimeRelatedStateDriverOne -->

    <owl:Class rdf:about="&iottaxolite;TimeRelatedStateDriverOne">
        <rdfs:subClassOf rdf:resource="&iottaxolite;TimeRelatedStateDriver"/>
        <rdfs:comment xml:lang="en">Indicates if the first driver approaches or exceeds working time limits (or other limits).</rdfs:comment>
        <rdfs:label xml:lang="en">Time Related State Driver 1</rdfs:label>
        <rdfs:isDefinedBy rdf:resource="http://purl.org/iot/vocab/m3-lite#"/>
    </owl:Class>



    <!-- http://purl.org/iot/vocab/iot-taxonomy-lite#TimeRelatedStateDriverTwo -->

    <owl:Class rdf:about="&iottaxolite;TimeRelatedStateDriverTwo">
        <rdfs:subClassOf rdf:resource="&iottaxolite;TimeRelatedStateDriver"/>
        <rdfs:comment xml:lang="en">Indicates if the second driver approaches or exceeds working time limits (or other limits).</rdfs:comment>
        <rdfs:label xml:lang="en">Time Related State Driver 2</rdfs:label>
        <rdfs:isDefinedBy rdf:resource="http://purl.org/iot/vocab/m3-lite#"/>
    </owl:Class>



    <!-- http://purl.org/iot/vocab/iot-taxonomy-lite#Timestamp -->

    <owl:Class rdf:about="&iottaxolite;Timestamp">
        <rdfs:subClassOf rdf:resource="&sosa;ObservableProperty"/>
        <rdfs:comment xml:lang="en">Sequence of characters or encoded information identifying when a certain event occurred, usually giving date and time of day, sometimes accurate to a small fraction of a second. This representation should be encoded following ISO8601.</rdfs:comment>
        <rdfs:label xml:lang="en">Timestamp</rdfs:label>
        <rdfs:seeAlso>http://sweet.jpl.nasa.gov/2.3/propTime.owl#Timestamp</rdfs:seeAlso>
        <rdfs:isDefinedBy rdf:resource="http://purl.org/iot/vocab/m3-lite#"/>
    </owl:Class>





    <!-- http://purl.org/iot/vocab/iot-taxonomy-lite#Tonne -->

    <owl:Class rdf:about="&iottaxolite;Tonne">
        <rdfs:subClassOf rdf:resource="&iottaxolite;Gram"/>
        <rdfs:comment xml:lang="en">It is a non-SI metric unit of mass equal to 1,000 kilograms.</rdfs:comment>
        <rdfs:label xml:lang="en">Tonne</rdfs:label>
        <rdfs:isDefinedBy rdf:resource="http://purl.org/iot/vocab/m3-lite#"/>
    </owl:Class>



    <!-- http://purl.org/iot/vocab/iot-taxonomy-lite#TouchSensor -->

    <owl:Class rdf:about="&iottaxolite;TouchSensor">
        <rdfs:subClassOf rdf:resource="&sosa;Sensor"/>
        <rdfs:comment xml:lang="en">Device that captures and records physical touch or embrace on a device and/or object.</rdfs:comment>
        <rdfs:label xml:lang="en">Touch Sensor</rdfs:label>
        <rdfs:isDefinedBy rdf:resource="http://purl.org/iot/vocab/m3-lite#"/>
    </owl:Class>



    <!-- http://purl.org/iot/vocab/iot-taxonomy-lite#Tourism -->

    <owl:Class rdf:about="&iottaxolite;Tourism">
        <rdfs:subClassOf rdf:resource="&iottaxolite;DomainOfInterest"/>
        <rdfs:comment xml:lang="en">Tourism as an Internet of Things (IoT) applicative domain.</rdfs:comment>
        <rdfs:label xml:lang="en">Tourism DOI</rdfs:label>
        <rdfs:isDefinedBy rdf:resource="http://purl.org/iot/vocab/m3-lite#"/>
    </owl:Class>

    <!-- http://purl.org/iot/vocab/iot-taxonomy-lite#Traffic -->

    <owl:Class rdf:about="&iottaxolite;Traffic">
        <rdfs:subClassOf rdf:resource="&iottaxolite;SoundSource"/>
        <rdfs:comment xml:lang="en">When the source of the sound was traffic.</rdfs:comment>
        <rdfs:label xml:lang="en">Traffic</rdfs:label>
        <rdfs:isDefinedBy rdf:resource="http://purl.org/iot/vocab/m3-lite#"/>
    </owl:Class>

    <!-- http://purl.org/iot/vocab/iot-taxonomy-lite#Transportation -->

    <owl:Class rdf:about="&iottaxolite;Transportation">
        <rdfs:subClassOf rdf:resource="&iottaxolite;DomainOfInterest"/>
        <rdfs:comment xml:lang="en">Transportation, Smart Car/Vehicle, Intelligent Transport System (ITS) as an Internet of Things (IoT) applicative domain.</rdfs:comment>
        <rdfs:label xml:lang="en">Transportation DOI</rdfs:label>
        <rdfs:isDefinedBy rdf:resource="http://purl.org/iot/vocab/m3-lite#"/>
    </owl:Class>



    <!-- http://purl.org/iot/vocab/iot-taxonomy-lite#UltrasonicSensor -->

    <owl:Class rdf:about="&iottaxolite;UltrasonicSensor">
        <rdfs:subClassOf rdf:resource="&sosa;Sensor"/>
        <rdfs:comment xml:lang="en">Ultrasonic sensors are used to deduce human posture in smart home for example.</rdfs:comment>
        <rdfs:label xml:lang="en">Ultrasonic Sensor</rdfs:label>
        <rdfs:isDefinedBy rdf:resource="http://purl.org/iot/vocab/m3-lite#"/>
    </owl:Class>



    <!-- http://purl.org/iot/vocab/iot-taxonomy-lite#VehicleCountSensor -->

    <owl:Class rdf:about="&iottaxolite;VehicleCountSensor">
        <rdfs:subClassOf rdf:resource="&iottaxolite;Counter"/>
        <rdfs:comment xml:lang="en">Device used to count the number of vehicles (e.g., used within the Citypulse project).</rdfs:comment>
        <rdfs:label xml:lang="en">Vehicle Count Sensor</rdfs:label>
        <rdfs:isDefinedBy rdf:resource="http://purl.org/iot/vocab/m3-lite#"/>
    </owl:Class>



    <!-- http://purl.org/iot/vocab/iot-taxonomy-lite#VehicleOverspeedState -->

    <owl:Class rdf:about="&iottaxolite;VehicleOverspeedState">
        <rdfs:subClassOf rdf:resource="&sosa;ObservableProperty"/>
        <rdfs:comment xml:lang="en">Measure to indicates whether the vehicle is exceeding the legal speed limit.</rdfs:comment>
        <rdfs:label xml:lang="en">Vehicle Overspeed State</rdfs:label>
        <rdfs:isDefinedBy rdf:resource="http://purl.org/iot/vocab/m3-lite#"/>
    </owl:Class>



    <!-- http://purl.org/iot/vocab/iot-taxonomy-lite#VehiclesPerMinute -->

    <owl:Class rdf:about="&iottaxolite;VehiclesPerMinute">
        <rdfs:subClassOf rdf:resource="&qu;Unit"/>
        <rdfs:comment xml:lang="en">Number of vehicles that traverse a concrete region of the space in one minute.</rdfs:comment>
        <rdfs:label xml:lang="en">Vehicles Per Minute</rdfs:label>
        <rdfs:isDefinedBy rdf:resource="http://purl.org/iot/vocab/m3-lite#"/>
    </owl:Class>



    <!-- http://purl.org/iot/vocab/iot-taxonomy-lite#Ventilation -->

    <owl:Class rdf:about="&iottaxolite;Ventilation">
        <rdfs:subClassOf rdf:resource="&sosa;Actuator"/>
        <rdfs:comment xml:lang="en">An actuator to automatically open/close the ventilation.</rdfs:comment>
        <rdfs:label xml:lang="en">Ventilation Actuating Device</rdfs:label>
        <rdfs:isDefinedBy rdf:resource="http://purl.org/iot/vocab/m3-lite#"/>
    </owl:Class>



    <!-- http://purl.org/iot/vocab/iot-taxonomy-lite#Visibility -->

    <owl:Class rdf:about="&iottaxolite;Visibility">
        <rdfs:subClassOf rdf:resource="&sosa;ObservableProperty"/>
        <rdfs:comment xml:lang="en">The state of being able to see or be seen.</rdfs:comment>
        <rdfs:label xml:lang="en">Visibility</rdfs:label>
        <rdfs:seeAlso rdf:resource="http://openiot.eu/ontology/ns/AtmosphereVisibility"/>
        <rdfs:isDefinedBy rdf:resource="http://purl.org/iot/vocab/m3-lite#"/>
    </owl:Class>



    <!-- http://purl.org/iot/vocab/iot-taxonomy-lite#VisibilitySensor -->

    <owl:Class rdf:about="&iottaxolite;VisibilitySensor">
        <rdfs:subClassOf rdf:resource="&sosa;Sensor"/>
        <rdfs:comment xml:lang="en">Device used to detect Visibility.</rdfs:comment>
        <rdfs:label xml:lang="en">Visibility Sensor</rdfs:label>
        <rdfs:isDefinedBy rdf:resource="http://purl.org/iot/vocab/m3-lite#"/>
    </owl:Class>



    <!-- http://purl.org/iot/vocab/iot-taxonomy-lite#Volt -->

    <owl:Class rdf:about="&iottaxolite;Volt">
        <rdfs:subClassOf rdf:resource="&qu;Unit"/>
        <rdfs:comment xml:lang="en">The SI unit of electromotive force, the difference of potential that would carry one ampere of current against one ohm resistance.</rdfs:comment>
        <rdfs:label xml:lang="en">Volt</rdfs:label>
        <rdfs:seeAlso rdf:resource="http://sweet.jpl.nasa.gov/ontology/units.owl#volt"/>
        <rdfs:isDefinedBy rdf:resource="http://purl.org/iot/vocab/m3-lite#"/>
    </owl:Class>



    <!-- http://purl.org/iot/vocab/iot-taxonomy-lite#VoltAmpereReactive -->

    <owl:Class rdf:about="&iottaxolite;VoltAmpereReactive">
        <rdfs:subClassOf rdf:resource="&qu;Unit"/>
        <rdfs:comment xml:lang="en">In electric power transmission and distribution, volt-ampere reactive (var) is a unit in which reactive power is expressed in an AC electric power system.</rdfs:comment>
        <rdfs:label xml:lang="en">Volt Ampere Reactive, VAR</rdfs:label>
        <rdfs:seeAlso>http://purl.oclc.org/NET/ssnx/qu/unit#var</rdfs:seeAlso>
        <rdfs:isDefinedBy rdf:resource="http://purl.org/iot/vocab/m3-lite#"/>
    </owl:Class>



    <!-- http://purl.org/iot/vocab/iot-taxonomy-lite#VoltageSensor -->

    <owl:Class rdf:about="&iottaxolite;VoltageSensor">
        <rdfs:subClassOf rdf:resource="&sosa;Sensor"/>
        <rdfs:comment xml:lang="en">Device which can measure the difference in electric potential energy between two points per unit electric charge.</rdfs:comment>
        <rdfs:label xml:lang="en">Voltage Sensor</rdfs:label>
        <rdfs:isDefinedBy rdf:resource="http://purl.org/iot/vocab/m3-lite#"/>
    </owl:Class>



    <!-- http://purl.org/iot/vocab/iot-taxonomy-lite#WashingMachine -->

    <owl:Class rdf:about="&iottaxolite;WashingMachine">
        <rdfs:subClassOf rdf:resource="&sosa;Actuator"/>
        <rdfs:comment xml:lang="en">An actuator to automatically switch on/off the washing machine.</rdfs:comment>
        <rdfs:label xml:lang="en">Washing Machine Actuation Device</rdfs:label>
        <rdfs:isDefinedBy rdf:resource="http://purl.org/iot/vocab/m3-lite#"/>
    </owl:Class>



    <!-- http://purl.org/iot/vocab/iot-taxonomy-lite#WaterLevel -->

    <owl:Class rdf:about="&iottaxolite;WaterLevel">
        <rdfs:subClassOf rdf:resource="&sosa;ObservableProperty"/>
        <rdfs:comment xml:lang="en">The height reached by the water in a reservoir, river, storage tank, or similar.</rdfs:comment>
        <rdfs:label xml:lang="en">Water Level</rdfs:label>
        <rdfs:isDefinedBy rdf:resource="http://purl.org/iot/vocab/m3-lite#"/>
    </owl:Class>



    <!-- http://purl.org/iot/vocab/iot-taxonomy-lite#WaterTemperature -->

    <owl:Class rdf:about="&iottaxolite;WaterTemperature">
        <rdfs:subClassOf rdf:resource="&iottaxolite;Temperature"/>
        <rdfs:comment xml:lang="en">Sea surface temperature (SST) is the water temperature close to the ocean's surface.</rdfs:comment>
        <rdfs:label xml:lang="en">Water Temperature</rdfs:label>
        <rdfs:isDefinedBy rdf:resource="http://purl.org/iot/vocab/m3-lite#"/>
    </owl:Class>



    <!-- http://purl.org/iot/vocab/iot-taxonomy-lite#Watt -->

    <owl:Class rdf:about="&iottaxolite;Watt">
        <rdfs:subClassOf rdf:resource="&qu;Unit"/>
        <rdfs:comment xml:lang="en">It is the SI unit of power, equivalent to one joule per second, corresponding to the rate of consumption of energy in an electric circuit where the potential difference is one volt and the current one ampere.</rdfs:comment>
        <rdfs:label xml:lang="en">Watt (W)</rdfs:label>
        <rdfs:seeAlso rdf:resource="http://sweet.jpl.nasa.gov/ontology/units.owl#watt"/>
        <rdfs:isDefinedBy rdf:resource="http://purl.org/iot/vocab/m3-lite#"/>
    </owl:Class>




    <!-- http://purl.org/iot/vocab/iot-taxonomy-lite#WattPerSquareMetre -->

    <owl:Class rdf:about="&iottaxolite;WattPerSquareMetre">
        <rdfs:subClassOf rdf:resource="&qu;Unit"/>
        <rdfs:comment xml:lang="en">It is the SI unit for radiative and other energy fluxes.</rdfs:comment>
        <rdfs:label xml:lang="en">Watt Per Square Metre, Watt Per Square Meter</rdfs:label>
        <rdfs:seeAlso>http://purl.oclc.org/NET/ssnx/qu/unit#wattPerSquareMetre</rdfs:seeAlso>
        <rdfs:isDefinedBy rdf:resource="http://purl.org/iot/vocab/m3-lite#"/>
    </owl:Class>

    <!--  http://purl.org/iot/vocab/iot-taxonomy-lite#MicrowattPerSquareCentimetre -->

    <owl:Class rdf:about="&iottaxolite;MicrowattPerSquareCentimetre">
        <rdfs:subClassOf rdf:resource="&iottaxolite;WattPerSquareMetre"/>
        <rdfs:comment xml:lang="en">It is one of the unit for radiative and other energy fluxes.</rdfs:comment>
        <rdfs:label xml:lang="en">Microwatt Per Square Centimetre, Microwatt Per Square Centimeter</rdfs:label>
        <rdfs:isDefinedBy rdf:resource="http://purl.org/iot/vocab/m3-lite#"/>
    </owl:Class>


    <!-- http://purl.org/iot/vocab/iot-taxonomy-lite#Weather -->

    <owl:Class rdf:about="&iottaxolite;Weather">
        <rdfs:subClassOf rdf:resource="&iottaxolite;DomainOfInterest"/>
        <rdfs:comment xml:lang="en">Weather Forecasting, Meterology as an Internet of Things (IoT) applicative domain.</rdfs:comment>
        <rdfs:label xml:lang="en">Weather Forecasting DOI</rdfs:label>
        <rdfs:seeAlso rdf:resource="http://archive.knoesis.org/research/semsci/application_domain/sem_sensor/ont/sensor-observation.owlWeatherObservation"/>
        <rdfs:isDefinedBy rdf:resource="http://purl.org/iot/vocab/m3-lite#"/>
    </owl:Class>



    <!-- http://purl.org/iot/vocab/iot-taxonomy-lite#WeatherLuminosity -->

    <owl:Class rdf:about="&iottaxolite;WeatherLuminosity">
        <rdfs:subClassOf rdf:resource="&iottaxolite;Illuminance"/>
        <rdfs:comment xml:lang="en">Luminosity in the weather</rdfs:comment>
        <rdfs:label xml:lang="en">Weather Luminosity</rdfs:label>
        <rdfs:isDefinedBy rdf:resource="http://purl.org/iot/vocab/m3-lite#"/>
    </owl:Class>



    <!-- http://purl.org/iot/vocab/iot-taxonomy-lite#WeatherPrecipitation -->

    <owl:Class rdf:about="&iottaxolite;WeatherPrecipitation">
        <rdfs:subClassOf rdf:resource="&iottaxolite;Precipitation"/>
        <rdfs:comment xml:lang="en">Weather Precipitation.</rdfs:comment>
        <rdfs:label xml:lang="en">Weather Precipitation</rdfs:label>
        <rdfs:isDefinedBy rdf:resource="http://purl.org/iot/vocab/m3-lite#"/>
    </owl:Class>



    <!-- http://purl.org/iot/vocab/iot-taxonomy-lite#Weight -->

    <owl:Class rdf:about="&iottaxolite;Weight">
        <rdfs:subClassOf rdf:resource="&sosa;ObservableProperty"/>
        <rdfs:comment xml:lang="en">A body's relative mass or the quantity of matter contained by it, giving rise to a downward force; the heaviness of a person or thing.</rdfs:comment>
        <rdfs:label xml:lang="en">Weight</rdfs:label>
        <rdfs:isDefinedBy rdf:resource="http://purl.org/iot/vocab/m3-lite#"/>
    </owl:Class>



    <!-- http://purl.org/iot/vocab/iot-taxonomy-lite#WeightSensor -->

    <owl:Class rdf:about="&iottaxolite;WeightSensor">
        <rdfs:subClassOf rdf:resource="&sosa;Sensor"/>
        <rdfs:comment xml:lang="en">Device used to weight an object.</rdfs:comment>
        <rdfs:label xml:lang="en">Weight Sensor</rdfs:label>
        <rdfs:isDefinedBy rdf:resource="http://purl.org/iot/vocab/m3-lite#"/>
    </owl:Class>



    <!-- http://purl.org/iot/vocab/iot-taxonomy-lite#WindChill -->

    <owl:Class rdf:about="&iottaxolite;WindChill">
        <rdfs:subClassOf rdf:resource="&sosa;ObservableProperty"/>
        <rdfs:comment xml:lang="en">The cooling effect of wind blowing on a surface.</rdfs:comment>
        <rdfs:label xml:lang="en">Wind Chill</rdfs:label>
        <rdfs:seeAlso rdf:resource="http://openiot.eu/ontology/ns/WindChill"/>
        <rdfs:isDefinedBy rdf:resource="http://purl.org/iot/vocab/m3-lite#"/>
    </owl:Class>



    <!-- http://purl.org/iot/vocab/iot-taxonomy-lite#WindChillSensor -->

    <owl:Class rdf:about="&iottaxolite;WindChillSensor">
        <rdfs:subClassOf rdf:resource="&sosa;Sensor"/>
        <rdfs:comment xml:lang="en">Device used to detect Wind Chill.</rdfs:comment>
        <rdfs:label xml:lang="en">Wind Chill Sensor</rdfs:label>
        <rdfs:isDefinedBy rdf:resource="http://purl.org/iot/vocab/m3-lite#"/>
    </owl:Class>



    <!-- http://purl.org/iot/vocab/iot-taxonomy-lite#WindDirection -->

    <owl:Class rdf:about="&iottaxolite;WindDirection">
        <rdfs:subClassOf rdf:resource="&sosa;ObservableProperty"/>
        <rdfs:comment xml:lang="en">The geodetic azimuth of the direction from which the wind is blowing.</rdfs:comment>
        <rdfs:label xml:lang="en">Wind Direction</rdfs:label>
        <rdfs:seeAlso rdf:resource="http://paul.staroch.name/thesis/SmartHomeWeather.owl#DirectionalWind"/>
        <rdfs:isDefinedBy rdf:resource="http://purl.org/iot/vocab/m3-lite#"/>
    </owl:Class>



    <!-- http://purl.org/iot/vocab/iot-taxonomy-lite#WindDirectionSensor -->

    <owl:Class rdf:about="&iottaxolite;WindDirectionSensor">
        <rdfs:subClassOf rdf:resource="&sosa;Sensor"/>
        <rdfs:comment xml:lang="en">Device used to detect wind direction.</rdfs:comment>
        <rdfs:label xml:lang="en">Wind Direction Sensor</rdfs:label>
        <rdfs:isDefinedBy rdf:resource="http://purl.org/iot/vocab/m3-lite#"/>
    </owl:Class>



    <!-- http://purl.org/iot/vocab/iot-taxonomy-lite#WindSpeed -->

    <owl:Class rdf:about="&iottaxolite;WindSpeed">
        <rdfs:subClassOf rdf:resource="&sosa;ObservableProperty"/>
        <rdfs:comment xml:lang="en">The ratio of the distance covered by moving air to the time quantity taken to cover it.</rdfs:comment>
        <rdfs:label xml:lang="en">Wind Velocity, Wind Speed</rdfs:label>
        <rdfs:seeAlso rdf:resource="http://openiot.eu/ontology/ns/WindSpeed"/>
        <rdfs:isDefinedBy rdf:resource="http://purl.org/iot/vocab/m3-lite#"/>
    </owl:Class>



    <!-- http://purl.org/iot/vocab/iot-taxonomy-lite#WindSpeedSensor -->

    <owl:Class rdf:about="&iottaxolite;WindSpeedSensor">
        <rdfs:subClassOf rdf:resource="&iottaxolite;SpeedSensor"/>
        <rdfs:comment xml:lang="en">Wind Speed Sensor, Anemometer or Wind Velocity Sensor is used to measure the wind speed.</rdfs:comment>
        <rdfs:label xml:lang="en">Wind Speed Sensor</rdfs:label>
        <rdfs:isDefinedBy rdf:resource="http://purl.org/iot/vocab/m3-lite#"/>
    </owl:Class>



    <!-- http://purl.org/iot/vocab/iot-taxonomy-lite#Window -->

    <owl:Class rdf:about="&iottaxolite;Window">
        <rdfs:subClassOf rdf:resource="&sosa;Actuator"/>
        <rdfs:comment xml:lang="en">An actuator to automatically open/close the window.</rdfs:comment>
        <rdfs:label xml:lang="en">Window Actuating Device</rdfs:label>
        <rdfs:isDefinedBy rdf:resource="http://purl.org/iot/vocab/m3-lite#"/>
    </owl:Class>


    <!-- NOT SURE -->
    <!-- http://purl.org/iot/vocab/iot-taxonomy-lite#WorkingState -->

    <owl:Class rdf:about="&iottaxolite;WorkingState">
        <rdfs:subClassOf rdf:resource="&sosa;ObservableProperty"/>
        <rdfs:label xml:lang="en">Working State</rdfs:label>
        <rdfs:comment xml:lang="en">Indicator of whether a person (or object) is working or not</rdfs:comment>
        <rdfs:isDefinedBy rdf:resource="http://purl.org/iot/vocab/m3-lite#"/>
    </owl:Class>


    <!-- NOT SURE -->
    <!-- http://purl.org/iot/vocab/iot-taxonomy-lite#WorkingStateDriver -->

    <owl:Class rdf:about="&iottaxolite;WorkingStateDriver">
        <rdfs:subClassOf rdf:resource="&iottaxolite;WorkingState"/>
        <rdfs:label xml:lang="en">Working State Driver</rdfs:label>
        <rdfs:comment xml:lang="en">Indicator of whether the driver of a vehicle is present or not</rdfs:comment>
        <rdfs:isDefinedBy rdf:resource="http://purl.org/iot/vocab/m3-lite#"/>
    </owl:Class>



    <!-- http://purl.org/iot/vocab/iot-taxonomy-lite#WorkingStateDriverOne -->

    <owl:Class rdf:about="&iottaxolite;WorkingStateDriverOne">
        <rdfs:subClassOf rdf:resource="&iottaxolite;WorkingStateDriver"/>
        <rdfs:comment xml:lang="en">State of work of the first driver as defined in the FMS standard.</rdfs:comment>
        <rdfs:label xml:lang="en">Working State Driver 1</rdfs:label>
        <rdfs:isDefinedBy rdf:resource="http://purl.org/iot/vocab/m3-lite#"/>
    </owl:Class>



    <!-- http://purl.org/iot/vocab/iot-taxonomy-lite#WorkingStateDriverTwo -->

    <owl:Class rdf:about="&iottaxolite;WorkingStateDriverTwo">
        <rdfs:subClassOf rdf:resource="&iottaxolite;WorkingStateDriver"/>
        <rdfs:comment xml:lang="en">State of work of the second driver as defined in the FMS standard.</rdfs:comment>
        <rdfs:label xml:lang="en">Working State Driver 2</rdfs:label>
        <rdfs:isDefinedBy rdf:resource="http://purl.org/iot/vocab/m3-lite#"/>
    </owl:Class>



    <!-- http://purl.org/iot/vocab/iot-taxonomy-lite#Wout -->

    <owl:Class rdf:about="&iottaxolite;Wout">
        <rdfs:subClassOf rdf:resource="&qu;Unit"/>
        <rdfs:comment xml:lang="en">This unit is used to measure delta dew point. Natural number (W/out unit).</rdfs:comment>
        <rdfs:label xml:lang="en">W/out</rdfs:label>
        <rdfs:isDefinedBy rdf:resource="http://purl.org/iot/vocab/m3-lite#"/>
    </owl:Class>



    <!-- http://purl.org/iot/vocab/iot-taxonomy-lite#Year -->

    <owl:Class rdf:about="&iottaxolite;Year">
        <rdfs:subClassOf rdf:resource="&iottaxolite;SecondTime"/>
        <rdfs:comment xml:lang="en">Year as a unit of time.</rdfs:comment>
        <rdfs:label xml:lang="en">Year</rdfs:label>
        <rdfs:seeAlso rdf:resource="http://sweet.jpl.nasa.gov/ontology/units.owl#year"/>
        <rdfs:isDefinedBy rdf:resource="http://purl.org/iot/vocab/m3-lite#"/>
    </owl:Class>



    <!-- http://purl.org/iot/vocab/iot-taxonomy-lite#ChemicalAgentAtmosphericConcentrationO3 -->

    <owl:Class rdf:about="&iottaxolite;ChemicalAgentAtmosphericConcentrationO3">
        <rdfs:subClassOf rdf:resource="&iottaxolite;ChemicalAgentAtmosphericConcentration"/>
        <rdfs:comment xml:lang="en">The concentration of ozone (O3) gas suspended in the atmosphere.</rdfs:comment>
        <rdfs:label xml:lang="en">Chemical Agent Atmospheric Concentration O3</rdfs:label>
        <rdfs:isDefinedBy rdf:resource="http://purl.org/iot/vocab/m3-lite#"/>
    </owl:Class>



    <!-- http://purl.org/iot/vocab/iot-taxonomy-lite#IntDlThroughputKbps -->

    <owl:Class rdf:about="&iottaxolite;IntDlThroughputKbps">
        <rdfs:subClassOf rdf:resource="&iottaxolite;Communication"/>
        <rdfs:comment xml:lang="en">Downlink Throughput.</rdfs:comment>
        <rdfs:label xml:lang="en">Downlink Throughput</rdfs:label>
        <rdfs:isDefinedBy rdf:resource="http://purl.org/iot/vocab/m3-lite#"/>
    </owl:Class>



    <!-- http://purl.org/iot/vocab/iot-taxonomy-lite#IntUlPacketLoss -->

    <owl:Class rdf:about="&iottaxolite;IntUlPacketLoss">
        <rdfs:subClassOf rdf:resource="&iottaxolite;Communication"/>
        <rdfs:comment xml:lang="en">Uplink Packet Loss.</rdfs:comment>
        <rdfs:label xml:lang="en">Uplink Packet Loss</rdfs:label>
        <rdfs:isDefinedBy rdf:resource="http://purl.org/iot/vocab/m3-lite#"/>
    </owl:Class>



    <!-- http://purl.org/iot/vocab/iot-taxonomy-lite#IntUlThroughputKbps -->

    <owl:Class rdf:about="&iottaxolite;IntUlThroughputKbps">
        <rdfs:subClassOf rdf:resource="&iottaxolite;Communication"/>
        <rdfs:comment xml:lang="en">Uplink Throughput.</rdfs:comment>
        <rdfs:label xml:lang="en">Uplink Throughput</rdfs:label>
        <rdfs:isDefinedBy rdf:resource="http://purl.org/iot/vocab/m3-lite#"/>
    </owl:Class>

<!-- http://purl.org/iot/vocab/iot-taxonomy-lite#Item -->

    <owl:Class rdf:about="&iottaxolite;Item">
        <rdfs:subClassOf rdf:resource="&qu;Unit"/>
        <rdfs:comment xml:lang="en">Each of the accountable elements within a group.</rdfs:comment>
        <rdfs:label xml:lang="en">Item</rdfs:label>
        <rdfs:isDefinedBy rdf:resource="http://purl.org/iot/vocab/m3-lite#"/>
    </owl:Class>
    

    <!-- http://purl.org/iot/vocab/iot-taxonomy-lite#Count -->

    <owl:Class rdf:about="&iottaxolite;Count">
        <rdfs:subClassOf rdf:resource="&sosa;ObservableProperty"/>
        <rdfs:comment xml:lang="en">Number of available particular things.</rdfs:comment>
        <rdfs:label xml:lang="en">Count</rdfs:label>
        <rdfs:isDefinedBy rdf:resource="http://purl.org/iot/vocab/m3-lite#"/>
    </owl:Class>

    <!-- http://purl.org/iot/vocab/iot-taxonomy-lite#DoorStatus -->

    <owl:Class rdf:about="&iottaxolite;DoorStatus">
        <rdfs:subClassOf rdf:resource="&sosa;ObservableProperty"/>
        <rdfs:comment xml:lang="en">Describes if a door is OPEN or CLOSED.</rdfs:comment>
        <rdfs:label xml:lang="en">Door Status</rdfs:label>
        <rdfs:isDefinedBy rdf:resource="http://purl.org/iot/vocab/m3-lite#"/>
    </owl:Class>

    <!-- http://purl.org/iot/vocab/iot-taxonomy-lite#CountAvailableBicycles -->

    <owl:Class rdf:about="&iottaxolite;CountAvailableBicycles">
        <rdfs:subClassOf rdf:resource="&iottaxolite;Count"/>
        <rdfs:comment xml:lang="en">Number of available bicycles at a particular bicycle docking station.</rdfs:comment>
        <rdfs:label xml:lang="en">Count Available Bicycles</rdfs:label>
        <rdfs:isDefinedBy rdf:resource="http://purl.org/iot/vocab/m3-lite#"/>
    </owl:Class>

    <!-- http://purl.org/iot/vocab/iot-taxonomy-lite#CountAvailableTaxis -->

    <owl:Class rdf:about="&iottaxolite;CountAvailableTaxis">
        <rdfs:subClassOf rdf:resource="&iottaxolite;Count"/>
        <rdfs:comment xml:lang="en">Number of taxis available at a particular taxi stop.</rdfs:comment>
        <rdfs:label xml:lang="en">Count Available Taxis</rdfs:label>
        <rdfs:isDefinedBy rdf:resource="http://purl.org/iot/vocab/m3-lite#"/>
    </owl:Class>

    <!-- http://purl.org/iot/vocab/iot-taxonomy-lite#CountEmptyDockingPoints -->

    <owl:Class rdf:about="&iottaxolite;CountEmptyDockingPoints">
        <rdfs:subClassOf rdf:resource="&iottaxolite;Count"/>
        <rdfs:comment xml:lang="en">Number of empty docking points at a particular bicycle docking station.</rdfs:comment>
        <rdfs:label xml:lang="en">Count Empty Docking Points</rdfs:label>
        <rdfs:isDefinedBy rdf:resource="http://purl.org/iot/vocab/m3-lite#"/>
    </owl:Class>

    <!-- http://purl.org/iot/vocab/iot-taxonomy-lite#TrafficIntensity -->

    <owl:Class rdf:about="&iottaxolite;TrafficIntensity">
        <rdfs:subClassOf rdf:resource="&sosa;ObservableProperty"/>
        <rdfs:comment xml:lang="en">The intensity of a traffic flow is the number of vehicles passing a cross section of a road in a unit of time.</rdfs:comment>
        <rdfs:label xml:lang="en">Traffic Intensity</rdfs:label>
        <rdfs:isDefinedBy rdf:resource="http://purl.org/iot/vocab/m3-lite#"/>
    </owl:Class>

    <!-- http://purl.org/iot/vocab/iot-taxonomy-lite#ElectricFieldSensor -->

    <owl:Class rdf:about="&iottaxolite;ElectricFieldSensor">
        <rdfs:subClassOf rdf:resource="&sosa;Sensor"/>
        <rdfs:comment xml:lang="en">Scientific instrument for measuring electromagnetic fields (EMF). Most of them measure the electromagnetic radiation flux density (DC fields) or the change in an electromagnetic field over time (AC fields).</rdfs:comment>
        <rdfs:label xml:lang="en">Electric Field Sensor</rdfs:label>
        <rdfs:isDefinedBy rdf:resource="http://purl.org/iot/vocab/m3-lite#"/>
    </owl:Class>
    
    <!-- http://purl.org/iot/vocab/iot-taxonomy-lite#Counter -->

    <owl:Class rdf:about="&iottaxolite;Counter">
        <rdfs:subClassOf rdf:resource="&sosa;Sensor"/>
        <rdfs:comment xml:lang="en">Sensors that reckons occurrences or repetitions of physical objects, phenomena or events.</rdfs:comment>
        <rdfs:label xml:lang="en">Counter</rdfs:label>
        <rdfs:isDefinedBy rdf:resource="http://purl.org/iot/vocab/m3-lite#"/>
    </owl:Class>

    <!-- http://purl.org/iot/vocab/iot-taxonomy-lite#DoorStateSensor -->

    <owl:Class rdf:about="&iottaxolite;DoorStateSensor">
        <rdfs:subClassOf rdf:resource="&sosa;Sensor"/>
        <rdfs:comment xml:lang="en">This sensor detects if a door is in the state of OPEN or CLOSED.</rdfs:comment>
        <rdfs:label xml:lang="en">Door State Sensor</rdfs:label>
        <rdfs:isDefinedBy rdf:resource="http://purl.org/iot/vocab/m3-lite#"/>
    </owl:Class>

    <!-- http://purl.org/iot/vocab/iot-taxonomy-lite#SoilTemperatureThermometer -->

    <owl:Class rdf:about="&iottaxolite;SoilThermometer">
        <rdfs:subClassOf rdf:resource="&iottaxolite;Thermometer"/>
        <rdfs:comment xml:lang="en">This sensor reports Soil temperature.</rdfs:comment>
        <rdfs:label xml:lang="en">Soil Thermometer</rdfs:label>
        <rdfs:isDefinedBy rdf:resource="http://purl.org/iot/vocab/m3-lite#"/>
    </owl:Class>
    
    <!-- http://purl.org/iot/vocab/iot-taxonomy-lite#SiemensPerMetre -->

    <owl:Class rdf:about="&iottaxolite;SiemensPerMetre">
        <rdfs:subClassOf rdf:resource="&qu;Unit"/>
        <rdfs:comment xml:lang="en">Conductivity is measured in Siemens per metre (S/m).</rdfs:comment>
        <rdfs:label xml:lang="en">Siemens Per Metre, Siemens Per Meter</rdfs:label>
        <rdfs:isDefinedBy rdf:resource="http://purl.org/iot/vocab/m3-lite#"/>
    </owl:Class>

    <!-- http://purl.org/iot/vocab/iot-taxonomy-lite#MilligramPerLitre -->

    <owl:Class rdf:about="&iottaxolite;MilligramPerLitre">
        <rdfs:subClassOf rdf:resource="&iottaxolite;GramPerLitre"/>
        <rdfs:comment xml:lang="en">Level of Dissolved substance in liquid measured in mg per litre.</rdfs:comment>
        <rdfs:label xml:lang="en">Milligram Per Litre, Milligram Per Liter</rdfs:label>
        <rdfs:isDefinedBy rdf:resource="http://purl.org/iot/vocab/m3-lite#"/>
    </owl:Class>

    <!-- http://purl.org/iot/vocab/iot-taxonomy-lite#AirHumiditySensor -->

    <owl:Class rdf:about="&iottaxolite;AirHumiditySensor">
        <rdfs:subClassOf rdf:resource="&iottaxolite;HumiditySensor"/>
        <rdfs:comment xml:lang="en">Sensor used to measure air humidity.</rdfs:comment>
        <rdfs:label xml:lang="en">Air Humidity Sensor</rdfs:label>
        <rdfs:isDefinedBy rdf:resource="http://purl.org/iot/vocab/m3-lite#"/>
    </owl:Class>

    <!-- http://purl.org/iot/vocab/iot-taxonomy-lite#WaterThermometer -->

    <owl:Class rdf:about="&iottaxolite;WaterThermometer">
        <rdfs:subClassOf rdf:resource="&iottaxolite;Thermometer"/>
        <rdfs:comment xml:lang="en">This sensor reports Water temperature.</rdfs:comment>
        <rdfs:label xml:lang="en">Water Thermometer</rdfs:label>
        <rdfs:isDefinedBy rdf:resource="http://purl.org/iot/vocab/m3-lite#"/>
    </owl:Class>

    <!-- http://purl.org/iot/vocab/iot-taxonomy-lite#WaterConductivitySensor -->

    <owl:Class rdf:about="&iottaxolite;WaterConductivitySensor">
        <rdfs:subClassOf rdf:resource="&iottaxolite;ConductivitySensor"/>
        <rdfs:comment xml:lang="en">Device used to measure the conductivity of water.</rdfs:comment>
        <rdfs:label xml:lang="en">Water Conductivity Sensor</rdfs:label>
        <rdfs:isDefinedBy rdf:resource="http://purl.org/iot/vocab/m3-lite#"/>
    </owl:Class>

    <!-- http://purl.org/iot/vocab/iot-taxonomy-lite#WaterPHSensor -->

    <owl:Class rdf:about="&iottaxolite;WaterPHSensor">
        <rdfs:subClassOf rdf:resource="&iottaxolite;PHSensor"/>
        <rdfs:comment xml:lang="en">Device used to detect PH level of water.</rdfs:comment>
        <rdfs:label xml:lang="en">Water PH Sensor</rdfs:label>
        <rdfs:isDefinedBy rdf:resource="http://purl.org/iot/vocab/m3-lite#"/>
    </owl:Class>

        <!-- http://purl.org/iot/vocab/iot-taxonomy-lite#WaterO2IonSensor -->

    <owl:Class rdf:about="&iottaxolite;WaterO2IonSensor">
        <rdfs:subClassOf rdf:resource="&sosa;Sensor"/>
        <rdfs:comment xml:lang="en">Sensor used to measure O2 concentration level in the water.</rdfs:comment>
        <rdfs:label xml:lang="en">Water O2 Ion Sensor</rdfs:label>
        <rdfs:isDefinedBy rdf:resource="http://purl.org/iot/vocab/m3-lite#"/>
    </owl:Class>

    <!-- http://purl.org/iot/vocab/iot-taxonomy-lite#WaterNH4IonSensor -->

    <owl:Class rdf:about="&iottaxolite;WaterNH4IonSensor">
        <rdfs:subClassOf rdf:resource="&sosa;Sensor"/>
        <rdfs:comment xml:lang="en">Sensor used to measure NH4 concentration level in the water.</rdfs:comment>
        <rdfs:label xml:lang="en">Water NH4 Ion Sensor</rdfs:label>
        <rdfs:isDefinedBy rdf:resource="http://purl.org/iot/vocab/m3-lite#"/>
    </owl:Class>

    <!-- http://purl.org/iot/vocab/iot-taxonomy-lite#WaterNO3IonSensor -->

    <owl:Class rdf:about="&iottaxolite;WaterNO3IonSensor">
        <rdfs:subClassOf rdf:resource="&sosa;Sensor"/>
        <rdfs:comment xml:lang="en">Sensor used to measure NO3 concentration level in the water.</rdfs:comment>
        <rdfs:label xml:lang="en">Water NO3 Ion Sensor</rdfs:label>
        <rdfs:isDefinedBy rdf:resource="http://purl.org/iot/vocab/m3-lite#"/>
    </owl:Class>

    <!-- http://purl.org/iot/vocab/iot-taxonomy-lite#LoRaInterfaceEnergyMeter -->

    <owl:Class rdf:about="&iottaxolite;LoRaInterfaceEnergyMeter">
        <rdfs:subClassOf rdf:resource="&iottaxolite;EnergyMeter"/>
        <rdfs:comment xml:lang="en">Measure the average power consumption of the LoRa interface nodes.</rdfs:comment>
        <rdfs:label xml:lang="en">LoRa Interface Energy Meter</rdfs:label>
        <rdfs:isDefinedBy rdf:resource="http://purl.org/iot/vocab/m3-lite#"/>
    </owl:Class>

    <!-- http://purl.org/iot/vocab/iot-taxonomy-lite#WiFiInterfaceEnergyMeter -->

    <owl:Class rdf:about="&iottaxolite;WiFiInterfaceEnergyMeter">
        <rdfs:subClassOf rdf:resource="&iottaxolite;EnergyMeter"/>
        <rdfs:comment xml:lang="en">Measure the average power consumption of the WiFi interface nodes.</rdfs:comment>
        <rdfs:label xml:lang="en">WiFi Interface Energy Meter</rdfs:label>
        <rdfs:isDefinedBy rdf:resource="http://purl.org/iot/vocab/m3-lite#"/>
    </owl:Class>

    <!-- http://purl.org/iot/vocab/iot-taxonomy-lite#Clock -->

    <owl:Class rdf:about="&iottaxolite;Clock">
        <rdfs:subClassOf rdf:resource="&sosa;Sensor"/>
        <rdfs:comment xml:lang="en">sensor that measures time</rdfs:comment>
        <rdfs:label xml:lang="en">Clock</rdfs:label>
        <rdfs:isDefinedBy rdf:resource="http://purl.org/iot/vocab/m3-lite#"/>
    </owl:Class>

    <!-- http://purl.org/iot/vocab/iot-taxonomy-lite#HumanPresenceDetector -->

    <owl:Class rdf:about="&iottaxolite;HumanPresenceDetector">
        <rdfs:subClassOf rdf:resource="&iottaxolite;PresenceDetector"/>
        <rdfs:comment xml:lang="en">Device used to detect if an object (vehicle, room, place, etc.) is occupied by Human.</rdfs:comment>
        <rdfs:label xml:lang="en"> Human Presence Detector</rdfs:label>
        <rdfs:isDefinedBy rdf:resource="http://purl.org/iot/vocab/m3-lite#"/>
    </owl:Class>

    <!-- http://purl.org/iot/vocab/iot-taxonomy-lite#VehiclePresenceDetector -->

    <owl:Class rdf:about="&iottaxolite;VehiclePresenceDetector">
        <rdfs:subClassOf rdf:resource="&iottaxolite;PresenceDetector"/>
        <rdfs:comment xml:lang="en">Device used to detect if an vehicle is present at a place.</rdfs:comment>
        <rdfs:label xml:lang="en"> Vehicle Presence Detector</rdfs:label>
        <rdfs:isDefinedBy rdf:resource="http://purl.org/iot/vocab/m3-lite#"/>
    </owl:Class>

    <!-- http://purl.org/iot/vocab/iot-taxonomy-lite#ChemicalAgentConcentration -->

    <owl:Class rdf:about="&iottaxolite;ChemicalAgentConcentration">
        <rdfs:subClassOf rdf:resource="&sosa;ObservableProperty"/>
        <rdfs:comment xml:lang="en">Measure of Chemical Agent Concentration</rdfs:comment>
        <rdfs:label xml:lang="en">Chemical Agent Concentration Quantity Kind</rdfs:label>
        <rdfs:isDefinedBy rdf:resource="http://purl.org/iot/vocab/m3-lite#"/>
    </owl:Class>

    <!-- http://purl.org/iot/vocab/iot-taxonomy-lite#ChemicalAgentWaterConcentration -->

    <owl:Class rdf:about="&iottaxolite;ChemicalAgentWaterConcentration">
        <rdfs:subClassOf rdf:resource="&iottaxolite;ChemicalAgentConcentration"/>
        <rdfs:comment xml:lang="en">Measure of Chemical Agent Concentration in Water </rdfs:comment>
        <rdfs:label xml:lang="en">Chemical Agent Water Concentration Quantity Kind</rdfs:label>
        <rdfs:isDefinedBy rdf:resource="http://purl.org/iot/vocab/m3-lite#"/>
    </owl:Class>

    <!-- http://purl.org/iot/vocab/iot-taxonomy-lite#ChemicalAgentWaterConcentrationO2 -->

    <owl:Class rdf:about="&iottaxolite;ChemicalAgentWaterConcentrationO2">
        <rdfs:subClassOf rdf:resource="&iottaxolite;ChemicalAgentWaterConcentration"/>
        <rdfs:comment xml:lang="en">Measure of O2 concentration in Water </rdfs:comment>
        <rdfs:label xml:lang="en">Oxygen (O2) Chemical Agent Water Concentration</rdfs:label>
        <rdfs:isDefinedBy rdf:resource="http://purl.org/iot/vocab/m3-lite#"/>
    </owl:Class>

    <!-- http://purl.org/iot/vocab/iot-taxonomy-lite#ChemicalAgentWaterConcentrationNH4Ion -->

    <owl:Class rdf:about="&iottaxolite;ChemicalAgentWaterConcentrationNH4Ion">
        <rdfs:subClassOf rdf:resource="&iottaxolite;ChemicalAgentWaterConcentration"/>
        <rdfs:comment xml:lang="en">Measure of NH4 ion concentration in Water </rdfs:comment>
        <rdfs:label xml:lang="en">Ammonium ion (NH4+) Chemical Agent Water Concentration</rdfs:label>
        <rdfs:isDefinedBy rdf:resource="http://purl.org/iot/vocab/m3-lite#"/>
    </owl:Class>

    <!-- http://purl.org/iot/vocab/iot-taxonomy-lite#ChemicalAgentWaterConcentrationNO3Ion -->

    <owl:Class rdf:about="&iottaxolite;ChemicalAgentWaterConcentrationNO3Ion">
        <rdfs:subClassOf rdf:resource="&iottaxolite;ChemicalAgentWaterConcentration"/>
        <rdfs:comment xml:lang="en">Measure of NO3 ion concentration in Water </rdfs:comment>
        <rdfs:label xml:lang="en">Nitrate Ion (NO3-) Chemical Agent Water Concentration</rdfs:label>
        <rdfs:isDefinedBy rdf:resource="http://purl.org/iot/vocab/m3-lite#"/>
    </owl:Class>

        <!-- http://purl.org/iot/vocab/iot-taxonomy-lite#RadiationParticleDetector -->

    <owl:Class rdf:about="&iottaxolite;RadiationParticleDetector">
        <rdfs:subClassOf rdf:resource="&sosa;Sensor"/>
        <rdfs:comment xml:lang="en">A particle detector, also known as a radiation detector or Geiger counter, is a device used to detect, track, and/or identify ionising particles, such as those produced by nuclear decay, cosmic radiation, or reactions in a particle accelerator.</rdfs:comment>
        <rdfs:label xml:lang="en">Radiation Particle Detector</rdfs:label>
        <rdfs:isDefinedBy rdf:resource="http://purl.org/iot/vocab/m3-lite#"/>
    </owl:Class>

    <!-- http://purl.org/iot/vocab/iot-taxonomy-lite#IonisingRadiation -->

    <owl:Class rdf:about="&iottaxolite;IonisingRadiation">
        <rdfs:subClassOf rdf:resource="&sosa;ObservableProperty"/>
        <rdfs:comment xml:lang="en">Ionising radiation is radiation that carries enough energy to free electrons from atoms or molecules, thereby ionizing them. Gamma rays, X-rays, and the higher ultraviolet part of the electromagnetic spectrum are ionizing, whereas the lower ultraviolet part of the electromagnetic spectrum, and also the lower part of the spectrum below UV, including visible light (including nearly all types of laser light), infrared, microwaves, and radio waves are all considered non-ionizing radiation.</rdfs:comment>
        <rdfs:label xml:lang="en">Ionising Radiation</rdfs:label>
        <rdfs:isDefinedBy rdf:resource="http://purl.org/iot/vocab/m3-lite#"/>
    </owl:Class>


    <!-- http://purl.org/iot/vocab/iot-taxonomy-lite#RadiationParticlesPerMinute -->

    <owl:Class rdf:about="&iottaxolite;RadiationParticlesPerMinute">
        <rdfs:subClassOf rdf:resource="&qu;Unit"/>
        <rdfs:comment xml:lang="en">The number of ionizing events detected in one minute.</rdfs:comment>
        <rdfs:label xml:lang="en">Radiation Particles Per Minute</rdfs:label>
        <rdfs:isDefinedBy rdf:resource="http://purl.org/iot/vocab/m3-lite#"/>
    </owl:Class>

    <!-- http://purl.org/iot/vocab/iot-taxonomy-lite#ChemicalAgentAtmosphericConcentrationDust -->

    <owl:Class rdf:about="&iottaxolite;ChemicalAgentAtmosphericConcentrationDust">
        <rdfs:subClassOf rdf:resource="&iottaxolite;ChemicalAgentAtmosphericConcentration"/>
        <rdfs:comment xml:lang="en">Measure of the concentration of dust suspended in the air.</rdfs:comment>
        <rdfs:label xml:lang="en">Chemical Agent Atmospheric Concentration Dust</rdfs:label>
        <rdfs:isDefinedBy rdf:resource="http://purl.org/iot/vocab/m3-lite#"/>
    </owl:Class>

    <!-- http://purl.org/iot/vocab/iot-taxonomy-lite#DustSensor -->

    <owl:Class rdf:about="&iottaxolite;DustSensor">
        <rdfs:subClassOf rdf:resource="&sosa;Sensor"/>
        <rdfs:comment xml:lang="en">A sensing device that measures dust particle concentration.</rdfs:comment>
        <rdfs:label xml:lang="en">Dust Sensor</rdfs:label>
        <rdfs:isDefinedBy rdf:resource="http://purl.org/iot/vocab/m3-lite#"/>
    </owl:Class>

    <!-- http://purl.org/iot/vocab/iot-taxonomy-lite#OpticalDustSensor -->

    <owl:Class rdf:about="&iottaxolite;OpticalDustSensor">
        <rdfs:subClassOf rdf:resource="&iottaxolite;DustSensor"/>
        <rdfs:comment xml:lang="en">A sensing device that measures dust particle concentration using optical sensing mean.</rdfs:comment>
        <rdfs:label xml:lang="en">Optical Dust Sensor</rdfs:label>
        <rdfs:isDefinedBy rdf:resource="http://purl.org/iot/vocab/m3-lite#"/>
    </owl:Class>

    <!-- http://purl.org/iot/vocab/iot-taxonomy-lite#Voltage -->

    <owl:Class rdf:about="&iottaxolite;Voltage">
        <rdfs:subClassOf rdf:resource="&sosa;ObservableProperty"/>
        <rdfs:comment xml:lang="en">An electromotive force or potential difference expressed in volts (Source Google).</rdfs:comment>
        <rdfs:label xml:lang="en">Voltage</rdfs:label>
        <rdfs:isDefinedBy rdf:resource="http://purl.org/iot/vocab/m3-lite#"/>
    </owl:Class>


    <!-- V3 updates-->



	<!-- http://purl.org/iot/vocab/iot-taxonomy-lite#VOCSensor -->

    <owl:Class rdf:about="&iottaxolite;VOCSensor">
        <rdfs:subClassOf rdf:resource="&iottaxolite;GaseousPollutantSensor"/>
        <rdfs:comment xml:lang="en">Sensor that detects levels of Volatile Organic Components (VOC) in the environment.</rdfs:comment>
        <rdfs:label xml:lang="en">Volatile Organic Compound (VOC) Sensor</rdfs:label>
        <rdfs:isDefinedBy rdf:resource="http://purl.org/iot/vocab/m3-lite#"/>
    </owl:Class>

	<!-- http://purl.org/iot/vocab/iot-taxonomy-lite#IEEE802154InterfaceEnergyMeter -->

    <owl:Class rdf:about="&iottaxolite;IEEE802154InterfaceEnergyMeter">
        <rdfs:subClassOf rdf:resource="&iottaxolite;EnergyMeter"/>
        <rdfs:comment xml:lang="en">Sensor that measures the power consumption of the IEEE802.15.4 interface nodes.</rdfs:comment>
        <rdfs:label xml:lang="en">IEEE802.15.4 Interface Energy Meter</rdfs:label>
        <rdfs:isDefinedBy rdf:resource="http://purl.org/iot/vocab/m3-lite#"/>
    </owl:Class>

	<!-- http://purl.org/iot/vocab/iot-taxonomy-lite#BoardVoltageSensor -->

    <owl:Class rdf:about="&iottaxolite;BoardVoltageSensor">
        <rdfs:subClassOf rdf:resource="&iottaxolite;VoltageSensor"/>
        <rdfs:comment xml:lang="en">Sensor used to measure board input voltage.</rdfs:comment>
        <rdfs:label xml:lang="en">Board Voltage Sensor</rdfs:label>
        <rdfs:isDefinedBy rdf:resource="http://purl.org/iot/vocab/m3-lite#"/>
    </owl:Class>

    <!-- http://purl.org/iot/vocab/iot-taxonomy-lite#DeviceUptimeClock -->

    <owl:Class rdf:about="&iottaxolite;DeviceUptimeClock">
        <rdfs:subClassOf rdf:resource="&iottaxolite;Clock"/>
        <rdfs:comment xml:lang="en">Sensor that measures time a device is working and is available.</rdfs:comment>
        <rdfs:label xml:lang="en">Device Uptime Clock</rdfs:label>
        <rdfs:isDefinedBy rdf:resource="http://purl.org/iot/vocab/m3-lite#"/>
    </owl:Class>

    <!-- http://purl.org/iot/vocab/iot-taxonomy-lite#VoiceCommandSensor -->

    <owl:Class rdf:about="&iottaxolite;VoiceCommandSensor">
        <rdfs:subClassOf rdf:resource="&sosa;Sensor"/>
        <rdfs:comment xml:lang="en">Sensor that uses automatic speech recognition technology to match or reject a recorded voice command according to a specified set of available voice commands.</rdfs:comment>
        <rdfs:label xml:lang="en">Voice Command Sensor</rdfs:label>
        <rdfs:isDefinedBy rdf:resource="http://purl.org/iot/vocab/m3-lite#"/>
    </owl:Class>

    <!-- http://purl.org/iot/vocab/iot-taxonomy-lite#DirectionOfArrivalSensor -->

    <owl:Class rdf:about="&iottaxolite;DirectionOfArrivalSensor">
        <rdfs:subClassOf rdf:resource="&sosa;Sensor"/>
        <rdfs:comment xml:lang="en">Sensor that estimates the azimuth direction of sources relative to the sensor’s position.</rdfs:comment>
        <rdfs:label xml:lang="en">Direction Of Arrival (DOA) Sensor</rdfs:label>
        <rdfs:isDefinedBy rdf:resource="http://purl.org/iot/vocab/m3-lite#"/>
    </owl:Class>


    <!-- http://purl.org/iot/vocab/iot-taxonomy-lite#ChemicalAgentAtmosphericConcentrationNO -->

    <owl:Class rdf:about="&iottaxolite;ChemicalAgentAtmosphericConcentrationNO">
        <rdfs:subClassOf rdf:resource="&iottaxolite;ChemicalAgentAtmosphericConcentration"/>
        <rdfs:comment xml:lang="en">Measure of the concentration of Carbon Monoxide (CO) gas suspended in the atmosphere.</rdfs:comment>
        <rdfs:label xml:lang="en">Nitrogen Monoxide (NO) Chemical Agent Atmospheric Concentration</rdfs:label>
        <rdfs:isDefinedBy rdf:resource="http://purl.org/iot/vocab/m3-lite#"/>
    </owl:Class>

    <!-- http://purl.org/iot/vocab/iot-taxonomy-lite#ChemicalAgentAtmosphericConcentrationSO2 -->

    <owl:Class rdf:about="&iottaxolite;ChemicalAgentAtmosphericConcentrationSO2">
        <rdfs:subClassOf rdf:resource="&iottaxolite;ChemicalAgentAtmosphericConcentration"/>
        <rdfs:comment xml:lang="en">Measure of the concentration of Sulphur dioxide (SO2) gas suspended in the atmosphere.</rdfs:comment>
        <rdfs:label xml:lang="en">Sulphur dioxide (SO2) Chemical Agent Atmospheric Concentration</rdfs:label>
        <rdfs:isDefinedBy rdf:resource="http://purl.org/iot/vocab/m3-lite#"/>
    </owl:Class>

    <!-- http://purl.org/iot/vocab/iot-taxonomy-lite#ChemicalAgentAtmosphericConcentrationVOC -->

    <owl:Class rdf:about="&iottaxolite;ChemicalAgentAtmosphericConcentrationVOC">
        <rdfs:subClassOf rdf:resource="&iottaxolite;ChemicalAgentAtmosphericConcentration"/>
        <rdfs:comment xml:lang="en">Measure of the concentration of Volatile Organic Compound gas suspended in the atmosphere.</rdfs:comment>
        <rdfs:label xml:lang="en">Volatile Organic Compound Chemical Agent Atmospheric Concentration</rdfs:label>
        <rdfs:isDefinedBy rdf:resource="http://purl.org/iot/vocab/m3-lite#"/>
    </owl:Class>

    <!-- http://purl.org/iot/vocab/iot-taxonomy-lite#ChemicalAgentAtmosphericConcentrationNH3 -->
     
     <owl:Class rdf:about="&iottaxolite;ChemicalAgentAtmosphericConcentrationNH3">
         <rdfs:subClassOf rdf:resource="&iottaxolite;ChemicalAgentAtmosphericConcentration"/>
        <rdfs:comment xml:lang="en">Measure of the concentration of Ammonia (NH3) gas suspended in the atmosphere.</rdfs:comment>
        <rdfs:label xml:lang="en">Ammonia (NH3) Chemical Agent Atmospheric Concentration</rdfs:label>
        <rdfs:isDefinedBy rdf:resource="http://purl.org/iot/vocab/m3-lite#"/>
    </owl:Class>

	<!-- http://purl.org/iot/vocab/iot-taxonomy-lite#DeviceUptime -->

    <owl:Class rdf:about="&iottaxolite;DeviceUptime">
        <rdfs:subClassOf rdf:resource="&sosa;ObservableProperty"/>
        <rdfs:comment xml:lang="en">Time a device is working and is available</rdfs:comment>
        <rdfs:label xml:lang="en">Device Uptime</rdfs:label>
        <rdfs:isDefinedBy rdf:resource="http://purl.org/iot/vocab/m3-lite#"/>
    </owl:Class>
    
    <!-- http://purl.org/iot/vocab/iot-taxonomy-lite#VoiceCommand -->

    <owl:Class rdf:about="&iottaxolite;VoiceCommand">
        <rdfs:subClassOf rdf:resource="&sosa;ObservableProperty"/>
        <rdfs:comment xml:lang="en">A voice command to control a voice controlled system or environment, such as a smart home.</rdfs:comment>
        <rdfs:label xml:lang="en">Voice Command</rdfs:label>
        <rdfs:isDefinedBy rdf:resource="http://purl.org/iot/vocab/m3-lite#"/>
    </owl:Class>

    <!-- http://purl.org/iot/vocab/iot-taxonomy-lite#DirectionOfArrival -->

    <owl:Class rdf:about="&iottaxolite;DirectionOfArrival">
        <rdfs:subClassOf rdf:resource="&sosa;ObservableProperty"/>
        <rdfs:comment xml:lang="en">The azimuth direction of a  source relative to the azimuth direction of the DOA sensor.</rdfs:comment>
        <rdfs:label xml:lang="en">Direction Of Arrival</rdfs:label>
        <rdfs:isDefinedBy rdf:resource="http://purl.org/iot/vocab/m3-lite#"/>
    </owl:Class>

    <!-- http://purl.org/iot/vocab/iot-taxonomy-lite#PartsPerBillion -->

    <owl:Class rdf:about="&iottaxolite;PartsPerBillion">
        <rdfs:subClassOf rdf:resource="&iottaxolite;PPM"/>
        <rdfs:comment xml:lang="en">It describes the concentration of something in parts per billion parts of water or soil, expressed in any (but common) unit of measurement.</rdfs:comment>
        <rdfs:label xml:lang="en">Parts Per Billion</rdfs:label>
        <rdfs:isDefinedBy rdf:resource="http://purl.org/iot/vocab/m3-lite#"/>
    </owl:Class>
	
	<!-- http://purl.org/iot/vocab/iot-taxonomy-lite#DecibelMilliwatt -->

    <owl:Class rdf:about="&iottaxolite;DecibelMilliwatt">
        <rdfs:subClassOf rdf:resource="&iottaxolite;Decibel"/>
        <rdfs:comment xml:lang="en">It describes power ratio in decibels of the measured power referenced to one milliwatt.</rdfs:comment>
        <rdfs:label xml:lang="en">Decibel Milliwatt</rdfs:label>
        <rdfs:isDefinedBy rdf:resource="http://purl.org/iot/vocab/m3-lite#"/>
    </owl:Class>

    <!-- http://purl.org/iot/vocab/iot-taxonomy-lite#VoiceCommandController -->

    <owl:Class rdf:about="&iottaxolite;VoiceCommandController">
        <rdfs:subClassOf rdf:resource="&sosa;Actuator"/>
        <rdfs:comment xml:lang="en">An actuating device called  that allows to semi-control the environment of the Voice Command Sensor.</rdfs:comment>
        <rdfs:label xml:lang="en">Voice Command Controller</rdfs:label>
        <rdfs:isDefinedBy rdf:resource="http://purl.org/iot/vocab/m3-lite#"/>
    </owl:Class>

    <!-- http://purl.org/iot/vocab/iot-taxonomy-lite#OxidationReductionPotentialSensor -->

    <owl:Class rdf:about="&iottaxolite;OxidationReductionPotentialSensor">
        <rdfs:subClassOf rdf:resource="&sosa;Sensor"/>
        <rdfs:comment xml:lang="en">Measures the Water Oxidation Reduction Potential (ORP) as the tendency of a chemical species to acquire electrons and thereby be reduced.</rdfs:comment>
        <rdfs:label xml:lang="en">Oxidation Reduction Potential (ORP) Sensor</rdfs:label>
        <rdfs:isDefinedBy rdf:resource="http://purl.org/iot/vocab/m3-lite#"/>
    </owl:Class>



	<!--  http://purl.org/iot/vocab/iot-taxonomy-lite#CountPeople -->

	<owl:Class rdf:about="&iottaxolite;CountPeople">
		<rdfs:subClassOf rdf:resource="&iottaxolite;Count"/>
		<rdfs:comment xml:lang="en">Number of people within a particular area</rdfs:comment>
		<rdfs:label xml:lang="en">Count People</rdfs:label>
	</owl:Class>

	<!--  http://purl.org/iot/vocab/iot-taxonomy-lite#PeopleCountSensor -->
	
	<owl:Class rdf:about="&iottaxolite;PeopleCountSensor">
		<rdfs:subClassOf rdf:resource="&iottaxolite;Counter"/>
		<rdfs:comment xml:lang="en">Device used to count the number of people (eg., used within an indoor area).</rdfs:comment>
		<rdfs:label xml:lang="en">People Count Sensor</rdfs:label>
	</owl:Class>

	<!-- http://purl.org/iot/vocab/iot-taxonomy-lite#TimeOfArrival -->
	
	<owl:Class rdf:about="&iottaxolite;TimeOfArrival">
		<rdfs:subClassOf rdf:resource="&sosa;ObservableProperty"/>
		<rdfs:comment xml:lang="en">Estimated time till an object is arriving to a specific location (typically used in transportation).</rdfs:comment>
		<rdfs:label xml:lang="en">Time of arrival</rdfs:label>
	</owl:Class>

	<!-- http://purl.org/iot/vocab/iot-taxonomy-lite#TimeOfArrivalSensor -->
	
	<owl:Class rdf:about="&iottaxolite;TimeOfArrivalSensor">
		<rdfs:subClassOf rdf:resource="&sosa;Sensor"/>
		<rdfs:comment xml:lang="en">Virtual device that estimates the remaining time for an object to arrive at a specific location.</rdfs:comment>
		<rdfs:label xml:lang="en">Time of Arrival Sensor</rdfs:label>
	</owl:Class>


	<!-- http://purl.org/iot/vocab/iot-taxonomy-lite#Bus   -->
	
	<owl:Class rdf:about="&iottaxolite;Bus">
		<rdfs:subClassOf rdf:resource="&sosa;Platform"/>
		<rdfs:comment xml:lang="en">A large motor vehicle carrying passengers by road, typically one serving the public on a fixed route and for a fare.</rdfs:comment>
		<rdfs:label xml:lang="en">Bus</rdfs:label>
	</owl:Class>


    <!-- http://purl.org/iot/vocab/iot-taxonomy-lite#LoRaInterface -->
    
    <owl:Class rdf:about="&iottaxolite;LoRaInterface">
        <rdfs:subClassOf rdf:resource="&sosa;Sensor"/>
        <rdfs:comment xml:lang="en">This device is used for long range low power wireless communications. We can use this device to report network metrics (SNR, latence, etc.)</rdfs:comment>
        <rdfs:label xml:lang="en">LoRa Interface</rdfs:label>
        <rdfs:isDefinedBy rdf:resource="http://purl.org/iot/vocab/m3-lite#"/>
    </owl:Class>

    <!-- http://purl.org/iot/vocab/iot-taxonomy-lite#SNR -->
    
    <owl:Class rdf:about="&iottaxolite;SNR">
        <rdfs:subClassOf rdf:resource="&sosa;ObservableProperty"/>
        <rdfs:comment xml:lang="en">Compares the level of a desired signal to the level of noise. </rdfs:comment>
        <rdfs:label xml:lang="en">Signal to Noise Ratio</rdfs:label>
        <rdfs:isDefinedBy rdf:resource="http://purl.org/iot/vocab/m3-lite#"/>
    </owl:Class>

    <!-- http://purl.org/iot/vocab/iot-taxonomy-lite#RSSI -->
    
    <owl:Class rdf:about="&iottaxolite;RSSI">
        <rdfs:subClassOf rdf:resource="&sosa;ObservableProperty"/>
        <rdfs:comment xml:lang="en">Received Signal Strength Indicator is the signal strength in a wireless network environment.</rdfs:comment>
        <rdfs:label xml:lang="en">Received Signal Strength Indicator</rdfs:label>
        <rdfs:isDefinedBy rdf:resource="http://purl.org/iot/vocab/m3-lite#"/>
    </owl:Class>

    <!-- http://purl.org/iot/vocab/iot-taxonomy-lite#HDOP -->
    
    <owl:Class rdf:about="&iottaxolite;HDOP">
        <rdfs:subClassOf rdf:resource="&sosa;ObservableProperty"/>
        <rdfs:comment xml:lang="en">Describes the preceision of the GPS signal. Smaller the value is, more precise the signal is.</rdfs:comment>
        <rdfs:label xml:lang="en">Horizontal Dilution of Precision</rdfs:label>
        <rdfs:isDefinedBy rdf:resource="http://purl.org/iot/vocab/m3-lite#"/>
    </owl:Class>

    <!--  http://purl.org/iot/vocab/iot-taxonomy-lite#CountStatellitesSignalReceived -->
    
    <owl:Class rdf:about="&iottaxolite;CountStatellitesSignalReceived">
        <rdfs:subClassOf rdf:resource="&iottaxolite;Count"/>
        <rdfs:comment xml:lang="en">Count of satellites from which a signal is received</rdfs:comment>
        <rdfs:label xml:lang="en">Count Statellites Signal Received</rdfs:label>
        <rdfs:isDefinedBy rdf:resource="http://purl.org/iot/vocab/m3-lite#"/>
    </owl:Class>

    <!--  http://purl.org/iot/vocab/iot-taxonomy-lite#CurrentSensor -->
     
    <owl:Class rdf:about="&iottaxolite;CurrentSensor">
        <rdfs:subClassOf rdf:resource="&sosa;Sensor"/>
        <rdfs:comment xml:lang="en">A current sensor is a device that detects electric current in a wire, and generates a signal proportional to that current.</rdfs:comment>
        <rdfs:label xml:lang="en">Current Sensor</rdfs:label>
        <rdfs:isDefinedBy rdf:resource="http://purl.org/iot/vocab/m3-lite#"/>
    </owl:Class>

    <!-- http://purl.org/iot/vocab/iot-taxonomy-lite#TimeOfArrivalNextBus -->
    <owl:Class rdf:about="&iottaxolite;TimeOfArrivalNextBus">
        <rdfs:subClassOf rdf:resource="&iottaxolite;TimeOfArrival"/>
        <rdfs:comment xml:lang="en">Estimated time (in seconds) till a bus will arrive at a specific bus stop. </rdfs:comment>
        <rdfs:label xml:lang="en">Time of arrival for the next bus</rdfs:label>
        <rdfs:isDefinedBy rdf:resource="http://purl.org/iot/vocab/m3-lite#"/>
    </owl:Class>

    <!--http://purl.org/iot/vocab/iot-taxonomy-lite#TimeOfArrivalNextBusSensor -->
    <owl:Class rdf:about="&iottaxolite;TimeOfArrivalNextBusSensor">
        <rdfs:subClassOf rdf:resource="&iottaxolite;TimeOfArrivalSensor"/>
        <rdfs:comment xml:lang="en">Virtual device that represents a bus stop X and a bus line Y; it estimates the remaining time the next bus (belonging to line Y) will arrive at bus stop X. </rdfs:comment>
        <rdfs:label xml:lang="en">Time of arrival sensor for the next bus</rdfs:label>
        <rdfs:isDefinedBy rdf:resource="http://purl.org/iot/vocab/m3-lite#"/>
    </owl:Class>

    <!-- http://purl.org/iot/vocab/iot-taxonomy-lite#DistanceNextBus -->
    <owl:Class rdf:about="&iottaxolite;DistanceNextBus">
        <rdfs:subClassOf rdf:resource="&iottaxolite;Distance"/>
        <rdfs:comment xml:lang="en">Estimated driving distance (in meters) between a bus and the next bus stop. </rdfs:comment>
        <rdfs:label xml:lang="en">Driving distance between a bus and the next bus stop</rdfs:label>
        <rdfs:isDefinedBy rdf:resource="http://purl.org/iot/vocab/m3-lite#"/>
    </owl:Class>

    <!-- http://purl.org/iot/vocab/iot-taxonomy-lite#DistanceNextBusSensor -->
    <owl:Class rdf:about="&iottaxolite;DistanceNextBusSensor">
        <rdfs:subClassOf rdf:resource="&iottaxolite;DistanceSensor"/>
        <rdfs:comment xml:lang="en"> Virtual device that represents a bus stop X and a bus line Y; it measures the driving distance between the next bus (belonging to line Y) and the bus stop X. </rdfs:comment>
        <rdfs:label xml:lang="en">Sensor measuring the driving distance between a bus and the next bus stop</rdfs:label>
        <rdfs:isDefinedBy rdf:resource="http://purl.org/iot/vocab/m3-lite#"/>
    </owl:Class>

    <!-- http://purl.org/iot/vocab/iot-taxonomy-lite#StayingPeopleCountSensor -->
    <owl:Class rdf:about="&iottaxolite;StayingPeopleCountSensor">
        <rdfs:subClassOf rdf:resource="&iottaxolite;PeopleCountSensor"/>
        <rdfs:comment xml:lang="en">Device used to count the number of people that stays within an area for more than a threshold of time.</rdfs:comment>
        <rdfs:label xml:lang="en">Staying People Count Sensor</rdfs:label>
        <rdfs:isDefinedBy rdf:resource="http://purl.org/iot/vocab/m3-lite#"/>
    </owl:Class>

    <!-- http://purl.org/iot/vocab/iot-taxonomy-lite#CountPeopleStaying -->
    
    <owl:Class rdf:about="&iottaxolite;CountPeopleStaying">
        <rdfs:subClassOf rdf:resource="&iottaxolite;CountPeople"/>
        <rdfs:comment xml:lang="en">Number of people that stayed within an area for more than a threshold of time.</rdfs:comment>
        <rdfs:label xml:lang="en">Count People Staying</rdfs:label>
        <rdfs:isDefinedBy rdf:resource="http://purl.org/iot/vocab/m3-lite#"/>
    </owl:Class>

    <!-- http://purl.org/iot/vocab/iot-taxonomy-lite#PeopleStayDurationSensor  -->
    
    <owl:Class rdf:about="&iottaxolite;PeopleStayDurationSensor">
         <rdfs:subClassOf rdf:resource="&sosa;Sensor"/>
        <rdfs:comment xml:lang="en">Device used to measure the time people stays within an area.</rdfs:comment>
        <rdfs:label xml:lang="en">People Stay Duration Sensor</rdfs:label>
        <rdfs:isDefinedBy rdf:resource="http://purl.org/iot/vocab/m3-lite#"/>
    </owl:Class>
    
    <!-- http://purl.org/iot/vocab/iot-taxonomy-lite#PeopleStayDurationAverage  -->
    
    <owl:Class rdf:about="&iottaxolite;PeopleStayDurationAverage">
        <rdfs:subClassOf rdf:resource="&sosa;ObservableProperty"/>
        <rdfs:comment xml:lang="en">Average time people stays within an area.</rdfs:comment>
        <rdfs:label xml:lang="en">People Stay Duration Average </rdfs:label>
        <rdfs:isDefinedBy rdf:resource="http://purl.org/iot/vocab/m3-lite#"/>
    </owl:Class>

    <!-- http://purl.org/iot/vocab/iot-taxonomy-lite#PeopleFlowCountSensor -->
    
    <owl:Class rdf:about="&iottaxolite;PeopleFlowCountSensor">
        <rdfs:subClassOf rdf:resource="&iottaxolite;PeopleCountSensor"/>
        <rdfs:comment xml:lang="en">Device used to count the number of people the moves from an area towards another area during a time window.</rdfs:comment>
        <rdfs:label xml:lang="en">People Flow Count Sensor</rdfs:label>
        <rdfs:isDefinedBy rdf:resource="http://purl.org/iot/vocab/m3-lite#"/>
    </owl:Class>

     <!-- http://purl.org/iot/vocab/iot-taxonomy-lite#CountPeopleMoving -->
    
    <owl:Class rdf:about="&iottaxolite;CountPeopleMoving">
        <rdfs:subClassOf rdf:resource="&iottaxolite;CountPeople"/>
        <rdfs:comment xml:lang="en">Number of people that moved outside an area towards another area during a time window.</rdfs:comment>
        <rdfs:label xml:lang="en">Count People Moving</rdfs:label>
        <rdfs:isDefinedBy rdf:resource="http://purl.org/iot/vocab/m3-lite#"/>
    </owl:Class>


    <!-- http://purl.org/iot/vocab/iot-taxonomy-lite#QualityOfObservation -->
    
    <owl:Class rdf:about="&iottaxolite;QualityOfObservation">
        <rdfs:comment xml:lang="en">It identifies the quality of observation taken by a sensor or an actuator</rdfs:comment>
        <rdfs:label xml:lang="en">Quality Of Observation</rdfs:label>
    </owl:Class>


    <!-- http://purl.org/iot/vocab/iot-taxonomy-lite#Fair -->
    
    <owl:Class rdf:about="&iottaxolite;Fair">
        <rdfs:subClassOf rdf:resource="&iottaxolite;QualityOfObservation"/>
        <rdfs:comment xml:lang="en">When the quality of observation is fair</rdfs:comment>
        <rdfs:label xml:lang="en">Fair</rdfs:label>
    </owl:Class>

    <!-- http://purl.org/iot/vocab/iot-taxonomy-lite#Good -->
    
    <owl:Class rdf:about="&iottaxolite;Good">
        <rdfs:subClassOf rdf:resource="&iottaxolite;QualityOfObservation"/>
        <rdfs:comment xml:lang="en">When the quality of observation is good</rdfs:comment>
        <rdfs:label xml:lang="en">Good</rdfs:label>
    </owl:Class>

    <!-- http://purl.org/iot/vocab/iot-taxonomy-lite#Bad -->
    
    <owl:Class rdf:about="&iottaxolite;Bad">
        <rdfs:subClassOf rdf:resource="&iottaxolite;QualityOfObservation"/>
        <rdfs:comment xml:lang="en">When the quality of observation is bad</rdfs:comment>
        <rdfs:label xml:lang="en">Bad</rdfs:label>
    </owl:Class>


    <!-- http://purl.org/iot/vocab/iot-taxonomy-lite#Room -->
    
    <owl:Class rdf:about="&iottaxolite;Room">
        <rdfs:subClassOf rdf:resource="&sosa;FeatureOfInterest"/>
        <rdfs:comment xml:lang="en">When the feature of interest is room</rdfs:comment>
        <rdfs:label xml:lang="en">Room</rdfs:label>
    </owl:Class>



    <!-- http://purl.org/adaptcentre/openscience/ontologies/consent#Action -->


    <owl:Class rdf:about="http://purl.org/adaptcentre/openscience/ontologies/consent#Action">
        <rdfs:comment>&apos;action&apos; is used to identify what action is permitted by the consent.</rdfs:comment>
        <rdfs:label>Action</rdfs:label>
        <rdfs:comment>&apos;action&apos; defines what action is permitted by the consent.</rdfs:comment>
    </owl:Class>


    <!-- http://purl.org/adaptcentre/openscience/ontologies/consent#Purpose -->


    <owl:Class rdf:about="http://purl.org/adaptcentre/openscience/ontologies/consent#Purpose">
        <rdfs:label>Purpose</rdfs:label>
        <rdfs:comment>&apos;purpose&apos; indicates for what purpose the action is allowed by the consent on the data</rdfs:comment>
    </owl:Class>

    <!-- http://purl.org/iot/vocab/iot-taxonomy-lite#DiscoverSensors -->
    
    <owl:Class rdf:about="&iottaxolite;DiscoverSensors">
        <rdfs:subClassOf rdf:resource="&consent;Action"/>
        <rdfs:comment xml:lang="en">Discover sensors in a given context</rdfs:comment>
        <rdfs:label xml:lang="en">Discover Sensors</rdfs:label>
    </owl:Class>


    <!-- http://purl.org/iot/vocab/iot-taxonomy-lite#KnowSensorsInTheArea -->
    
    <owl:Class rdf:about="&iottaxolite;KnowSensorsInTheArea">
        <rdfs:subClassOf rdf:resource="&consent;Purpose"/>
        <rdfs:comment xml:lang="en">Purpose to know sensors in the given area</rdfs:comment>
        <rdfs:label xml:lang="en">Know Sensors In The Area</rdfs:label>
    </owl:Class>


    <!-- http://purl.org/iot/vocab/iot-taxonomy-lite#BloodCoagulation -->

    <owl:Class rdf:about="&iottaxolite;BloodCoagulation">
        <rdfs:subClassOf rdf:resource="&sosa;ObservableProperty"/>
        <dc:description xml:lang="en">Blood Coagulation is the process by which blood changes from  liquid to gel to form a blood clot. It allows the cessation of blood loss from an injury.</dc:description>
        <rdfs:label xml:lang="en">Blood Coagulation</rdfs:label>
        <rdfs:isDefinedBy rdf:resource="http://purl.org/iot/vocab/m3-lite#"/>
    </owl:Class>
    

    <!-- http://purl.org/iot/vocab/iot-taxonomy-lite#Coagulometer -->

    <owl:Class rdf:about="&iottaxolite;Coagulometer">
        <rdfs:subClassOf rdf:resource="&sosa;Sensor"/>
        <dc:description>Coagulometer is a medical device used for measuring the coagulation of a patient&apos;s blood and testing of the hemostasis system.</dc:description>
        <rdfs:label>Coagulometer</rdfs:label>
        <rdfs:isDefinedBy rdf:resource="http://purl.org/iot/vocab/m3-lite#"/>
    </owl:Class>


    <!-- http://purl.org/iot/vocab/iot-taxonomy-lite#FloorSensor -->

    <owl:Class rdf:about="&iottaxolite;FloorSensor">
        <rdfs:subClassOf rdf:resource="&sosa;Sensor"/>
        <dc:description>A floor sensor is a set of sensors covering a floor that can be used for measuring load and proximity. By using this information the floor sensor can be also used for detecting activity in a room</dc:description>
        <rdfs:label xml:lang="en">FloorSensor</rdfs:label>
        <rdfs:isDefinedBy rdf:resource="http://purl.org/iot/vocab/m3-lite#"/>
    </owl:Class>


    <!-- http://purl.org/iot/vocab/iot-taxonomy-lite#HDOP -->

    <owl:Class rdf:about="&iottaxolite;HDOP">
        <rdfs:subClassOf rdf:resource="&sosa;ObservableProperty"/>
        <rdfs:comment xml:lang="en">Describes the preceision of the GPS signal. Smaller the value is, more precise the signal is.</rdfs:comment>
        <rdfs:label xml:lang="en">Horizontal Dilution of Precision</rdfs:label>
        <rdfs:isDefinedBy rdf:resource="http://purl.org/iot/vocab/m3-lite#"/>
    </owl:Class>
    
    <!-- http://purl.org/iot/vocab/iot-taxonomy-lite#INR -->

    <owl:Class rdf:about="&iottaxolite;INR">
        <rdfs:subClassOf rdf:resource="&qu;Unit"/>
        <dc:description xml:lang="en">A system established by the World Health Organization (WHO) and the International Committee on Thrombosis and Hemostasis for reporting the results of blood coagulation (clotting) tests. Abbreviated INR. Under the INR system, all results are standardized. For example, a person taking the anticoagulant warfarin (brand name: Coumadin) would regularly have blood tested to measure the INR. The INR permits patients on anticoagulants to travel and obtain comparable test results wherever they are.
        Medical Definition of International normalized ratio, MedicineNet</dc:description>
        <rdfs:label xml:lang="en">International Normalized Ratio</rdfs:label>
        <rdfs:isDefinedBy rdf:resource="http://purl.org/iot/vocab/m3-lite#"/>
    </owl:Class>



     <!-- http://purl.org/iot/vocab/iot-taxonomy-lite#SleepDetector -->

    <owl:Class rdf:about="&iottaxolite;SleepDetector">
        <rdfs:subClassOf rdf:resource="&iottaxolite;SleepSensor"/>
        <rdfs:comment xml:lang="en">A sleep detector sensor which detects whether the human falls asleep or wakes up.</rdfs:comment>
        <rdfs:label xml:lang="en">Sleep Detector</rdfs:label>
        <rdfs:isDefinedBy rdf:resource="http://purl.org/iot/vocab/m3-lite#"/>
    </owl:Class>
    


    <!-- http://purl.org/iot/vocab/iot-taxonomy-lite#SleepMonitor -->

    <owl:Class rdf:about="&iottaxolite;SleepMonitor">
        <rdfs:subClassOf rdf:resource="&iottaxolite;SleepSensor"/>
        <rdfs:comment xml:lang="en">A sleep monitor sensor which tracks the human sleep state.</rdfs:comment>
        <rdfs:label xml:lang="en">Sleep Monitor</rdfs:label>
        <rdfs:isDefinedBy rdf:resource="http://purl.org/iot/vocab/m3-lite#"/>
    </owl:Class>
    


    <!-- http://purl.org/iot/vocab/iot-taxonomy-lite#SleepSensor -->

    <owl:Class rdf:about="&iottaxolite;SleepSensor">
        <rdfs:subClassOf rdf:resource="&sosa;Sensor"/>
        <rdfs:label xml:lang="en">Sleep Sensor</rdfs:label>
        <rdfs:isDefinedBy rdf:resource="http://purl.org/iot/vocab/m3-lite#"/>
    </owl:Class>
    


    <!-- http://purl.org/iot/vocab/iot-taxonomy-lite#SleepState -->

    <owl:Class rdf:about="&iottaxolite;SleepState">
        <rdfs:subClassOf rdf:resource="&sosa;ObservableProperty"/>
        <dc:description xml:lang="en">The event at which a person or animal sleep state has been detected. This could be measured as a Boolean, or labels if the state is not binary</dc:description>
        <rdfs:label xml:lang="en">Sleep State</rdfs:label>
        <rdfs:isDefinedBy rdf:resource="http://purl.org/iot/vocab/m3-lite#"/>
    </owl:Class>

    <!-- http://purl.org/iot/vocab/iot-taxonomy-lite#IdentifyOutlierObservsations -->
    
    <owl:Class rdf:about="&iottaxolite;IdentifyOutlierObservsations">
        <rdfs:subClassOf rdf:resource="&consent;Purpose"/>
        <rdfs:comment xml:lang="en">Purpose to identify if an observation is outlier or not.</rdfs:comment>
        <rdfs:label xml:lang="en">Identify Outlier Observsations</rdfs:label>
    </owl:Class>

    <!-- http://purl.org/iot/vocab/iot-taxonomy-lite#EnvironmentalChatbot -->
    
    <owl:Class rdf:about="&iottaxolite;EnvironmentalChatbot">
        <rdfs:subClassOf rdf:resource="&consent;Purpose"/>
        <rdfs:comment xml:lang="en">Purpose to create a chatbot that could provide environment related knowledge in a userfriendly manner.</rdfs:comment>
        <rdfs:label xml:lang="en">Environmental Chatbot</rdfs:label>
    </owl:Class>

    <!-- http://purl.org/iot/vocab/iot-taxonomy-lite#EnvironmentalDashboard -->
    
    <owl:Class rdf:about="&iottaxolite;EnvironmentalDashboard">
        <rdfs:subClassOf rdf:resource="&consent;Purpose"/>
        <rdfs:comment xml:lang="en">Purpose to create a dashbord that could provide environment related knowledge to the people.</rdfs:comment>
        <rdfs:label xml:lang="en">Environmental Dashboard</rdfs:label>
    </owl:Class>

    <!-- http://purl.org/iot/vocab/iot-taxonomy-lite#Meeting -->
    
    <owl:Class rdf:about="&iottaxolite;Meeting">
        <rdfs:subClassOf rdf:resource="&consent;Purpose"/>
        <rdfs:comment xml:lang="en">Purpose for either arranging a meeting or actually meeting someone.</rdfs:comment>
        <rdfs:label xml:lang="en">Meeting</rdfs:label>
    </owl:Class>

    <!-- http://purl.org/iot/vocab/iot-taxonomy-lite#EnterRoom -->
    
    <owl:Class rdf:about="&iottaxolite;EnterRoom">
        <rdfs:subClassOf rdf:resource="&consent;Purpose"/>
        <rdfs:comment xml:lang="en">Purpose for requesting to enter a room.</rdfs:comment>
        <rdfs:label xml:lang="en">Enter Room</rdfs:label>
    </owl:Class>

    <!-- http://purl.org/iot/vocab/iot-taxonomy-lite#MonitorTemperature -->
    
    <owl:Class rdf:about="&iottaxolite;MonitorTemperature">
        <rdfs:subClassOf rdf:resource="&consent;Purpose"/>
        <rdfs:comment xml:lang="en">Purpose for monitoring temperature.</rdfs:comment>
        <rdfs:label xml:lang="en">Monitor Temperature</rdfs:label>
    </owl:Class>

    <!-- http://purl.org/iot/vocab/iot-taxonomy-lite#CalculateEnergyConsumption -->
    
    <owl:Class rdf:about="&iottaxolite;CalculateEnergyConsumption">
        <rdfs:subClassOf rdf:resource="&consent;Purpose"/>
        <rdfs:comment xml:lang="en">Purpose of calculating energy consumption by a resource.</rdfs:comment>
        <rdfs:label xml:lang="en">Calculate Energy Consumption</rdfs:label>
    </owl:Class>

    <!-- http://purl.org/iot/vocab/iot-taxonomy-lite#MeetForCoffee -->
    
    <owl:Class rdf:about="&iottaxolite;MeetForCoffee">
        <rdfs:subClassOf rdf:resource="&iottaxolite;Meeting"/>
        <rdfs:comment xml:lang="en">Purpose of meeting a person for a coffee or arranging a meeting</rdfs:comment>
        <rdfs:label xml:lang="en">Meet For Coffee</rdfs:label>
    </owl:Class>


    <!-- http://purl.org/iot/vocab/iot-taxonomy-lite#ErrorCorrection -->
    
    <owl:Class rdf:about="&iottaxolite;ErrorCorrection">
        <rdfs:subClassOf rdf:resource="&consent;Action"/>
        <rdfs:comment xml:lang="en">Action related to finding error in the data and correcting them</rdfs:comment>
        <rdfs:label xml:lang="en">Error Correction</rdfs:label>
    </owl:Class>

    <!-- http://purl.org/iot/vocab/iot-taxonomy-lite#DiscoverObservsation -->
    
    <owl:Class rdf:about="&iottaxolite;DiscoverObservsation">
        <rdfs:subClassOf rdf:resource="&consent;Action"/>
        <rdfs:comment xml:lang="en">Action related to finding observsations either of a particular kind or all.</rdfs:comment>
        <rdfs:label xml:lang="en">Discover Observsation</rdfs:label>
    </owl:Class>

    <!-- http://purl.org/iot/vocab/iot-taxonomy-lite#OpenTheDoor -->
    
    <owl:Class rdf:about="&iottaxolite;OpenTheDoor">
        <rdfs:subClassOf rdf:resource="&consent;Action"/>
        <rdfs:comment xml:lang="en">Action related to either request for opening the door or actually opening it.</rdfs:comment>
        <rdfs:label xml:lang="en">Open The Door</rdfs:label>
    </owl:Class>

</rdf:RDF>




<!-- Generated by the OWL API (version 4.2.1.20160306-0033) https://github.com/owlcs/owlapi -->

